<?xml version="1.0" encoding="utf-8"?>
<!DOCTYPE rdf:RDF [
 <!ENTITY owl  "http://www.w3.org/2002/07/owl#">
 <!ENTITY rdf  "http://www.w3.org/1999/02/22-rdf-syntax-ns#">
 <!ENTITY rdfs "http://www.w3.org/2000/01/rdf-schema#">
 <!ENTITY dc   "http://purl.org/dc/elements/1.1/">
 <!ENTITY dcterms  "http://purl.org/dc/terms/">
 <!ENTITY foaf "http://xmlns.com/foaf/0.1/">
 <!ENTITY skos "http://www.w3.org/2004/02/skos/core#">
 <!ENTITY sioc "http://rdfs.org/sioc/ns#">
 <!ENTITY sioct "http://rdfs.org/sioc/types#">
 <!ENTITY geo "http://www.w3.org/2003/01/geo/wgs84_pos#">
 <!ENTITY xsd  "http://www.w3.org/2001/XMLSchema#" >
 <!ENTITY rel "http://purl.org/vocab/relationship/" >
]>

<rdf:RDF
	xmlns:owl="&owl;" xmlns:rdf="&rdf;" xmlns:rdfs="&rdfs;"
	xmlns:dc="&dc;" xmlns:dcterms="&dcterms;" xmlns:skos="&skos;"
	xmlns:foaf="&foaf;" xmlns:sioc="&sioc;" xmlns:sioct="&sioct;" xmlns:rel="&rel;"
	xmlns:vs="http://www.w3.org/2003/06/sw-vocab-status/ns#" 
>

<owl:Ontology rdf:about="http://ns.ontowiki.net/SysBase/">
  <rdfs:label>OntoWiki System Base</rdfs:label>
	<owl:versionInfo>$Id: SysBase.rdf 4285 2009-10-12 13:15:09Z sebastian.dietzold $</owl:versionInfo>
  <owl:versionInfo rdf:resource="http://code.google.com/p/ontowiki/source/list?path=/trunk/ontowiki/src/application/config/SysBase.rdf" />
  <rdfs:comment>This is a collection of several property and class descriptions intended to be imported automatically.</rdfs:comment>
	<dcterms:description>This model consists of all statements from the RDF, RDFS, OWL, DC, DCTERMS, SKOS, FOAF, SIOC and GEO namespaces to provide proper labels for standard properties and support better resource selection for standard object properties.</dcterms:description>
  <skos:note>Do NOT import this ontology directly! Instead, use the original resources you got from the seeAlso links.</skos:note>
  <skos:editorialNote>Inside OntoWiki, this model is used for the following tasks: (1) property selection in edit widgets (2) property labels in several tabs and modules.</skos:editorialNote>
	<rdfs:seeAlso rdf:resource="&owl;" />
	<rdfs:seeAlso rdf:resource="&rdf;" />
	<rdfs:seeAlso rdf:resource="&rdfs;" />
	<rdfs:seeAlso rdf:resource="&dc;" />
	<rdfs:seeAlso rdf:resource="&dcterms;" />
	<rdfs:seeAlso rdf:resource="&skos;" />
	<rdfs:seeAlso rdf:resource="&foaf;" />
	<rdfs:seeAlso rdf:resource="&sioc;" />
	<rdfs:seeAlso rdf:resource="&geo;" />
	<rdfs:seeAlso rdf:resource="&rel;" />
</owl:Ontology>

<!-- RDF -->

<rdf:Property rdf:about="&rdf;type">
  <rdfs:label>type</rdfs:label>
  <rdfs:comment>The subject is an instance of a class.</rdfs:comment>
  <rdfs:range rdf:resource="&rdfs;Class"/>
  <rdfs:domain rdf:resource="&rdfs;Resource"/>
</rdf:Property>

<rdf:Description rdf:about="&rdf;Property">
  <rdfs:label>Property</rdfs:label>
  <rdfs:comment>The class of RDF properties.</rdfs:comment>
</rdf:Description>

<rdf:Description rdf:about="&rdf;Statement">
  <rdfs:label>Statement</rdfs:label>
  <rdfs:comment>The class of RDF statements.</rdfs:comment>
</rdf:Description>

<rdf:Property rdf:about="&rdf;subject">
  <rdfs:label>subject</rdfs:label>
  <rdfs:comment>The subject of the subject RDF statement.</rdfs:comment>
  <rdfs:domain rdf:resource="&rdf;Statement"/>
  <rdfs:range rdf:resource="&rdfs;Resource"/>
</rdf:Property>

<rdf:Property rdf:about="&rdf;predicate">
  <rdfs:label>predicate</rdfs:label>
  <rdfs:comment>The predicate of the subject RDF statement.</rdfs:comment>
  <rdfs:domain rdf:resource="&rdf;Statement"/>
  <rdfs:range rdf:resource="&rdfs;Resource"/>
</rdf:Property>

<rdf:Property rdf:about="&rdf;object">
  <rdfs:label>object</rdfs:label>
  <rdfs:comment>The object of the subject RDF statement.</rdfs:comment>
  <rdfs:domain rdf:resource="&rdf;Statement"/>
  <rdfs:range rdf:resource="&rdfs;Resource"/>
</rdf:Property>

<rdf:Description rdf:about="&rdf;Bag">
  <rdfs:label>Bag</rdfs:label>
  <rdfs:comment>The class of unordered containers.</rdfs:comment>
</rdf:Description>

<rdf:Description rdf:about="&rdf;Seq">
  <rdfs:label>Seq</rdfs:label>
  <rdfs:comment>The class of ordered containers.</rdfs:comment>
</rdf:Description>

<rdf:Description rdf:about="&rdf;Alt">
  <rdfs:label>Alt</rdfs:label>
  <rdfs:comment>The class of containers of alternatives.</rdfs:comment>
</rdf:Description>

<rdf:Property rdf:about="&rdf;value">
  <rdfs:label>value</rdfs:label>
  <rdfs:comment>Idiomatic property used for structured values.</rdfs:comment>
  <rdfs:domain rdf:resource="&rdfs;Resource"/>
  <rdfs:range rdf:resource="&rdfs;Resource"/>
</rdf:Property>

<!-- the following are new additions, Nov 2002 -->

<rdf:Description rdf:about="&rdf;List">
  <rdfs:label>List</rdfs:label>
  <rdfs:comment>The class of RDF Lists.</rdfs:comment>
</rdf:Description>

<rdf:List rdf:about="&rdf;nil">
  <rdfs:label>nil</rdfs:label>
  <rdfs:comment>The empty list, with no items in it. If the rest of a list is nil then the list has no more items in it.</rdfs:comment>
</rdf:List>

<rdf:Property rdf:about="&rdf;first">
  <rdfs:label>first</rdfs:label>
  <rdfs:comment>The first item in the subject RDF list.</rdfs:comment>
  <rdfs:domain rdf:resource="&rdf;List"/>
  <rdfs:range rdf:resource="&rdfs;Resource"/>
</rdf:Property>

<rdf:Property rdf:about="&rdf;rest">
  <rdfs:label>rest</rdfs:label>
  <rdfs:comment>The rest of the subject RDF list after the first item.</rdfs:comment>
  <rdfs:domain rdf:resource="&rdf;List"/>
  <rdfs:range rdf:resource="&rdf;List"/>
</rdf:Property>
	
<rdfs:Datatype rdf:about="&rdf;XMLLiteral">
  <rdfs:label>XMLLiteral</rdfs:label>
  <rdfs:comment>The class of XML literal values.</rdfs:comment>
</rdfs:Datatype>

<rdf:Description rdf:about="&rdf;">
  <rdfs:seeAlso rdf:resource="http://www.w3.org/2000/01/rdf-schema-more"/>
</rdf:Description>


<!-- RDF Schema -->


<rdf:Description rdf:about="http://www.w3.org/2000/01/rdf-schema#Resource">
  <rdfs:isDefinedBy rdf:resource="http://www.w3.org/2000/01/rdf-schema#"/>
  <rdfs:label>Resource</rdfs:label>
  <rdfs:comment>The class resource, everything.</rdfs:comment>
</rdf:Description>

<rdf:Description rdf:about="http://www.w3.org/2000/01/rdf-schema#Class">

  <rdfs:isDefinedBy rdf:resource="http://www.w3.org/2000/01/rdf-schema#"/>
  <rdfs:label>Class</rdfs:label>
  <rdfs:comment>The class of classes.</rdfs:comment>
</rdf:Description>

<rdf:Property rdf:about="http://www.w3.org/2000/01/rdf-schema#subClassOf">
  <rdfs:isDefinedBy rdf:resource="http://www.w3.org/2000/01/rdf-schema#"/>
  <rdfs:label>subClassOf</rdfs:label>

  <rdfs:comment>The subject is a subclass of a class.</rdfs:comment>
  <rdfs:range rdf:resource="http://www.w3.org/2000/01/rdf-schema#Class"/>
  <rdfs:domain rdf:resource="http://www.w3.org/2000/01/rdf-schema#Class"/>
</rdf:Property>

<rdf:Property rdf:about="http://www.w3.org/2000/01/rdf-schema#subPropertyOf">
  <rdfs:isDefinedBy rdf:resource="http://www.w3.org/2000/01/rdf-schema#"/>
  <rdfs:label>subPropertyOf</rdfs:label>
  <rdfs:comment>The subject is a subproperty of a property.</rdfs:comment>

  <rdfs:range rdf:resource="&rdfs;Property"/>
  <rdfs:domain rdf:resource="&rdfs;Property"/>
</rdf:Property>

<rdf:Property rdf:about="http://www.w3.org/2000/01/rdf-schema#comment">
  <rdfs:isDefinedBy rdf:resource="http://www.w3.org/2000/01/rdf-schema#"/>
  <rdfs:label>comment</rdfs:label>
  <rdfs:comment>A description of the subject resource.</rdfs:comment>
  <rdfs:domain rdf:resource="http://www.w3.org/2000/01/rdf-schema#Resource"/>

  <rdfs:range rdf:resource="http://www.w3.org/2000/01/rdf-schema#Literal"/>
</rdf:Property>

<rdf:Property rdf:about="http://www.w3.org/2000/01/rdf-schema#label">
  <rdfs:isDefinedBy rdf:resource="http://www.w3.org/2000/01/rdf-schema#"/>
  <rdfs:label>label</rdfs:label>
  <rdfs:comment>A human-readable name for the subject.</rdfs:comment>
  <rdfs:domain rdf:resource="http://www.w3.org/2000/01/rdf-schema#Resource"/>
  <rdfs:range rdf:resource="http://www.w3.org/2000/01/rdf-schema#Literal"/>

</rdf:Property>

<rdf:Property rdf:about="http://www.w3.org/2000/01/rdf-schema#domain">
  <rdfs:isDefinedBy rdf:resource="http://www.w3.org/2000/01/rdf-schema#"/>
  <rdfs:label>domain</rdfs:label>
  <rdfs:comment>A domain of the subject property.</rdfs:comment>
 <rdfs:range rdf:resource="http://www.w3.org/2000/01/rdf-schema#Class"/>
  <rdfs:domain rdf:resource="&rdfs;Property"/>
</rdf:Property>

<rdf:Property rdf:about="http://www.w3.org/2000/01/rdf-schema#range">
  <rdfs:isDefinedBy rdf:resource="http://www.w3.org/2000/01/rdf-schema#"/>
  <rdfs:label>range</rdfs:label>
  <rdfs:comment>A range of the subject property.</rdfs:comment>
  <rdfs:range rdf:resource="http://www.w3.org/2000/01/rdf-schema#Class"/>
  <rdfs:domain rdf:resource="&rdfs;Property"/>
</rdf:Property>

<rdf:Property rdf:about="http://www.w3.org/2000/01/rdf-schema#seeAlso">
  <rdfs:isDefinedBy rdf:resource="http://www.w3.org/2000/01/rdf-schema#"/>

  <rdfs:label>seeAlso</rdfs:label>
  <rdfs:comment>Further information about the subject resource.</rdfs:comment>
  <rdfs:range rdf:resource="http://www.w3.org/2000/01/rdf-schema#Resource"/>
  <rdfs:domain   rdf:resource="http://www.w3.org/2000/01/rdf-schema#Resource"/>
</rdf:Property>

<rdf:Property rdf:about="http://www.w3.org/2000/01/rdf-schema#isDefinedBy">
  <rdfs:isDefinedBy rdf:resource="http://www.w3.org/2000/01/rdf-schema#"/>
  <rdfs:subPropertyOf rdf:resource="http://www.w3.org/2000/01/rdf-schema#seeAlso"/>

  <rdfs:label>isDefinedBy</rdfs:label>
  <rdfs:comment>The defininition of the subject resource.</rdfs:comment>
  <rdfs:range rdf:resource="http://www.w3.org/2000/01/rdf-schema#Resource"/>
  <rdfs:domain rdf:resource="http://www.w3.org/2000/01/rdf-schema#Resource"/>
</rdf:Property>

<rdf:Description rdf:about="http://www.w3.org/2000/01/rdf-schema#Literal">
  <rdfs:isDefinedBy rdf:resource="http://www.w3.org/2000/01/rdf-schema#"/>
  <rdfs:label>Literal</rdfs:label>

  <rdfs:comment>The class of literal values, eg. textual strings and integers.</rdfs:comment>
</rdf:Description>

<rdf:Description rdf:about="http://www.w3.org/2000/01/rdf-schema#Container">
  <rdfs:isDefinedBy rdf:resource="http://www.w3.org/2000/01/rdf-schema#"/>
  <rdfs:label>Container</rdfs:label>
  <rdfs:comment>The class of RDF containers.</rdfs:comment>

</rdf:Description>

<rdf:Description rdf:about="http://www.w3.org/2000/01/rdf-schema#ContainerMembershipProperty">
  <rdfs:isDefinedBy rdf:resource="http://www.w3.org/2000/01/rdf-schema#"/>
  <rdfs:label>ContainerMembershipProperty</rdfs:label>
  <rdfs:comment>The class of container membership properties, rdf:_1, rdf:_2, ...,
                    all of which are sub-properties of 'member'.</rdfs:comment>
</rdf:Description>

<rdf:Property rdf:about="http://www.w3.org/2000/01/rdf-schema#member">
  <rdfs:isDefinedBy rdf:resource="http://www.w3.org/2000/01/rdf-schema#"/>

  <rdfs:label>member</rdfs:label>
  <rdfs:comment>A member of the subject resource.</rdfs:comment>
  <rdfs:domain rdf:resource="http://www.w3.org/2000/01/rdf-schema#Resource"/>
  <rdfs:range rdf:resource="http://www.w3.org/2000/01/rdf-schema#Resource"/>
</rdf:Property>

<rdf:Description rdf:about="http://www.w3.org/2000/01/rdf-schema#Datatype">
  <rdfs:isDefinedBy rdf:resource="http://www.w3.org/2000/01/rdf-schema#"/>
  <rdfs:label>Datatype</rdfs:label>

  <rdfs:comment>The class of RDF datatypes.</rdfs:comment>
</rdf:Description>
	
<!-- OWL -->



<rdf:Description rdf:about="&owl;Class">
  <rdfs:label>Class</rdfs:label>
</rdf:Description>

<rdf:Description rdf:about="&owl;Thing">
  <rdfs:label>Thing</rdfs:label>
</rdf:Description>

<rdf:Description rdf:about="&owl;Nothing">
  <rdfs:label>Nothing</rdfs:label>
  <owl:complementOf rdf:resource="&owl;Thing"/>
</rdf:Description>

<rdf:Property rdf:about="&owl;equivalentClass">
  <rdfs:label>equivalentClass</rdfs:label>
  <rdfs:domain rdf:resource="&owl;Class"/>
  <rdfs:range rdf:resource="&owl;Class"/>
</rdf:Property>

<rdf:Property rdf:about="&owl;disjointWith">
  <rdfs:label>disjointWith</rdfs:label>
  <rdfs:domain rdf:resource="&owl;Class"/>
  <rdfs:range rdf:resource="&owl;Class"/>
</rdf:Property>

<rdf:Property rdf:about="&owl;equivalentProperty">
  <rdfs:label>equivalentProperty</rdfs:label>
  <rdfs:subPropertyOf rdf:resource="&rdfs;subPropertyOf"/>
</rdf:Property>

<rdf:Property rdf:about="&owl;sameAs"> 
  <rdfs:label>sameAs</rdfs:label>
  <rdfs:domain rdf:resource="&owl;Thing"/>
  <rdfs:range rdf:resource="&owl;Thing"/>
</rdf:Property>

<rdf:Property rdf:about="&owl;differentFrom">
  <rdfs:label>differentFrom</rdfs:label>
  <rdfs:domain rdf:resource="&owl;Thing"/>
  <rdfs:range rdf:resource="&owl;Thing"/>
</rdf:Property>

<rdf:Description rdf:about="&owl;AllDifferent">
  <rdfs:label>AllDifferent</rdfs:label>
</rdf:Description>

<rdf:Property rdf:about="&owl;distinctMembers">
  <rdfs:label>distinctMembers</rdfs:label>
  <rdfs:domain rdf:resource="&owl;AllDifferent"/>
  <rdfs:range rdf:resource="&rdf;List"/>
</rdf:Property>
  
<rdf:Property rdf:about="&owl;unionOf">
  <rdfs:label>unionOf</rdfs:label>
  <rdfs:domain rdf:resource="&owl;Class"/>
  <rdfs:range rdf:resource="&rdf;List"/>
</rdf:Property>

<rdf:Property rdf:about="&owl;intersectionOf">
  <rdfs:label>intersectionOf</rdfs:label>
  <rdfs:domain rdf:resource="&owl;Class"/>
  <rdfs:range rdf:resource="&rdf;List"/>
</rdf:Property>

<rdf:Property rdf:about="&owl;complementOf">
  <rdfs:label>complementOf</rdfs:label>
  <rdfs:domain rdf:resource="&owl;Class"/>
  <rdfs:range rdf:resource="&owl;Class"/>
</rdf:Property>

<rdf:Property rdf:about="&owl;oneOf">
  <rdfs:label>oneOf</rdfs:label>
  <rdfs:domain rdf:resource="&rdfs;Class"/>
  <rdfs:range rdf:resource="&rdf;List"/>
</rdf:Property>

<rdf:Description rdf:about="&owl;Restriction">
  <rdfs:label>Restriction</rdfs:label>
</rdf:Description>

<rdf:Property rdf:about="&owl;onProperty">
  <rdfs:label>onProperty</rdfs:label>
  <rdfs:domain rdf:resource="&owl;Restriction"/>
  <rdfs:range rdf:resource="&rdf;Property"/>
</rdf:Property>

<rdf:Property rdf:about="&owl;allValuesFrom">
  <rdfs:label>allValuesFrom</rdfs:label>
  <rdfs:domain rdf:resource="&owl;Restriction"/>
  <rdfs:range rdf:resource="&rdfs;Class"/>
</rdf:Property>

<rdf:Property rdf:about="&owl;hasValue">
  <rdfs:label>hasValue</rdfs:label>
  <rdfs:domain rdf:resource="&owl;Restriction"/>
</rdf:Property>

<rdf:Property rdf:about="&owl;someValuesFrom">
  <rdfs:label>someValuesFrom</rdfs:label>
  <rdfs:domain rdf:resource="&owl;Restriction"/>
  <rdfs:range rdf:resource="&rdfs;Class"/>
</rdf:Property>

<rdf:Property rdf:about="&owl;minCardinality">
  <rdfs:label>minCardinality</rdfs:label>
  <rdfs:domain rdf:resource="&owl;Restriction"/>
  <rdfs:range rdf:resource="&xsd;nonNegativeInteger"/>
</rdf:Property>

<rdf:Property rdf:about="&owl;maxCardinality">
  <rdfs:label>maxCardinality</rdfs:label>
  <rdfs:domain rdf:resource="&owl;Restriction"/>
  <rdfs:range rdf:resource="&xsd;nonNegativeInteger"/>
</rdf:Property>

<rdf:Property rdf:about="&owl;cardinality">
  <rdfs:label>cardinality</rdfs:label>
  <rdfs:domain rdf:resource="&owl;Restriction"/>
  <rdfs:range rdf:resource="&xsd;nonNegativeInteger"/>
</rdf:Property>

<rdf:Description rdf:about="&owl;ObjectProperty">
  <rdfs:label>ObjectProperty</rdfs:label>
</rdf:Description>

<rdf:Description rdf:about="&owl;DatatypeProperty">
  <rdfs:label>DatatypeProperty</rdfs:label>
</rdf:Description>

<rdf:Property rdf:about="&owl;inverseOf">
  <rdfs:label>inverseOf</rdfs:label>
  <rdfs:domain rdf:resource="&owl;ObjectProperty"/>
  <rdfs:range rdf:resource="&owl;ObjectProperty"/>
</rdf:Property>

<rdf:Description rdf:about="&owl;TransitiveProperty">
  <rdfs:label>TransitiveProperty</rdfs:label>
</rdf:Description>

<rdf:Description rdf:about="&owl;SymmetricProperty">
  <rdfs:label>SymmetricProperty</rdfs:label>
</rdf:Description>

<rdf:Description rdf:about="&owl;FunctionalProperty">
  <rdfs:label>FunctionalProperty</rdfs:label>
</rdf:Description>

<rdf:Description rdf:about="&owl;InverseFunctionalProperty">
  <rdfs:label>InverseFunctionalProperty</rdfs:label>
</rdf:Description>

<rdf:Description rdf:about="&owl;AnnotationProperty">
  <rdfs:label>AnnotationProperty</rdfs:label>
</rdf:Description>

<owl:AnnotationProperty rdf:about="&rdfs;label"/>
<owl:AnnotationProperty rdf:about="&rdfs;comment"/>
<owl:AnnotationProperty rdf:about="&rdfs;seeAlso"/>
<owl:AnnotationProperty rdf:about="&rdfs;isDefinedBy"/>

<rdf:Description rdf:about="&owl;Ontology">
  <rdfs:label>Ontology</rdfs:label>
</rdf:Description>

<rdf:Description rdf:about="&owl;OntologyProperty">
  <rdfs:label>OntologyProperty</rdfs:label>
</rdf:Description>

<rdf:Property rdf:about="&owl;imports">
  <rdfs:label>imports</rdfs:label>
  <rdf:type rdf:resource="&owl;OntologyProperty"/>
  <rdfs:domain rdf:resource="&owl;Ontology"/>
  <rdfs:range rdf:resource="&owl;Ontology"/>
</rdf:Property>

<rdf:Property rdf:about="&owl;versionInfo">
  <rdfs:label>versionInfo</rdfs:label>
  <rdf:type rdf:resource="&owl;AnnotationProperty"/>
</rdf:Property>

<rdf:Property rdf:about="&owl;priorVersion">
  <rdfs:label>priorVersion</rdfs:label>
  <rdf:type rdf:resource="&owl;OntologyProperty"/>
  <rdfs:domain rdf:resource="&owl;Ontology"/>
  <rdfs:range rdf:resource="&owl;Ontology"/>
</rdf:Property>

<rdf:Property rdf:about="&owl;backwardCompatibleWith">
  <rdfs:label>backwardCompatibleWith</rdfs:label>
  <rdf:type rdf:resource="&owl;OntologyProperty"/>
  <rdfs:domain rdf:resource="&owl;Ontology"/>
  <rdfs:range rdf:resource="&owl;Ontology"/>
</rdf:Property>

<rdf:Property rdf:about="&owl;incompatibleWith">
  <rdfs:label>incompatibleWith</rdfs:label>
  <rdf:type rdf:resource="&owl;OntologyProperty"/>
  <rdfs:domain rdf:resource="&owl;Ontology"/>
  <rdfs:range rdf:resource="&owl;Ontology"/>
</rdf:Property>

<rdf:Description rdf:about="&owl;DeprecatedClass">
  <rdfs:label>DeprecatedClass</rdfs:label>
</rdf:Description>

<rdf:Description rdf:about="&owl;DeprecatedProperty">
  <rdfs:label>DeprecatedProperty</rdfs:label>
</rdf:Description>

<rdf:Description rdf:about="&owl;DataRange">
  <rdfs:label>DataRange</rdfs:label>
</rdf:Description>

<!-- DC -->

<rdf:Property rdf:about="&dc;title">
<rdfs:label xml:lang="en">Title</rdfs:label>
<rdfs:comment xml:lang="en">A name given to the resource.</rdfs:comment>
<dcterms:hasVersion rdf:resource="http://dublincore.org/usage/terms/history/#title-006"/>
</rdf:Property>

<rdf:Property rdf:about="&dc;creator">
<rdfs:label xml:lang="en">Creator</rdfs:label>
<rdfs:comment xml:lang="en">An entity primarily responsible for making the resource.</rdfs:comment>
<dcterms:description xml:lang="en">Examples of a Creator include a person, an organization, or a service. Typically, the name of a Creator should be used to indicate the entity.</dcterms:description>
<dcterms:hasVersion rdf:resource="http://dublincore.org/usage/terms/history/#creator-006"/>
</rdf:Property>

<rdf:Property rdf:about="&dc;subject">
<rdfs:label xml:lang="en">Subject</rdfs:label>
<rdfs:comment xml:lang="en">The topic of the resource.</rdfs:comment>
<dcterms:description xml:lang="en">Typically, the subject will be represented using keywords, key phrases, or classification codes. Recommended best practice is to use a controlled vocabulary. To describe the spatial or temporal topic of the resource, use the Coverage element.</dcterms:description>
<dcterms:hasVersion rdf:resource="http://dublincore.org/usage/terms/history/#subject-006"/>
</rdf:Property>

<rdf:Property rdf:about="&dc;description">
<rdfs:label xml:lang="en">Description</rdfs:label>
<rdfs:comment xml:lang="en">An account of the resource.</rdfs:comment>
<dcterms:description xml:lang="en">Description may include but is not limited to: an abstract, a table of contents, a graphical representation, or a free-text account of the resource.</dcterms:description>
<dcterms:hasVersion rdf:resource="http://dublincore.org/usage/terms/history/#description-006"/>
</rdf:Property>

<rdf:Property rdf:about="&dc;publisher">
<rdfs:label xml:lang="en">Publisher</rdfs:label>
<rdfs:comment xml:lang="en">An entity responsible for making the resource available.</rdfs:comment>
<dcterms:description xml:lang="en">Examples of a Publisher include a person, an organization, or a service. Typically, the name of a Publisher should be used to indicate the entity.</dcterms:description>
<dcterms:hasVersion rdf:resource="http://dublincore.org/usage/terms/history/#publisher-006"/>
</rdf:Property>

<rdf:Property rdf:about="&dc;contributor">
<rdfs:label xml:lang="en">Contributor</rdfs:label>
<rdfs:comment xml:lang="en">An entity responsible for making contributions to the resource.</rdfs:comment>
<dcterms:description xml:lang="en">Examples of a Contributor include a person, an organization, or a service. Typically, the name of a Contributor should be used to indicate the entity.</dcterms:description>
<dcterms:hasVersion rdf:resource="http://dublincore.org/usage/terms/history/#contributor-006"/>
</rdf:Property>

<rdf:Property rdf:about="&dc;date">
<rdfs:label xml:lang="en">Date</rdfs:label>
<rdfs:comment xml:lang="en">A point or period of time associated with an event in the lifecycle of the resource.</rdfs:comment>
<dcterms:description xml:lang="en">Date may be used to express temporal information at any level of granularity.  Recommended best practice is to use an encoding scheme, such as the W3CDTF profile of ISO 8601 [W3CDTF].</dcterms:description>
<dcterms:hasVersion rdf:resource="http://dublincore.org/usage/terms/history/#date-006"/>
</rdf:Property>

<rdf:Property rdf:about="&dc;type">
<rdfs:label xml:lang="en">Type</rdfs:label>
<rdfs:comment xml:lang="en">The nature or genre of the resource.</rdfs:comment>
<dcterms:description xml:lang="en">Recommended best practice is to use a controlled vocabulary such as the DCMI Type Vocabulary [DCMITYPE]. To describe the file format, physical medium, or dimensions of the resource, use the Format element.</dcterms:description>
<dcterms:hasVersion rdf:resource="http://dublincore.org/usage/terms/history/#type-006"/>
</rdf:Property>

<rdf:Property rdf:about="&dc;format">
<rdfs:label xml:lang="en">Format</rdfs:label>
<rdfs:comment xml:lang="en">The file format, physical medium, or dimensions of the resource.</rdfs:comment>
<dcterms:description xml:lang="en">Examples of dimensions include size and duration. Recommended best practice is to use a controlled vocabulary such as the list of Internet Media Types [MIME].</dcterms:description>
<dcterms:hasVersion rdf:resource="http://dublincore.org/usage/terms/history/#format-007"/>
</rdf:Property>

<rdf:Property rdf:about="&dc;identifier">
<rdfs:label xml:lang="en">Identifier</rdfs:label>
<rdfs:comment xml:lang="en">An unambiguous reference to the resource within a given context.</rdfs:comment>
<dcterms:description xml:lang="en">Recommended best practice is to identify the resource by means of a string conforming to a formal identification system. </dcterms:description>
<dcterms:hasVersion rdf:resource="http://dublincore.org/usage/terms/history/#identifier-006"/>
</rdf:Property>

<rdf:Property rdf:about="&dc;source">
<rdfs:label xml:lang="en">Source</rdfs:label>
<rdfs:comment xml:lang="en">A related resource from which the described resource is derived.</rdfs:comment>
<dcterms:description xml:lang="en">The described resource may be derived from the related resource in whole or in part. Recommended best practice is to identify the related resource by means of a string conforming to a formal identification system.</dcterms:description>
<dcterms:hasVersion rdf:resource="http://dublincore.org/usage/terms/history/#source-006"/>
</rdf:Property>

<rdf:Property rdf:about="&dc;language">
<rdfs:label xml:lang="en">Language</rdfs:label>
<rdfs:comment xml:lang="en">A language of the resource.</rdfs:comment>
<dcterms:description xml:lang="en">Recommended best practice is to use a controlled vocabulary such as RFC 4646 [RFC4646].</dcterms:description>
<dcterms:hasVersion rdf:resource="http://dublincore.org/usage/terms/history/#language-007"/>
<rdfs:seeAlso rdf:resource="http://www.ietf.org/rfc/rfc4646.txt"/>
</rdf:Property>

<rdf:Property rdf:about="&dc;relation">
<rdfs:label xml:lang="en">Relation</rdfs:label>
<rdfs:comment xml:lang="en">A related resource.</rdfs:comment>
<dcterms:description xml:lang="en">Recommended best practice is to identify the related resource by means of a string conforming to a formal identification system. </dcterms:description>
<dcterms:hasVersion rdf:resource="http://dublincore.org/usage/terms/history/#relation-006"/>
</rdf:Property>

<rdf:Property rdf:about="&dc;coverage">
<rdfs:label xml:lang="en">Coverage</rdfs:label>
<rdfs:comment xml:lang="en">The spatial or temporal topic of the resource, the spatial applicability of the resource, or the jurisdiction under which the resource is relevant.</rdfs:comment>
<dcterms:description xml:lang="en">Spatial topic and spatial applicability may be a named place or a location specified by its geographic coordinates. Temporal topic may be a named period, date, or date range. A jurisdiction may be a named administrative entity or a geographic place to which the resource applies. Recommended best practice is to use a controlled vocabulary such as the Thesaurus of Geographic Names [TGN]. Where appropriate, named places or time periods can be used in preference to numeric identifiers such as sets of coordinates or date ranges.</dcterms:description>
<dcterms:hasVersion rdf:resource="http://dublincore.org/usage/terms/history/#coverage-006"/>
</rdf:Property>

<rdf:Property rdf:about="&dc;rights">
<rdfs:label xml:lang="en">Rights</rdfs:label>
<rdfs:comment xml:lang="en">Information about rights held in and over the resource.</rdfs:comment>
<dcterms:description xml:lang="en">Typically, rights information includes a statement about various property rights associated with the resource, including intellectual property rights.</dcterms:description>
<dcterms:hasVersion rdf:resource="http://dublincore.org/usage/terms/history/#rights-006"/>
</rdf:Property>


<!-- DCTERMS -->


<rdf:Description rdf:about="&dcterms;title">
<rdfs:label xml:lang="en">Title</rdfs:label>
<dcterms:description xml:lang="en">A name given to the resource.</dcterms:description>
<rdf:type rdf:resource="&rdf;Property"/>
<dcterms:hasVersion rdf:resource="http://dublincore.org/usage/terms/history/#titleT-001"/>
<skos:note xml:lang="en">In current practice, this term is used primarily with literal values; however, there are important uses with non-literal values as well.  As of December 2007, the DCMI Usage Board is leaving this range unspecified pending an investigation of options.</skos:note>
<rdfs:subPropertyOf rdf:resource="http://purl.org/dc/elements/1.1/title"/>
</rdf:Description>

<rdf:Description rdf:about="&dcterms;creator">
<rdfs:label xml:lang="en">Creator</rdfs:label>
<rdfs:comment xml:lang="en">An entity primarily responsible for making the resource.</rdfs:comment>
<dcterms:description xml:lang="en">Examples of a Creator include a person, an organization, or a service. Typically, the name of a Creator should be used to indicate the entity.</dcterms:description>
<rdf:type rdf:resource="&rdf;Property"/>
<dcterms:hasVersion rdf:resource="http://dublincore.org/usage/terms/history/#creatorT-001"/>
<rdfs:range rdf:resource="&dcterms;Agent"/>
<rdfs:subPropertyOf rdf:resource="http://purl.org/dc/elements/1.1/creator"/>
<rdfs:subPropertyOf rdf:resource="&dcterms;contributor"/>
</rdf:Description>

<rdf:Description rdf:about="&dcterms;subject">
<rdfs:label xml:lang="en">Subject</rdfs:label>
<rdfs:comment xml:lang="en">The topic of the resource.</rdfs:comment>
<dcterms:description xml:lang="en">Typically, the subject will be represented using keywords, key phrases, or classification codes. Recommended best practice is to use a controlled vocabulary. To describe the spatial or temporal topic of the resource, use the Coverage element.</dcterms:description>
<rdf:type rdf:resource="&rdf;Property"/>
<dcterms:hasVersion rdf:resource="http://dublincore.org/usage/terms/history/#subjectT-001"/>
<skos:note xml:lang="en">This term is intended to be used with non-literal values as defined in the DCMI Abstract Model (http://dublincore.org/documents/abstract-model/).  As of December 2007, the DCMI Usage Board is seeking a way to express this intention with a formal range declaration.</skos:note>
<rdfs:subPropertyOf rdf:resource="http://purl.org/dc/elements/1.1/subject"/>
</rdf:Description>

<rdf:Description rdf:about="&dcterms;description">
<rdfs:label xml:lang="en">Description</rdfs:label>
<rdfs:comment xml:lang="en">An account of the resource.</rdfs:comment>
<dcterms:description xml:lang="en">Description may include but is not limited to: an abstract, a table of contents, a graphical representation, or a free-text account of the resource.</dcterms:description>
<rdf:type rdf:resource="&rdf;Property"/>
<dcterms:hasVersion rdf:resource="http://dublincore.org/usage/terms/history/#descriptionT-001"/>
<rdfs:subPropertyOf rdf:resource="http://purl.org/dc/elements/1.1/description"/>
</rdf:Description>

<rdf:Description rdf:about="&dcterms;publisher">
<rdfs:label xml:lang="en">Publisher</rdfs:label>
<rdfs:comment xml:lang="en">An entity responsible for making the resource available.</rdfs:comment>
<dcterms:description xml:lang="en">Examples of a Publisher include a person, an organization, or a service. Typically, the name of a Publisher should be used to indicate the entity.</dcterms:description>
<rdf:type rdf:resource="&rdf;Property"/>
<dcterms:hasVersion rdf:resource="http://dublincore.org/usage/terms/history/#publisherT-001"/>
<rdfs:range rdf:resource="&dcterms;Agent"/>
<rdfs:subPropertyOf rdf:resource="http://purl.org/dc/elements/1.1/publisher"/>
</rdf:Description>

<rdf:Description rdf:about="&dcterms;contributor">
<rdfs:label xml:lang="en">Contributor</rdfs:label>
<rdfs:comment xml:lang="en">An entity responsible for making contributions to the resource.</rdfs:comment>
<dcterms:description xml:lang="en">Examples of a Contributor include a person, an organization, or a service. Typically, the name of a Contributor should be used to indicate the entity.</dcterms:description>
<rdf:type rdf:resource="&rdf;Property"/>
<dcterms:hasVersion rdf:resource="http://dublincore.org/usage/terms/history/#contributorT-001"/>
<rdfs:range rdf:resource="&dcterms;Agent"/>
<rdfs:subPropertyOf rdf:resource="http://purl.org/dc/elements/1.1/contributor"/>
</rdf:Description>

<rdf:Description rdf:about="&dcterms;date">
<rdfs:label xml:lang="en">Date</rdfs:label>
<rdfs:comment xml:lang="en">A point or period of time associated with an event in the lifecycle of the resource.</rdfs:comment>
<dcterms:description xml:lang="en">Date may be used to express temporal information at any level of granularity.  Recommended best practice is to use an encoding scheme, such as the W3CDTF profile of ISO 8601 [W3CDTF].</dcterms:description>
<rdf:type rdf:resource="&rdf;Property"/>
<dcterms:hasVersion rdf:resource="http://dublincore.org/usage/terms/history/#dateT-001"/>
<rdfs:range rdf:resource="http://www.w3.org/2000/01/rdf-schema#Literal"/>
<rdfs:subPropertyOf rdf:resource="http://purl.org/dc/elements/1.1/date"/>
</rdf:Description>

<rdf:Description rdf:about="&dcterms;type">
<rdfs:label xml:lang="en">Type</rdfs:label>
<rdfs:comment xml:lang="en">The nature or genre of the resource.</rdfs:comment>
<dcterms:description xml:lang="en">Recommended best practice is to use a controlled vocabulary such as the DCMI Type Vocabulary [DCMITYPE]. To describe the file format, physical medium, or dimensions of the resource, use the Format element.</dcterms:description>
<rdf:type rdf:resource="&rdf;Property"/>
<dcterms:hasVersion rdf:resource="http://dublincore.org/usage/terms/history/#typeT-001"/>
<rdfs:range rdf:resource="http://www.w3.org/2000/01/rdf-schema#Class"/>
<rdfs:subPropertyOf rdf:resource="http://purl.org/dc/elements/1.1/type"/>
</rdf:Description>

<rdf:Description rdf:about="&dcterms;format">
<rdfs:label xml:lang="en">Format</rdfs:label>
<rdfs:comment xml:lang="en">The file format, physical medium, or dimensions of the resource.</rdfs:comment>
<dcterms:description xml:lang="en">Examples of dimensions include size and duration. Recommended best practice is to use a controlled vocabulary such as the list of Internet Media Types [MIME].</dcterms:description>
<rdf:type rdf:resource="&rdf;Property"/>
<dcterms:hasVersion rdf:resource="http://dublincore.org/usage/terms/history/#formatT-001"/>
<rdfs:range rdf:resource="&dcterms;MediaTypeOrExtent"/>
<rdfs:subPropertyOf rdf:resource="http://purl.org/dc/elements/1.1/format"/>
</rdf:Description>

<rdf:Description rdf:about="&dcterms;identifier">
<rdfs:label xml:lang="en">Identifier</rdfs:label>
<rdfs:comment xml:lang="en">An unambiguous reference to the resource within a given context.</rdfs:comment>
<dcterms:description xml:lang="en">Recommended best practice is to identify the resource by means of a string conforming to a formal identification system. </dcterms:description>
<rdf:type rdf:resource="&rdf;Property"/>
<dcterms:hasVersion rdf:resource="http://dublincore.org/usage/terms/history/#identifierT-001"/>
<rdfs:range rdf:resource="http://www.w3.org/2000/01/rdf-schema#Literal"/>
<rdfs:subPropertyOf rdf:resource="http://purl.org/dc/elements/1.1/identifier"/>
</rdf:Description>

<rdf:Description rdf:about="&dcterms;source">
<rdfs:label xml:lang="en">Source</rdfs:label>
<rdfs:comment xml:lang="en">A related resource from which the described resource is derived.</rdfs:comment>
<dcterms:description xml:lang="en">The described resource may be derived from the related resource in whole or in part. Recommended best practice is to identify the related resource by means of a string conforming to a formal identification system.</dcterms:description>
<rdf:type rdf:resource="&rdf;Property"/>
<dcterms:hasVersion rdf:resource="http://dublincore.org/usage/terms/history/#sourceT-001"/>
<skos:note xml:lang="en">This term is intended to be used with non-literal values as defined in the DCMI Abstract Model (http://dublincore.org/documents/abstract-model/).  As of December 2007, the DCMI Usage Board is seeking a way to express this intention with a formal range declaration.</skos:note>
<rdfs:subPropertyOf rdf:resource="http://purl.org/dc/elements/1.1/source"/>
<rdfs:subPropertyOf rdf:resource="&dcterms;relation"/>
</rdf:Description>

<rdf:Description rdf:about="&dcterms;language">
<rdfs:label xml:lang="en">Language</rdfs:label>
<rdfs:comment xml:lang="en">A language of the resource.</rdfs:comment>
<dcterms:description xml:lang="en">Recommended best practice is to use a controlled vocabulary such as RFC 4646 [RFC4646].</dcterms:description>
<rdf:type rdf:resource="&rdf;Property"/>
<dcterms:hasVersion rdf:resource="http://dublincore.org/usage/terms/history/#languageT-001"/>
<rdfs:range rdf:resource="&dcterms;LinguisticSystem"/>
<rdfs:subPropertyOf rdf:resource="http://purl.org/dc/elements/1.1/language"/>
</rdf:Description>

<rdf:Description rdf:about="&dcterms;relation">
<rdfs:label xml:lang="en">Relation</rdfs:label>
<rdfs:comment xml:lang="en">A related resource.</rdfs:comment>
<dcterms:description xml:lang="en">Recommended best practice is to identify the related resource by means of a string conforming to a formal identification system. </dcterms:description>
<rdf:type rdf:resource="&rdf;Property"/>
<dcterms:hasVersion rdf:resource="http://dublincore.org/usage/terms/history/#relationT-001"/>
<skos:note xml:lang="en">This term is intended to be used with non-literal values as defined in the DCMI Abstract Model (http://dublincore.org/documents/abstract-model/).  As of December 2007, the DCMI Usage Board is seeking a way to express this intention with a formal range declaration.</skos:note>
<rdfs:subPropertyOf rdf:resource="http://purl.org/dc/elements/1.1/relation"/>
</rdf:Description>

<rdf:Description rdf:about="&dcterms;coverage">
<rdfs:label xml:lang="en">Coverage</rdfs:label>
<rdfs:comment xml:lang="en">The spatial or temporal topic of the resource, the spatial applicability of the resource, or the jurisdiction under which the resource is relevant.</rdfs:comment>
<dcterms:description xml:lang="en">Spatial topic and spatial applicability may be a named place or a location specified by its geographic coordinates. Temporal topic may be a named period, date, or date range. A jurisdiction may be a named administrative entity or a geographic place to which the resource applies. Recommended best practice is to use a controlled vocabulary such as the Thesaurus of Geographic Names [TGN]. Where appropriate, named places or time periods can be used in preference to numeric identifiers such as sets of coordinates or date ranges.</dcterms:description>
<rdf:type rdf:resource="&rdf;Property"/>
<dcterms:hasVersion rdf:resource="http://dublincore.org/usage/terms/history/#coverageT-001"/>
<rdfs:range rdf:resource="&dcterms;LocationPeriodOrJurisdiction"/>
<rdfs:subPropertyOf rdf:resource="http://purl.org/dc/elements/1.1/coverage"/>
</rdf:Description>

<rdf:Description rdf:about="&dcterms;rights">
<rdfs:label xml:lang="en">Rights</rdfs:label>
<rdfs:comment xml:lang="en">Information about rights held in and over the resource.</rdfs:comment>
<dcterms:description xml:lang="en">Typically, rights information includes a statement about various property rights associated with the resource, including intellectual property rights.</dcterms:description>
<rdf:type rdf:resource="&rdf;Property"/>
<dcterms:hasVersion rdf:resource="http://dublincore.org/usage/terms/history/#rightsT-001"/>
<rdfs:range rdf:resource="&dcterms;RightsStatement"/>
<rdfs:subPropertyOf rdf:resource="http://purl.org/dc/elements/1.1/rights"/>
</rdf:Description>

<rdf:Description rdf:about="&dcterms;audience">
<rdfs:label xml:lang="en">Audience</rdfs:label>
<rdfs:comment xml:lang="en">A class of entity for whom the resource is intended or useful.</rdfs:comment>
<dcterms:issued>2001-05-21</dcterms:issued>
<rdf:type rdf:resource="&rdf;Property"/>
<dcterms:hasVersion rdf:resource="http://dublincore.org/usage/terms/history/#audience-003"/>
<rdfs:range rdf:resource="&dcterms;AgentClass"/>
</rdf:Description>

<rdf:Description rdf:about="&dcterms;alternative">
<rdfs:label xml:lang="en">Alternative Title</rdfs:label>
<rdfs:comment xml:lang="en">An alternative name for the resource.</rdfs:comment>
<dcterms:description xml:lang="en">The distinction between titles and alternative titles is application-specific.</dcterms:description>
<dcterms:issued>2000-07-11</dcterms:issued>
<rdf:type rdf:resource="&rdf;Property"/>
<dcterms:hasVersion rdf:resource="http://dublincore.org/usage/terms/history/#alternative-003"/>
<skos:note xml:lang="en">In current practice, this term is used primarily with literal values; however, there are important uses with non-literal values as well.  As of December 2007, the DCMI Usage Board is leaving this range unspecified pending an investigation of options.</skos:note>
<rdfs:subPropertyOf rdf:resource="http://purl.org/dc/elements/1.1/title"/>
<rdfs:subPropertyOf rdf:resource="&dcterms;title"/>
</rdf:Description>

<rdf:Description rdf:about="&dcterms;tableOfContents">
<rdfs:label xml:lang="en">Table Of Contents</rdfs:label>
<rdfs:comment xml:lang="en">A list of subunits of the resource.</rdfs:comment>
<dcterms:issued>2000-07-11</dcterms:issued>
<rdf:type rdf:resource="&rdf;Property"/>
<dcterms:hasVersion rdf:resource="http://dublincore.org/usage/terms/history/#tableOfContents-003"/>
<rdfs:subPropertyOf rdf:resource="http://purl.org/dc/elements/1.1/description"/>
<rdfs:subPropertyOf rdf:resource="&dcterms;description"/>
</rdf:Description>

<rdf:Description rdf:about="&dcterms;abstract">
<rdfs:label xml:lang="en">Abstract</rdfs:label>
<rdfs:comment xml:lang="en">A summary of the resource.</rdfs:comment>
<dcterms:issued>2000-07-11</dcterms:issued>
<rdf:type rdf:resource="&rdf;Property"/>
<dcterms:hasVersion rdf:resource="http://dublincore.org/usage/terms/history/#abstract-003"/>
<rdfs:subPropertyOf rdf:resource="http://purl.org/dc/elements/1.1/description"/>
<rdfs:subPropertyOf rdf:resource="&dcterms;description"/>
</rdf:Description>

<rdf:Description rdf:about="&dcterms;created">
<rdfs:label xml:lang="en">Date Created</rdfs:label>
<rdfs:comment xml:lang="en">Date of creation of the resource.</rdfs:comment>
<dcterms:issued>2000-07-11</dcterms:issued>
<rdf:type rdf:resource="&rdf;Property"/>
<dcterms:hasVersion rdf:resource="http://dublincore.org/usage/terms/history/#created-003"/>
<rdfs:range rdf:resource="http://www.w3.org/2000/01/rdf-schema#Literal"/>
<rdfs:subPropertyOf rdf:resource="http://purl.org/dc/elements/1.1/date"/>
<rdfs:subPropertyOf rdf:resource="&dcterms;date"/>
</rdf:Description>

<rdf:Description rdf:about="&dcterms;valid">
<rdfs:label xml:lang="en">Date Valid</rdfs:label>
<rdfs:comment xml:lang="en">Date (often a range) of validity of a resource.</rdfs:comment>
<dcterms:issued>2000-07-11</dcterms:issued>
<rdf:type rdf:resource="&rdf;Property"/>
<dcterms:hasVersion rdf:resource="http://dublincore.org/usage/terms/history/#valid-003"/>
<rdfs:range rdf:resource="http://www.w3.org/2000/01/rdf-schema#Literal"/>
<rdfs:subPropertyOf rdf:resource="http://purl.org/dc/elements/1.1/date"/>
<rdfs:subPropertyOf rdf:resource="&dcterms;date"/>
</rdf:Description>

<rdf:Description rdf:about="&dcterms;available">
<rdfs:label xml:lang="en">Date Available</rdfs:label>
<rdfs:comment xml:lang="en">Date (often a range) that the resource became or will become available.</rdfs:comment>
<dcterms:issued>2000-07-11</dcterms:issued>
<rdf:type rdf:resource="&rdf;Property"/>
<dcterms:hasVersion rdf:resource="http://dublincore.org/usage/terms/history/#available-003"/>
<rdfs:range rdf:resource="http://www.w3.org/2000/01/rdf-schema#Literal"/>
<rdfs:subPropertyOf rdf:resource="http://purl.org/dc/elements/1.1/date"/>
<rdfs:subPropertyOf rdf:resource="&dcterms;date"/>
</rdf:Description>

<rdf:Description rdf:about="&dcterms;issued">
<rdfs:label xml:lang="en">Date Issued</rdfs:label>
<rdfs:comment xml:lang="en">Date of formal issuance (e.g., publication) of the resource.</rdfs:comment>
<dcterms:issued>2000-07-11</dcterms:issued>
<rdf:type rdf:resource="&rdf;Property"/>
<dcterms:hasVersion rdf:resource="http://dublincore.org/usage/terms/history/#issued-003"/>
<rdfs:range rdf:resource="http://www.w3.org/2000/01/rdf-schema#Literal"/>
<rdfs:subPropertyOf rdf:resource="http://purl.org/dc/elements/1.1/date"/>
<rdfs:subPropertyOf rdf:resource="&dcterms;date"/>
</rdf:Description>

<rdf:Description rdf:about="&dcterms;modified">
<rdfs:label xml:lang="en">Date Modified</rdfs:label>
<rdfs:comment xml:lang="en">Date on which the resource was changed.</rdfs:comment>
<dcterms:issued>2000-07-11</dcterms:issued>
<rdf:type rdf:resource="&rdf;Property"/>
<dcterms:hasVersion rdf:resource="http://dublincore.org/usage/terms/history/#modified-003"/>
<rdfs:range rdf:resource="http://www.w3.org/2000/01/rdf-schema#Literal"/>
<rdfs:subPropertyOf rdf:resource="http://purl.org/dc/elements/1.1/date"/>
<rdfs:subPropertyOf rdf:resource="&dcterms;date"/>
</rdf:Description>

<rdf:Description rdf:about="&dcterms;extent">
<rdfs:label xml:lang="en">Extent</rdfs:label>
<rdfs:comment xml:lang="en">The size or duration of the resource.</rdfs:comment>
<dcterms:issued>2000-07-11</dcterms:issued>
<rdf:type rdf:resource="&rdf;Property"/>
<dcterms:hasVersion rdf:resource="http://dublincore.org/usage/terms/history/#extent-003"/>
<rdfs:range rdf:resource="&dcterms;SizeOrDuration"/>
<rdfs:subPropertyOf rdf:resource="http://purl.org/dc/elements/1.1/format"/>
<rdfs:subPropertyOf rdf:resource="&dcterms;format"/>
</rdf:Description>

<rdf:Description rdf:about="&dcterms;medium">
<rdfs:label xml:lang="en">Medium</rdfs:label>
<rdfs:comment xml:lang="en">The material or physical carrier of the resource.</rdfs:comment>
<dcterms:issued>2000-07-11</dcterms:issued>
<rdf:type rdf:resource="&rdf;Property"/>
<dcterms:hasVersion rdf:resource="http://dublincore.org/usage/terms/history/#medium-003"/>
<rdfs:domain rdf:resource="&dcterms;PhysicalResource"/>
<rdfs:range rdf:resource="&dcterms;PhysicalMedium"/>
<rdfs:subPropertyOf rdf:resource="http://purl.org/dc/elements/1.1/format"/>
<rdfs:subPropertyOf rdf:resource="&dcterms;format"/>
</rdf:Description>

<rdf:Description rdf:about="&dcterms;isVersionOf">
<rdfs:label xml:lang="en">Is Version Of</rdfs:label>
<rdfs:comment xml:lang="en">A related resource of which the described resource is a version, edition, or adaptation.</rdfs:comment>
<dcterms:description xml:lang="en">Changes in version imply substantive changes in content rather than differences in format.</dcterms:description>
<dcterms:issued>2000-07-11</dcterms:issued>
<rdf:type rdf:resource="&rdf;Property"/>
<dcterms:hasVersion rdf:resource="http://dublincore.org/usage/terms/history/#isVersionOf-003"/>
<skos:note xml:lang="en">This term is intended to be used with non-literal values as defined in the DCMI Abstract Model (http://dublincore.org/documents/abstract-model/).  As of December 2007, the DCMI Usage Board is seeking a way to express this intention with a formal range declaration.</skos:note>
<rdfs:subPropertyOf rdf:resource="http://purl.org/dc/elements/1.1/relation"/>
<rdfs:subPropertyOf rdf:resource="&dcterms;relation"/>
</rdf:Description>

<rdf:Description rdf:about="&dcterms;hasVersion">
<rdfs:label xml:lang="en">Has Version</rdfs:label>
<rdfs:comment xml:lang="en">A related resource that is a version, edition, or adaptation of the described resource.</rdfs:comment>
<dcterms:issued>2000-07-11</dcterms:issued>
<rdf:type rdf:resource="&rdf;Property"/>
<dcterms:hasVersion rdf:resource="http://dublincore.org/usage/terms/history/#hasVersion-003"/>
<skos:note xml:lang="en">This term is intended to be used with non-literal values as defined in the DCMI Abstract Model (http://dublincore.org/documents/abstract-model/).  As of December 2007, the DCMI Usage Board is seeking a way to express this intention with a formal range declaration.</skos:note>
<rdfs:subPropertyOf rdf:resource="http://purl.org/dc/elements/1.1/relation"/>
<rdfs:subPropertyOf rdf:resource="&dcterms;relation"/>
</rdf:Description>

<rdf:Description rdf:about="&dcterms;isReplacedBy">
<rdfs:label xml:lang="en">Is Replaced By</rdfs:label>
<rdfs:comment xml:lang="en">A related resource that supplants, displaces, or supersedes the described resource.</rdfs:comment>
<dcterms:issued>2000-07-11</dcterms:issued>
<rdf:type rdf:resource="&rdf;Property"/>
<dcterms:hasVersion rdf:resource="http://dublincore.org/usage/terms/history/#isReplacedBy-003"/>
<skos:note xml:lang="en">This term is intended to be used with non-literal values as defined in the DCMI Abstract Model (http://dublincore.org/documents/abstract-model/).  As of December 2007, the DCMI Usage Board is seeking a way to express this intention with a formal range declaration.</skos:note>
<rdfs:subPropertyOf rdf:resource="http://purl.org/dc/elements/1.1/relation"/>
<rdfs:subPropertyOf rdf:resource="&dcterms;relation"/>
</rdf:Description>

<rdf:Description rdf:about="&dcterms;replaces">
<rdfs:label xml:lang="en">Replaces</rdfs:label>
<rdfs:comment xml:lang="en">A related resource that is supplanted, displaced, or superseded by the described resource.</rdfs:comment>
<dcterms:issued>2000-07-11</dcterms:issued>
<rdf:type rdf:resource="&rdf;Property"/>
<dcterms:hasVersion rdf:resource="http://dublincore.org/usage/terms/history/#replaces-003"/>
<skos:note xml:lang="en">This term is intended to be used with non-literal values as defined in the DCMI Abstract Model (http://dublincore.org/documents/abstract-model/).  As of December 2007, the DCMI Usage Board is seeking a way to express this intention with a formal range declaration.</skos:note>
<rdfs:subPropertyOf rdf:resource="http://purl.org/dc/elements/1.1/relation"/>
<rdfs:subPropertyOf rdf:resource="&dcterms;relation"/>
</rdf:Description>

<rdf:Description rdf:about="&dcterms;isRequiredBy">
<rdfs:label xml:lang="en">Is Required By</rdfs:label>
<rdfs:comment xml:lang="en">A related resource that requires the described resource to support its function, delivery, or coherence.</rdfs:comment>
<dcterms:issued>2000-07-11</dcterms:issued>
<rdf:type rdf:resource="&rdf;Property"/>
<dcterms:hasVersion rdf:resource="http://dublincore.org/usage/terms/history/#isRequiredBy-003"/>
<skos:note xml:lang="en">This term is intended to be used with non-literal values as defined in the DCMI Abstract Model (http://dublincore.org/documents/abstract-model/).  As of December 2007, the DCMI Usage Board is seeking a way to express this intention with a formal range declaration.</skos:note>
<rdfs:subPropertyOf rdf:resource="http://purl.org/dc/elements/1.1/relation"/>
<rdfs:subPropertyOf rdf:resource="&dcterms;relation"/>
</rdf:Description>

<rdf:Description rdf:about="&dcterms;requires">
<rdfs:label xml:lang="en">Requires</rdfs:label>
<rdfs:comment xml:lang="en">A related resource that is required by the described resource to support its function, delivery, or coherence.</rdfs:comment>
<dcterms:issued>2000-07-11</dcterms:issued>
<rdf:type rdf:resource="&rdf;Property"/>
<dcterms:hasVersion rdf:resource="http://dublincore.org/usage/terms/history/#requires-003"/>
<skos:note xml:lang="en">This term is intended to be used with non-literal values as defined in the DCMI Abstract Model (http://dublincore.org/documents/abstract-model/).  As of December 2007, the DCMI Usage Board is seeking a way to express this intention with a formal range declaration.</skos:note>
<rdfs:subPropertyOf rdf:resource="http://purl.org/dc/elements/1.1/relation"/>
<rdfs:subPropertyOf rdf:resource="&dcterms;relation"/>
</rdf:Description>

<rdf:Description rdf:about="&dcterms;isPartOf">
<rdfs:label xml:lang="en">Is Part Of</rdfs:label>
<rdfs:comment xml:lang="en">A related resource in which the described resource is physically or logically included.</rdfs:comment>
<dcterms:issued>2000-07-11</dcterms:issued>
<rdf:type rdf:resource="&rdf;Property"/>
<dcterms:hasVersion rdf:resource="http://dublincore.org/usage/terms/history/#isPartOf-003"/>
<skos:note xml:lang="en">This term is intended to be used with non-literal values as defined in the DCMI Abstract Model (http://dublincore.org/documents/abstract-model/).  As of December 2007, the DCMI Usage Board is seeking a way to express this intention with a formal range declaration.</skos:note>
<rdfs:subPropertyOf rdf:resource="http://purl.org/dc/elements/1.1/relation"/>
<rdfs:subPropertyOf rdf:resource="&dcterms;relation"/>
</rdf:Description>

<rdf:Description rdf:about="&dcterms;hasPart">
<rdfs:label xml:lang="en">Has Part</rdfs:label>
<rdfs:comment xml:lang="en">A related resource that is included either physically or logically in the described resource.</rdfs:comment>
<dcterms:issued>2000-07-11</dcterms:issued>
<rdf:type rdf:resource="&rdf;Property"/>
<dcterms:hasVersion rdf:resource="http://dublincore.org/usage/terms/history/#hasPart-003"/>
<skos:note xml:lang="en">This term is intended to be used with non-literal values as defined in the DCMI Abstract Model (http://dublincore.org/documents/abstract-model/).  As of December 2007, the DCMI Usage Board is seeking a way to express this intention with a formal range declaration.</skos:note>
<rdfs:subPropertyOf rdf:resource="http://purl.org/dc/elements/1.1/relation"/>
<rdfs:subPropertyOf rdf:resource="&dcterms;relation"/>
</rdf:Description>

<rdf:Description rdf:about="&dcterms;isReferencedBy">
<rdfs:label xml:lang="en">Is Referenced By</rdfs:label>
<rdfs:comment xml:lang="en">A related resource that references, cites, or otherwise points to the described resource.</rdfs:comment>
<dcterms:issued>2000-07-11</dcterms:issued>
<rdf:type rdf:resource="&rdf;Property"/>
<dcterms:hasVersion rdf:resource="http://dublincore.org/usage/terms/history/#isReferencedBy-003"/>
<skos:note xml:lang="en">This term is intended to be used with non-literal values as defined in the DCMI Abstract Model (http://dublincore.org/documents/abstract-model/).  As of December 2007, the DCMI Usage Board is seeking a way to express this intention with a formal range declaration.</skos:note>
<rdfs:subPropertyOf rdf:resource="http://purl.org/dc/elements/1.1/relation"/>
<rdfs:subPropertyOf rdf:resource="&dcterms;relation"/>
</rdf:Description>

<rdf:Description rdf:about="&dcterms;references">
<rdfs:label xml:lang="en">References</rdfs:label>
<rdfs:comment xml:lang="en">A related resource that is referenced, cited, or otherwise pointed to by the described resource.</rdfs:comment>
<dcterms:issued>2000-07-11</dcterms:issued>
<rdf:type rdf:resource="&rdf;Property"/>
<dcterms:hasVersion rdf:resource="http://dublincore.org/usage/terms/history/#references-003"/>
<skos:note xml:lang="en">This term is intended to be used with non-literal values as defined in the DCMI Abstract Model (http://dublincore.org/documents/abstract-model/).  As of December 2007, the DCMI Usage Board is seeking a way to express this intention with a formal range declaration.</skos:note>
<rdfs:subPropertyOf rdf:resource="http://purl.org/dc/elements/1.1/relation"/>
<rdfs:subPropertyOf rdf:resource="&dcterms;relation"/>
</rdf:Description>

<rdf:Description rdf:about="&dcterms;isFormatOf">
<rdfs:label xml:lang="en">Is Format Of</rdfs:label>
<rdfs:comment xml:lang="en">A related resource that is substantially the same as the described resource, but in another format.</rdfs:comment>
<dcterms:issued>2000-07-11</dcterms:issued>
<rdf:type rdf:resource="&rdf;Property"/>
<dcterms:hasVersion rdf:resource="http://dublincore.org/usage/terms/history/#isFormatOf-003"/>
<skos:note xml:lang="en">This term is intended to be used with non-literal values as defined in the DCMI Abstract Model (http://dublincore.org/documents/abstract-model/).  As of December 2007, the DCMI Usage Board is seeking a way to express this intention with a formal range declaration.</skos:note>
<rdfs:subPropertyOf rdf:resource="http://purl.org/dc/elements/1.1/relation"/>
<rdfs:subPropertyOf rdf:resource="&dcterms;relation"/>
</rdf:Description>

<rdf:Description rdf:about="&dcterms;hasFormat">
<rdfs:label xml:lang="en">Has Format</rdfs:label>
<rdfs:comment xml:lang="en">A related resource that is substantially the same as the pre-existing described resource, but in another format.</rdfs:comment>
<dcterms:issued>2000-07-11</dcterms:issued>
<rdf:type rdf:resource="&rdf;Property"/>
<dcterms:hasVersion rdf:resource="http://dublincore.org/usage/terms/history/#hasFormat-003"/>
<skos:note xml:lang="en">This term is intended to be used with non-literal values as defined in the DCMI Abstract Model (http://dublincore.org/documents/abstract-model/).  As of December 2007, the DCMI Usage Board is seeking a way to express this intention with a formal range declaration.</skos:note>
<rdfs:subPropertyOf rdf:resource="http://purl.org/dc/elements/1.1/relation"/>
<rdfs:subPropertyOf rdf:resource="&dcterms;relation"/>
</rdf:Description>

<rdf:Description rdf:about="&dcterms;conformsTo">
<rdfs:label xml:lang="en">Conforms To</rdfs:label>
<rdfs:comment xml:lang="en">An established standard to which the described resource conforms.</rdfs:comment>
<dcterms:issued>2001-05-21</dcterms:issued>
<rdf:type rdf:resource="&rdf;Property"/>
<dcterms:hasVersion rdf:resource="http://dublincore.org/usage/terms/history/#conformsTo-003"/>
<rdfs:range rdf:resource="&dcterms;Standard"/>
<rdfs:subPropertyOf rdf:resource="http://purl.org/dc/elements/1.1/relation"/>
<rdfs:subPropertyOf rdf:resource="&dcterms;relation"/>
</rdf:Description>

<rdf:Description rdf:about="&dcterms;spatial">
<rdfs:label xml:lang="en">Spatial Coverage</rdfs:label>
<rdfs:comment xml:lang="en">Spatial characteristics of the resource.</rdfs:comment>
<dcterms:issued>2000-07-11</dcterms:issued>
<rdf:type rdf:resource="&rdf;Property"/>
<dcterms:hasVersion rdf:resource="http://dublincore.org/usage/terms/history/#spatial-003"/>
<rdfs:range rdf:resource="&dcterms;Location"/>
<rdfs:subPropertyOf rdf:resource="http://purl.org/dc/elements/1.1/coverage"/>
<rdfs:subPropertyOf rdf:resource="&dcterms;coverage"/>
</rdf:Description>

<rdf:Description rdf:about="&dcterms;temporal">
<rdfs:label xml:lang="en">Temporal Coverage</rdfs:label>
<rdfs:comment xml:lang="en">Temporal characteristics of the resource.</rdfs:comment>
<dcterms:issued>2000-07-11</dcterms:issued>
<rdf:type rdf:resource="&rdf;Property"/>
<dcterms:hasVersion rdf:resource="http://dublincore.org/usage/terms/history/#temporal-003"/>
<rdfs:range rdf:resource="&dcterms;PeriodOfTime"/>
<rdfs:subPropertyOf rdf:resource="http://purl.org/dc/elements/1.1/coverage"/>
<rdfs:subPropertyOf rdf:resource="&dcterms;coverage"/>
</rdf:Description>

<rdf:Description rdf:about="&dcterms;mediator">
<rdfs:label xml:lang="en">Mediator</rdfs:label>
<rdfs:comment xml:lang="en">An entity that mediates access to the resource and for whom the resource is intended or useful.</rdfs:comment>
<dcterms:description xml:lang="en">In an educational context, a mediator might be a parent, teacher, teaching assistant, or care-giver.</dcterms:description>
<dcterms:issued>2001-05-21</dcterms:issued>
<rdf:type rdf:resource="&rdf;Property"/>
<dcterms:hasVersion rdf:resource="http://dublincore.org/usage/terms/history/#mediator-003"/>
<rdfs:range rdf:resource="&dcterms;AgentClass"/>
<rdfs:subPropertyOf rdf:resource="&dcterms;audience"/>
</rdf:Description>

<rdf:Description rdf:about="&dcterms;dateAccepted">
<rdfs:label xml:lang="en">Date Accepted</rdfs:label>
<rdfs:comment xml:lang="en">Date of acceptance of the resource.</rdfs:comment>
<dcterms:description xml:lang="en">Examples of resources to which a Date Accepted may be relevant are a thesis (accepted by a university department) or an article (accepted by a journal).</dcterms:description>
<dcterms:issued>2002-07-13</dcterms:issued>
<rdf:type rdf:resource="&rdf;Property"/>
<dcterms:hasVersion rdf:resource="http://dublincore.org/usage/terms/history/#dateAccepted-002"/>
<rdfs:range rdf:resource="http://www.w3.org/2000/01/rdf-schema#Literal"/>
<rdfs:subPropertyOf rdf:resource="http://purl.org/dc/elements/1.1/date"/>
<rdfs:subPropertyOf rdf:resource="&dcterms;date"/>
</rdf:Description>

<rdf:Description rdf:about="&dcterms;dateCopyrighted">
<rdfs:label xml:lang="en">Date Copyrighted</rdfs:label>
<rdfs:comment xml:lang="en">Date of copyright.</rdfs:comment>
<dcterms:issued>2002-07-13</dcterms:issued>
<rdf:type rdf:resource="&rdf;Property"/>
<dcterms:hasVersion rdf:resource="http://dublincore.org/usage/terms/history/#dateCopyrighted-002"/>
<rdfs:range rdf:resource="http://www.w3.org/2000/01/rdf-schema#Literal"/>
<rdfs:subPropertyOf rdf:resource="http://purl.org/dc/elements/1.1/date"/>
<rdfs:subPropertyOf rdf:resource="&dcterms;date"/>
</rdf:Description>

<rdf:Description rdf:about="&dcterms;dateSubmitted">
<rdfs:label xml:lang="en">Date Submitted</rdfs:label>
<rdfs:comment xml:lang="en">Date of submission of the resource.</rdfs:comment>
<dcterms:description xml:lang="en">Examples of resources to which a Date Submitted may be relevant are a thesis (submitted to a university department) or an article (submitted to a journal).</dcterms:description>
<dcterms:issued>2002-07-13</dcterms:issued>
<rdf:type rdf:resource="&rdf;Property"/>
<dcterms:hasVersion rdf:resource="http://dublincore.org/usage/terms/history/#dateSubmitted-002"/>
<rdfs:range rdf:resource="http://www.w3.org/2000/01/rdf-schema#Literal"/>
<rdfs:subPropertyOf rdf:resource="http://purl.org/dc/elements/1.1/date"/>
<rdfs:subPropertyOf rdf:resource="&dcterms;date"/>
</rdf:Description>

<rdf:Description rdf:about="&dcterms;educationLevel">
<rdfs:label xml:lang="en">Audience Education Level</rdfs:label>
<rdfs:comment xml:lang="en">A class of entity, defined in terms of progression through an educational or training context, for which the described resource is intended.</rdfs:comment>
<dcterms:issued>2002-07-13</dcterms:issued>
<rdf:type rdf:resource="&rdf;Property"/>
<dcterms:hasVersion rdf:resource="http://dublincore.org/usage/terms/history/#educationLevel-002"/>
<rdfs:range rdf:resource="&dcterms;AgentClass"/>
<rdfs:subPropertyOf rdf:resource="&dcterms;audience"/>
</rdf:Description>

<rdf:Description rdf:about="&dcterms;accessRights">
<rdfs:label xml:lang="en">Access Rights</rdfs:label>
<rdfs:comment xml:lang="en">Information about who can access the resource or an indication of its security status.</rdfs:comment>
<dcterms:description xml:lang="en">Access Rights may include information regarding access or restrictions based on privacy, security, or other policies.</dcterms:description>
<dcterms:issued>2003-02-15</dcterms:issued>
<rdf:type rdf:resource="&rdf;Property"/>
<dcterms:hasVersion rdf:resource="http://dublincore.org/usage/terms/history/#accessRights-002"/>
<rdfs:range rdf:resource="&dcterms;RightsStatement"/>
<rdfs:subPropertyOf rdf:resource="http://purl.org/dc/elements/1.1/rights"/>
<rdfs:subPropertyOf rdf:resource="&dcterms;rights"/>
</rdf:Description>

<rdf:Description rdf:about="&dcterms;bibliographicCitation">
<rdfs:label xml:lang="en">Bibliographic Citation</rdfs:label>
<rdfs:comment xml:lang="en">A bibliographic reference for the resource.</rdfs:comment>
<dcterms:description xml:lang="en">Recommended practice is to include sufficient bibliographic detail to identify the resource as unambiguously as possible.</dcterms:description>
<dcterms:issued>2003-02-15</dcterms:issued>
<rdf:type rdf:resource="&rdf;Property"/>
<dcterms:hasVersion rdf:resource="http://dublincore.org/usage/terms/history/#bibliographicCitation-002"/>
<rdfs:domain rdf:resource="&dcterms;BibliographicResource"/>
<rdfs:range rdf:resource="http://www.w3.org/2000/01/rdf-schema#Literal"/>
<rdfs:subPropertyOf rdf:resource="http://purl.org/dc/elements/1.1/identifier"/>
<rdfs:subPropertyOf rdf:resource="&dcterms;identifier"/>
</rdf:Description>

<rdf:Description rdf:about="&dcterms;license">
<rdfs:label xml:lang="en">License</rdfs:label>
<rdfs:comment xml:lang="en">A legal document giving official permission to do something with the resource.</rdfs:comment>
<dcterms:issued>2004-06-14</dcterms:issued>
<rdf:type rdf:resource="&rdf;Property"/>
<dcterms:hasVersion rdf:resource="http://dublincore.org/usage/terms/history/#license-002"/>
<rdfs:range rdf:resource="&dcterms;LicenseDocument"/>
<rdfs:subPropertyOf rdf:resource="http://purl.org/dc/elements/1.1/rights"/>
<rdfs:subPropertyOf rdf:resource="&dcterms;rights"/>
</rdf:Description>

<rdf:Description rdf:about="&dcterms;rightsHolder">
<rdfs:label xml:lang="en">Rights Holder</rdfs:label>
<rdfs:comment xml:lang="en">A person or organization owning or managing rights over the resource.</rdfs:comment>
<dcterms:issued>2004-06-14</dcterms:issued>
<rdf:type rdf:resource="&rdf;Property"/>
<dcterms:hasVersion rdf:resource="http://dublincore.org/usage/terms/history/#rightsHolder-002"/>
<rdfs:range rdf:resource="&dcterms;Agent"/>
</rdf:Description>

<rdf:Description rdf:about="&dcterms;provenance">
<rdfs:label xml:lang="en">Provenance</rdfs:label>
<rdfs:comment xml:lang="en">A statement of any changes in ownership and custody of the resource since its creation that are significant for its authenticity, integrity, and interpretation.</rdfs:comment>
<dcterms:description xml:lang="en">The statement may include a description of any changes successive custodians made to the resource.</dcterms:description>
<dcterms:issued>2004-09-20</dcterms:issued>
<rdf:type rdf:resource="&rdf;Property"/>
<dcterms:hasVersion rdf:resource="http://dublincore.org/usage/terms/history/#provenance-002"/>
<rdfs:range rdf:resource="&dcterms;ProvenanceStatement"/>
</rdf:Description>

<rdf:Description rdf:about="&dcterms;instructionalMethod">
<rdfs:label xml:lang="en">Instructional Method</rdfs:label>
<rdfs:comment xml:lang="en">A process, used to engender knowledge, attitudes and skills, that the described resource is designed to support.</rdfs:comment>
<dcterms:description xml:lang="en">Instructional Method will typically include ways of presenting instructional materials or conducting instructional activities, patterns of learner-to-learner and learner-to-instructor interactions, and mechanisms by which group and individual levels of learning are measured.  Instructional methods include all aspects of the instruction and learning processes from planning and implementation through evaluation and feedback.</dcterms:description>
<dcterms:issued>2005-06-13</dcterms:issued>
<rdf:type rdf:resource="&rdf;Property"/>
<dcterms:hasVersion rdf:resource="http://dublincore.org/usage/terms/history/#instructionalMethod-002"/>
<rdfs:range rdf:resource="&dcterms;MethodOfInstruction"/>
</rdf:Description>

<rdf:Description rdf:about="&dcterms;accrualMethod">
<rdfs:label xml:lang="en">Accrual Method</rdfs:label>
<rdfs:comment xml:lang="en">The method by which items are added to a collection.</rdfs:comment>
<dcterms:issued>2005-06-13</dcterms:issued>
<rdf:type rdf:resource="&rdf;Property"/>
<dcterms:hasVersion rdf:resource="http://dublincore.org/usage/terms/history/#accrualMethod-002"/>
<rdfs:domain rdf:resource="&dcterms;Collection"/>
<rdfs:range rdf:resource="&dcterms;MethodOfAccrual"/>
</rdf:Description>

<rdf:Description rdf:about="&dcterms;accrualPeriodicity">
<rdfs:label xml:lang="en">Accrual Periodicity</rdfs:label>
<rdfs:comment xml:lang="en">The frequency with which items are added to a collection.</rdfs:comment>
<dcterms:issued>2005-06-13</dcterms:issued>
<rdf:type rdf:resource="&rdf;Property"/>
<dcterms:hasVersion rdf:resource="http://dublincore.org/usage/terms/history/#accrualPeriodicity-002"/>
<rdfs:domain rdf:resource="&dcterms;Collection"/>
<rdfs:range rdf:resource="&dcterms;Frequency"/>
</rdf:Description>

<rdf:Description rdf:about="&dcterms;accrualPolicy">
<rdfs:label xml:lang="en">Accrual Policy</rdfs:label>
<rdfs:comment xml:lang="en">The policy governing the addition of items to a collection.</rdfs:comment>
<dcterms:issued>2005-06-13</dcterms:issued>
<rdf:type rdf:resource="&rdf;Property"/>
<dcterms:hasVersion rdf:resource="http://dublincore.org/usage/terms/history/#accrualPolicy-002"/>
<rdfs:domain rdf:resource="&dcterms;Collection"/>
<rdfs:range rdf:resource="&dcterms;Policy"/>
</rdf:Description>

<rdf:Description rdf:about="&dcterms;Agent">
<rdfs:label xml:lang="en">Agent</rdfs:label>
<rdfs:comment xml:lang="en">A resource that acts or has the power to act.</rdfs:comment>
<dcterms:description xml:lang="en">Examples of Agent include person, organization, and software agent.</dcterms:description>

<dcterms:hasVersion rdf:resource="http://dublincore.org/usage/terms/history/#Agent-001"/>
</rdf:Description>

<rdf:Description rdf:about="&dcterms;AgentClass">
<rdfs:label xml:lang="en">Agent Class</rdfs:label>
<rdfs:comment xml:lang="en">A group of agents.</rdfs:comment>
<dcterms:description xml:lang="en">Examples of Agent Class include groups seen as classes, such as students, women, charities, lecturers.</dcterms:description>

<dcterms:hasVersion rdf:resource="http://dublincore.org/usage/terms/history/#AgentClass-001"/>
</rdf:Description>

<rdf:Description rdf:about="&dcterms;BibliographicResource">
<rdfs:label xml:lang="en">Bibliographic Resource</rdfs:label>
<rdfs:comment xml:lang="en">A book, article, or other documentary resource.</rdfs:comment>

<dcterms:hasVersion rdf:resource="http://dublincore.org/usage/terms/history/#BibliographicResource-001"/>
</rdf:Description>

<rdf:Description rdf:about="&dcterms;FileFormat">
<rdfs:label xml:lang="en">File Format</rdfs:label>
<rdfs:comment xml:lang="en">A digital resource format.</rdfs:comment>
<dcterms:description xml:lang="en">Examples include the formats defined by the list of Internet Media Types.</dcterms:description>

<dcterms:hasVersion rdf:resource="http://dublincore.org/usage/terms/history/#FileFormat-001"/>
</rdf:Description>

<rdf:Description rdf:about="&dcterms;Frequency">
<rdfs:label xml:lang="en">Frequency</rdfs:label>
<rdfs:comment xml:lang="en">A rate at which something recurs.</rdfs:comment>

<dcterms:hasVersion rdf:resource="http://dublincore.org/usage/terms/history/#Frequency-001"/>
</rdf:Description>

<rdf:Description rdf:about="&dcterms;Jurisdiction">
<rdfs:label xml:lang="en">Jurisdiction</rdfs:label>
<rdfs:comment xml:lang="en">The extent or range of judicial, law enforcement, or other authority.</rdfs:comment>

<dcterms:hasVersion rdf:resource="http://dublincore.org/usage/terms/history/#Jurisdiction-001"/>
</rdf:Description>

<rdf:Description rdf:about="&dcterms;LicenseDocument">
<rdfs:label xml:lang="en">License Document</rdfs:label>
<rdfs:comment xml:lang="en">A legal document giving official permission to do something with a Resource.</rdfs:comment>

<dcterms:hasVersion rdf:resource="http://dublincore.org/usage/terms/history/#LicenseDocument-001"/>
</rdf:Description>

<rdf:Description rdf:about="&dcterms;LinguisticSystem">
<rdfs:label xml:lang="en">Linguistic System</rdfs:label>
<rdfs:comment xml:lang="en">A system of signs, symbols, sounds, gestures, or rules used in communication.</rdfs:comment>
<dcterms:description xml:lang="en">Examples include written, spoken, sign, and computer languages.</dcterms:description>

<dcterms:hasVersion rdf:resource="http://dublincore.org/usage/terms/history/#LinguisticSystem-001"/>
</rdf:Description>

<rdf:Description rdf:about="&dcterms;Location">
<rdfs:label xml:lang="en">Location</rdfs:label>
<rdfs:comment xml:lang="en">A spatial region or named place.</rdfs:comment>

<dcterms:hasVersion rdf:resource="http://dublincore.org/usage/terms/history/#Location-001"/>
</rdf:Description>

<rdf:Description rdf:about="&dcterms;LocationPeriodOrJurisdiction">
<rdfs:label xml:lang="en">Location, Period, or Jurisdiction</rdfs:label>
<rdfs:comment xml:lang="en">A location, period of time, or jurisdiction.</rdfs:comment>

<dcterms:hasVersion rdf:resource="http://dublincore.org/usage/terms/history/#LocationPeriodOrJurisdiction-001"/>
</rdf:Description>

<rdf:Description rdf:about="&dcterms;MediaType">
<rdfs:label xml:lang="en">Media Type</rdfs:label>
<rdfs:comment xml:lang="en">A file format or physical medium.</rdfs:comment>

<dcterms:hasVersion rdf:resource="http://dublincore.org/usage/terms/history/#MediaType-001"/>
</rdf:Description>

<rdf:Description rdf:about="&dcterms;MediaTypeOrExtent">
<rdfs:label xml:lang="en">Media Type or Extent</rdfs:label>
<rdfs:comment xml:lang="en">A media type or extent.</rdfs:comment>

<dcterms:hasVersion rdf:resource="http://dublincore.org/usage/terms/history/#MediaTypeOrExtent-001"/>
</rdf:Description>

<rdf:Description rdf:about="&dcterms;MethodOfInstruction">
<rdfs:label xml:lang="en">Method of Instruction</rdfs:label>
<rdfs:comment xml:lang="en">A process that is used to engender knowledge, attitudes, and skills.</rdfs:comment>

<dcterms:hasVersion rdf:resource="http://dublincore.org/usage/terms/history/#MethodOfInstruction-001"/>
</rdf:Description>

<rdf:Description rdf:about="&dcterms;MethodOfAccrual">
<rdfs:label xml:lang="en">Method of Accrual</rdfs:label>
<rdfs:comment xml:lang="en">A method by which resources are added to a collection.</rdfs:comment>

<dcterms:hasVersion rdf:resource="http://dublincore.org/usage/terms/history/#MethodOfAccrual-001"/>
</rdf:Description>

<rdf:Description rdf:about="&dcterms;PeriodOfTime">
<rdfs:label xml:lang="en">Period of Time</rdfs:label>
<rdfs:comment xml:lang="en">An interval of time that is named or defined by its start and end dates.</rdfs:comment>

<dcterms:hasVersion rdf:resource="http://dublincore.org/usage/terms/history/#PeriodOfTime-001"/>
</rdf:Description>

<rdf:Description rdf:about="&dcterms;PhysicalMedium">
<rdfs:label xml:lang="en">Physical Medium</rdfs:label>
<rdfs:comment xml:lang="en">A physical material or carrier.</rdfs:comment>
<dcterms:description xml:lang="en">Examples include paper, canvas, or DVD.</dcterms:description>

<dcterms:hasVersion rdf:resource="http://dublincore.org/usage/terms/history/#PhysicalMedium-001"/>
</rdf:Description>

<rdf:Description rdf:about="&dcterms;PhysicalResource">
<rdfs:label xml:lang="en">Physical Resource</rdfs:label>
<rdfs:comment xml:lang="en">A material thing.</rdfs:comment>

<dcterms:hasVersion rdf:resource="http://dublincore.org/usage/terms/history/#PhysicalResource-001"/>
</rdf:Description>

<rdf:Description rdf:about="&dcterms;Policy">
<rdfs:label xml:lang="en">Policy</rdfs:label>
<rdfs:comment xml:lang="en">A plan or course of action by an authority, intended to influence and determine decisions, actions, and other matters.</rdfs:comment>

<dcterms:hasVersion rdf:resource="http://dublincore.org/usage/terms/history/#Policy-001"/>
</rdf:Description>

<rdf:Description rdf:about="&dcterms;ProvenanceStatement">
<rdfs:label xml:lang="en">Provenance Statement</rdfs:label>
<rdfs:comment xml:lang="en">A statement of any changes in ownership and custody of a resource since its creation that are significant for its authenticity, integrity, and interpretation.</rdfs:comment>

<dcterms:hasVersion rdf:resource="http://dublincore.org/usage/terms/history/#ProvenanceStatement-001"/>
</rdf:Description>

<rdf:Description rdf:about="&dcterms;RightsStatement">
<rdfs:label xml:lang="en">Rights Statement</rdfs:label>
<rdfs:comment xml:lang="en">A statement about the intellectual property rights (IPR) held in or over a Resource, a legal document giving official permission to do something with a resource, or a statement about access rights.</rdfs:comment>

<dcterms:hasVersion rdf:resource="http://dublincore.org/usage/terms/history/#RightsStatement-001"/>
</rdf:Description>

<rdf:Description rdf:about="&dcterms;SizeOrDuration">
<rdfs:label xml:lang="en">Size or Duration</rdfs:label>
<rdfs:comment xml:lang="en">A dimension or extent, or a time taken to play or execute.</rdfs:comment>
<dcterms:description xml:lang="en">Examples include a number of pages, a specification of length, width, and breadth, or a period in hours, minutes, and seconds.</dcterms:description>

<dcterms:hasVersion rdf:resource="http://dublincore.org/usage/terms/history/#SizeOrDuration-001"/>
</rdf:Description>

<rdf:Description rdf:about="&dcterms;Standard">
<rdfs:label xml:lang="en">Standard</rdfs:label>
<rdfs:comment xml:lang="en">A basis for comparison; a reference point against which other things can be evaluated.</rdfs:comment>

<dcterms:hasVersion rdf:resource="http://dublincore.org/usage/terms/history/#Standard-001"/>
</rdf:Description>

<rdf:Description rdf:about="&dcterms;ISO639-2">
<rdfs:label xml:lang="en">ISO 639-2</rdfs:label>
<rdfs:comment xml:lang="en">The three-letter alphabetic codes listed in ISO639-2 for the representation of names of languages.</rdfs:comment>
<dcterms:issued>2000-07-11</dcterms:issued>
<rdf:type rdf:resource="http://www.w3.org/2000/01/rdf-schema#Datatype"/>
<dcterms:hasVersion rdf:resource="http://dublincore.org/usage/terms/history/#ISO639-2-003"/>
<rdfs:seeAlso rdf:resource="http://lcweb.loc.gov/standards/iso639-2/langhome.html"/>
</rdf:Description>

<rdf:Description rdf:about="&dcterms;RFC1766">
<rdfs:label xml:lang="en">RFC 1766</rdfs:label>
<rdfs:comment xml:lang="en">The set of tags, constructed according to RFC 1766, for the identification of languages.</rdfs:comment>
<dcterms:issued>2000-07-11</dcterms:issued>
<rdf:type rdf:resource="http://www.w3.org/2000/01/rdf-schema#Datatype"/>
<dcterms:hasVersion rdf:resource="http://dublincore.org/usage/terms/history/#RFC1766-003"/>
<rdfs:seeAlso rdf:resource="http://www.ietf.org/rfc/rfc1766.txt"/>
</rdf:Description>

<rdf:Description rdf:about="&dcterms;URI">
<rdfs:label xml:lang="en">URI</rdfs:label>
<rdfs:comment xml:lang="en">The set of identifiers constructed according to the generic syntax for Uniform Resource Identifiers as specified by the Internet Engineering Task Force.</rdfs:comment>
<dcterms:issued>2000-07-11</dcterms:issued>
<rdf:type rdf:resource="http://www.w3.org/2000/01/rdf-schema#Datatype"/>
<dcterms:hasVersion rdf:resource="http://dublincore.org/usage/terms/history/#URI-003"/>
<rdfs:seeAlso rdf:resource="http://www.ietf.org/rfc/rfc3986.txt"/>
</rdf:Description>

<rdf:Description rdf:about="&dcterms;Point">
<rdfs:label xml:lang="en">DCMI Point</rdfs:label>
<rdfs:comment xml:lang="en">The set of points in space defined by their geographic coordinates according to the DCMI Point Encoding Scheme.</rdfs:comment>
<dcterms:issued>2000-07-11</dcterms:issued>
<rdf:type rdf:resource="http://www.w3.org/2000/01/rdf-schema#Datatype"/>
<dcterms:hasVersion rdf:resource="http://dublincore.org/usage/terms/history/#Point-003"/>
<rdfs:seeAlso rdf:resource="http://dublincore.org/documents/dcmi-point/"/>
</rdf:Description>

<rdf:Description rdf:about="&dcterms;ISO3166">
<rdfs:label xml:lang="en">ISO 3166</rdfs:label>
<rdfs:comment xml:lang="en">The set of codes listed in ISO 3166-1 for the representation of names of countries.</rdfs:comment>
<dcterms:issued>2000-07-11</dcterms:issued>
<rdf:type rdf:resource="http://www.w3.org/2000/01/rdf-schema#Datatype"/>
<dcterms:hasVersion rdf:resource="http://dublincore.org/usage/terms/history/#ISO3166-004"/>
<rdfs:seeAlso rdf:resource="http://www.iso.org/iso/en/prods-services/iso3166ma/02iso-3166-code-lists/list-en1.html"/>
</rdf:Description>

<rdf:Description rdf:about="&dcterms;Box">
<rdfs:label xml:lang="en">DCMI Box</rdfs:label>
<rdfs:comment xml:lang="en">The set of regions in space defined by their geographic coordinates according to the DCMI Box Encoding Scheme.</rdfs:comment>
<dcterms:issued>2000-07-11</dcterms:issued>
<rdf:type rdf:resource="http://www.w3.org/2000/01/rdf-schema#Datatype"/>
<dcterms:hasVersion rdf:resource="http://dublincore.org/usage/terms/history/#Box-003"/>
<rdfs:seeAlso rdf:resource="http://dublincore.org/documents/dcmi-box/"/>
</rdf:Description>

<rdf:Description rdf:about="&dcterms;Period">
<rdfs:label xml:lang="en">DCMI Period</rdfs:label>
<rdfs:comment xml:lang="en">The set of time intervals defined by their limits according to the DCMI Period Encoding Scheme.</rdfs:comment>
<dcterms:issued>2000-07-11</dcterms:issued>
<rdf:type rdf:resource="http://www.w3.org/2000/01/rdf-schema#Datatype"/>
<dcterms:hasVersion rdf:resource="http://dublincore.org/usage/terms/history/#Period-003"/>
<rdfs:seeAlso rdf:resource="http://dublincore.org/documents/dcmi-period/"/>
</rdf:Description>

<rdf:Description rdf:about="&dcterms;W3CDTF">
<rdfs:label xml:lang="en">W3C-DTF</rdfs:label>
<rdfs:comment xml:lang="en">The set of dates and times constructed according to the W3C Date and Time Formats Specification.</rdfs:comment>
<dcterms:issued>2000-07-11</dcterms:issued>
<rdf:type rdf:resource="http://www.w3.org/2000/01/rdf-schema#Datatype"/>
<dcterms:hasVersion rdf:resource="http://dublincore.org/usage/terms/history/#W3CDTF-003"/>
<rdfs:seeAlso rdf:resource="http://www.w3.org/TR/NOTE-datetime"/>
</rdf:Description>

<rdf:Description rdf:about="&dcterms;RFC3066">
<rdfs:label xml:lang="en">RFC 3066</rdfs:label>
<rdfs:comment xml:lang="en">The set of tags constructed according to RFC 3066 for the identification of languages.</rdfs:comment>
<dcterms:description xml:lang="en">RFC 3066 has been obsoleted by RFC 4646.</dcterms:description>
<dcterms:issued>2002-07-13</dcterms:issued>
<rdf:type rdf:resource="http://www.w3.org/2000/01/rdf-schema#Datatype"/>
<dcterms:hasVersion rdf:resource="http://dublincore.org/usage/terms/history/#RFC3066-002"/>
<rdfs:seeAlso rdf:resource="http://www.ietf.org/rfc/rfc3066.txt"/>
</rdf:Description>

<rdf:Description rdf:about="&dcterms;RFC4646">
<rdfs:label xml:lang="en">RFC 4646</rdfs:label>
<rdfs:comment xml:lang="en">The set of tags constructed according to RFC 4646 for the identification of languages.</rdfs:comment>
<dcterms:description xml:lang="en">RFC 4646 obsoletes RFC 3066.</dcterms:description>
<rdf:type rdf:resource="http://www.w3.org/2000/01/rdf-schema#Datatype"/>
<dcterms:hasVersion rdf:resource="http://dublincore.org/usage/terms/history/#RFC4646-001"/>
<rdfs:seeAlso rdf:resource="http://www.ietf.org/rfc/rfc4646.txt"/>
</rdf:Description>

<rdf:Description rdf:about="&dcterms;ISO639-3">
<rdfs:label xml:lang="en">ISO 639-3</rdfs:label>
<rdfs:comment xml:lang="en">The set of three-letter codes listed in ISO 639-3 for the representation of names of languages.</rdfs:comment>
<rdf:type rdf:resource="http://www.w3.org/2000/01/rdf-schema#Datatype"/>
<dcterms:hasVersion rdf:resource="http://dublincore.org/usage/terms/history/#ISO639-3-001"/>
<rdfs:seeAlso rdf:resource="http://www.sil.org/iso639-3/"/>
</rdf:Description>

<!--
<rdf:Description rdf:about="&dcterms;LCSH">
<rdfs:label xml:lang="en">LCSH</rdfs:label>
<rdfs:comment xml:lang="en">The set of labeled concepts specified by the Library of Congress Subject Headings.</rdfs:comment>
<dcterms:issued>2000-07-11</dcterms:issued>
<rdf:type rdf:resource="http://purl.org/dc/dcam/VocabularyEncodingScheme"/>
<dcterms:hasVersion rdf:resource="http://dublincore.org/usage/terms/history/#LCSH-003"/>
</rdf:Description>

<rdf:Description rdf:about="&dcterms;MESH">
<rdfs:label xml:lang="en">MeSH</rdfs:label>
<rdfs:comment xml:lang="en">The set of labeled concepts specified by the Medical Subject Headings.</rdfs:comment>
<dcterms:issued>2000-07-11</dcterms:issued>
<rdf:type rdf:resource="http://purl.org/dc/dcam/VocabularyEncodingScheme"/>
<dcterms:hasVersion rdf:resource="http://dublincore.org/usage/terms/history/#MESH-003"/>
<rdfs:seeAlso rdf:resource="http://www.nlm.nih.gov/mesh/meshhome.html"/>
</rdf:Description>

<rdf:Description rdf:about="&dcterms;DDC">
<rdfs:label xml:lang="en">DDC</rdfs:label>
<rdfs:comment xml:lang="en">The set of conceptual resources specified by the Dewey Decimal Classification.</rdfs:comment>
<dcterms:issued>2000-07-11</dcterms:issued>
<rdf:type rdf:resource="http://purl.org/dc/dcam/VocabularyEncodingScheme"/>
<dcterms:hasVersion rdf:resource="http://dublincore.org/usage/terms/history/#DDC-003"/>
<rdfs:seeAlso rdf:resource="http://www.oclc.org/dewey/"/>
</rdf:Description>

<rdf:Description rdf:about="&dcterms;LCC">
<rdfs:label xml:lang="en">LCC</rdfs:label>
<rdfs:comment xml:lang="en">The set of conceptual resources specified by the Library of Congress Classification.</rdfs:comment>
<dcterms:issued>2000-07-11</dcterms:issued>
<rdf:type rdf:resource="http://purl.org/dc/dcam/VocabularyEncodingScheme"/>
<dcterms:hasVersion rdf:resource="http://dublincore.org/usage/terms/history/#LCC-003"/>
<rdfs:seeAlso rdf:resource="http://lcweb.loc.gov/catdir/cpso/lcco/lcco.html"/>
</rdf:Description>

<rdf:Description rdf:about="&dcterms;UDC">
<rdfs:label xml:lang="en">UDC</rdfs:label>
<rdfs:comment xml:lang="en">The set of conceptual resources specified by the Universal Decimal Classification.</rdfs:comment>
<dcterms:issued>2000-07-11</dcterms:issued>
<rdf:type rdf:resource="http://purl.org/dc/dcam/VocabularyEncodingScheme"/>
<dcterms:hasVersion rdf:resource="http://dublincore.org/usage/terms/history/#UDC-003"/>
<rdfs:seeAlso rdf:resource="http://www.udcc.org/"/>
</rdf:Description>

<rdf:Description rdf:about="&dcterms;DCMIType">
<rdfs:label xml:lang="en">DCMI Type Vocabulary</rdfs:label>
<rdfs:comment xml:lang="en">The set of classes specified by the DCMI Type Vocabulary, used to categorize the nature or genre of the resource.</rdfs:comment>
<dcterms:issued>2000-07-11</dcterms:issued>
<rdf:type rdf:resource="http://purl.org/dc/dcam/VocabularyEncodingScheme"/>
<dcterms:hasVersion rdf:resource="http://dublincore.org/usage/terms/history/#DCMIType-003"/>
<rdfs:seeAlso rdf:resource="http://dublincore.org/documents/dcmi-type-vocabulary/"/>
</rdf:Description>

<rdf:Description rdf:about="&dcterms;IMT">
<rdfs:label xml:lang="en">IMT</rdfs:label>
<rdfs:comment xml:lang="en">The set of media types specified by the Internet Assigned Numbers Authority.</rdfs:comment>
<dcterms:issued>2000-07-11</dcterms:issued>
<rdf:type rdf:resource="http://purl.org/dc/dcam/VocabularyEncodingScheme"/>
<dcterms:hasVersion rdf:resource="http://dublincore.org/usage/terms/history/#IMT-004"/>
<rdfs:seeAlso rdf:resource="http://www.iana.org/assignments/media-types/"/>
</rdf:Description>

<rdf:Description rdf:about="&dcterms;TGN">
<rdfs:label xml:lang="en">TGN</rdfs:label>
<rdfs:comment xml:lang="en">The set of places specified by the Getty Thesaurus of Geographic Names.</rdfs:comment>
<dcterms:issued>2000-07-11</dcterms:issued>
<rdf:type rdf:resource="http://purl.org/dc/dcam/VocabularyEncodingScheme"/>
<dcterms:hasVersion rdf:resource="http://dublincore.org/usage/terms/history/#TGN-003"/>
<rdfs:seeAlso rdf:resource="http://www.getty.edu/research/tools/vocabulary/tgn/index.html"/>
</rdf:Description>

<rdf:Description rdf:about="&dcterms;NLM">
<rdfs:label xml:lang="en">NLM</rdfs:label>
<rdfs:comment xml:lang="en">The set of conceptual resources specified by the National Library of Medicine Classification.</rdfs:comment>
<dcterms:issued>2005-06-13</dcterms:issued>
<rdf:type rdf:resource="http://purl.org/dc/dcam/VocabularyEncodingScheme"/>
<dcterms:hasVersion rdf:resource="http://dublincore.org/usage/terms/history/#NLM-002"/>
<rdfs:seeAlso rdf:resource="http://wwwcf.nlm.nih.gov/class/"/>
</rdf:Description>
-->

<!-- SKOS -->



  <rdf:Description rdf:about="&skos;Concept">
    <rdfs:label xml:lang="en">Concept</rdfs:label>
    <skos:definition xml:lang="en">An idea or notion; a unit of thought.</skos:definition>
    <!-- S1 -->
    
  </rdf:Description>

  <rdf:Description rdf:about="&skos;ConceptScheme">
    <rdfs:label xml:lang="en">Concept Scheme</rdfs:label>
    <skos:definition xml:lang="en">A set of concepts, optionally including statements about semantic relationships between those concepts.</skos:definition>
    <skos:scopeNote xml:lang="en">A concept scheme may be defined to include concepts from different sources.</skos:scopeNote>
    <skos:example xml:lang="en">Thesauri, classification schemes, subject heading lists, taxonomies, 'folksonomies', and other types of controlled vocabulary are all examples of concept schemes. Concept schemes are also embedded in glossaries and terminologies.</skos:example>
    <!-- S2 -->
    
    <!-- S9 -->
    <owl:disjointWith rdf:resource="&skos;Concept"/>
  </rdf:Description>

  <rdf:Description rdf:about="&skos;Collection">

    <rdfs:label xml:lang="en">Collection</rdfs:label>
    <skos:definition xml:lang="en">A meaningful collection of concepts.</skos:definition>
    <skos:scopeNote xml:lang="en">Labelled collections can be used where you would like a set of concepts to be displayed under a 'node label' in the hierarchy.</skos:scopeNote>
    <!-- S28 -->
    
    <!-- S37 -->
    <owl:disjointWith rdf:resource="&skos;Concept"/>
    <!-- S37 -->
    <owl:disjointWith rdf:resource="&skos;ConceptScheme"/>
  </rdf:Description>

  <rdf:Description rdf:about="&skos;OrderedCollection">
    <rdfs:label xml:lang="en">Ordered Collection</rdfs:label>
    <skos:definition xml:lang="en">An ordered collection of concepts, where both the grouping and the ordering are meaningful.</skos:definition>
    <skos:scopeNote xml:lang="en">Ordered collections can be used where you would like a set of concepts to be displayed in a specific order, and optionally under a 'node label'.</skos:scopeNote>
    <!-- S28 -->
    
    <!-- S29 -->
  </rdf:Description>

  <rdf:Description rdf:about="&skos;inScheme">
    <rdfs:label xml:lang="en">is in scheme</rdfs:label>
    <skos:definition xml:lang="en">Relates a resource (for example a concept) to a concept scheme in which it is included.</skos:definition>
    <skos:scopeNote xml:lang="en">A concept may be a member of more than one concept scheme.</skos:scopeNote>
    <!-- S3 -->
    <rdf:type rdf:resource="&owl;ObjectProperty"/>
    <!-- S4 -->
    <rdfs:range rdf:resource="&skos;ConceptScheme"/>
    <!-- For non-OWL aware applications -->
    <rdf:type rdf:resource="http://www.w3.org/1999/02/22-rdf-syntax-ns#Property"/>
  </rdf:Description>

  <rdf:Description rdf:about="&skos;hasTopConcept">
    <rdfs:label xml:lang="en">has top concept</rdfs:label>
    <skos:definition xml:lang="en">Relates, by convention, a concept scheme to a concept which is topmost in the broader/narrower concept hierarchies for that scheme, providing an entry point to these hierarchies.</skos:definition>
    <!-- S3 -->
    <rdf:type rdf:resource="&owl;ObjectProperty"/>
    <!-- S5 -->
    <rdfs:domain rdf:resource="&skos;ConceptScheme"/>
    <!-- S6 -->
    <rdfs:range rdf:resource="&skos;Concept"/>
    <!-- S8 -->
    <owl:inverseOf rdf:resource="&skos;topConceptOf"/>
    <!-- For non-OWL aware applications -->
    <rdf:type rdf:resource="http://www.w3.org/1999/02/22-rdf-syntax-ns#Property"/>
  </rdf:Description>

  <rdf:Description rdf:about="&skos;topConceptOf">
    <rdfs:label xml:lang="en">is top concept in scheme</rdfs:label>
    <skos:definition xml:lang="en">Relates a concept to the concept scheme that it is a top level concept of.</skos:definition>
    <!-- S3 -->
    <rdf:type rdf:resource="&owl;ObjectProperty"/>
    <!-- S7 -->
    <rdfs:subPropertyOf rdf:resource="&skos;inScheme"/>
    <!-- S8 -->
    <owl:inverseOf rdf:resource="&skos;hasTopConcept"/>
    <!-- For non-OWL aware applications -->
    <rdf:type rdf:resource="http://www.w3.org/1999/02/22-rdf-syntax-ns#Property"/>
    <rdfs:domain rdf:resource="&skos;Concept"/>
    <rdfs:range rdf:resource="&skos;ConceptScheme"/> 
  </rdf:Description>

  <rdf:Description rdf:about="&skos;prefLabel">
    <rdfs:label xml:lang="en">preferred label</rdfs:label>
    <skos:definition xml:lang="en">The preferred lexical label for a resource, in a given language.</skos:definition>
    <!-- S10 -->
    <rdf:type rdf:resource="&owl;AnnotationProperty"/>
    <!-- S11 -->
    <rdfs:subPropertyOf rdf:resource="http://www.w3.org/2000/01/rdf-schema#label"/>
    <!-- S14 (not formally stated) -->
    <rdfs:comment xml:lang="en">A resource has no more than one value of skos:prefLabel per language tag.</rdfs:comment>
    <!-- S12 (not formally stated) -->
    <rdfs:comment xml:lang="en">The range of skos:prefLabel is the class of RDF plain literals.</rdfs:comment>
    <!-- S13 (not formally stated) -->
    <rdfs:comment xml:lang="en">skos:prefLabel, skos:altLabel and skos:hiddenLabel are pairwise
      disjoint properties.</rdfs:comment>
    <!-- For non-OWL aware applications -->
    <rdf:type rdf:resource="http://www.w3.org/1999/02/22-rdf-syntax-ns#Property"/>
  </rdf:Description>

  <rdf:Description rdf:about="&skos;altLabel">
    <rdfs:label xml:lang="en">alternative label</rdfs:label>
    <skos:definition xml:lang="en">An alternative lexical label for a resource.</skos:definition>
    <skos:example xml:lang="en">Acronyms, abbreviations, spelling variants, and irregular plural/singular forms may be included among the alternative labels for a concept. Mis-spelled terms are normally included as hidden labels (see skos:hiddenLabel).</skos:example>
    <!-- S10 -->
    <rdf:type rdf:resource="&owl;AnnotationProperty"/>
    <!-- S11 -->
    <rdfs:subPropertyOf rdf:resource="http://www.w3.org/2000/01/rdf-schema#label"/>
    <!-- S12 (not formally stated) -->
    <rdfs:comment xml:lang="en">The range of skos:altLabel is the class of RDF plain literals.</rdfs:comment>
    <!-- S13 (not formally stated) -->
    <rdfs:comment xml:lang="en">skos:prefLabel, skos:altLabel and skos:hiddenLabel are pairwise disjoint properties.</rdfs:comment>
    <!-- For non-OWL aware applications -->
    <rdf:type rdf:resource="http://www.w3.org/1999/02/22-rdf-syntax-ns#Property"/>
  </rdf:Description>

  <rdf:Description rdf:about="&skos;hiddenLabel">
    <rdfs:label xml:lang="en">hidden label</rdfs:label>
    <skos:definition xml:lang="en">A lexical label for a resource that should be hidden when generating visual displays of the resource, but should still be accessible to free text search operations.</skos:definition>
    <!-- S10 -->
    <rdf:type rdf:resource="&owl;AnnotationProperty"/>
    <!-- S11 -->
    <rdfs:subPropertyOf rdf:resource="http://www.w3.org/2000/01/rdf-schema#label"/>
    <!-- S12 (not formally stated) -->
    <rdfs:comment xml:lang="en">The range of skos:hiddenLabel is the class of RDF plain literals.</rdfs:comment>
    <!-- S13 (not formally stated) -->
    <rdfs:comment xml:lang="en">skos:prefLabel, skos:altLabel and skos:hiddenLabel are pairwise disjoint properties.</rdfs:comment>
    <!-- For non-OWL aware applications -->
    <rdf:type rdf:resource="http://www.w3.org/1999/02/22-rdf-syntax-ns#Property"/>
  </rdf:Description>

  <rdf:Description rdf:about="&skos;notation">
    <rdfs:label xml:lang="en">notation</rdfs:label>
    <skos:definition xml:lang="en">A notation, also known as classification code, is a string of characters such as "T58.5" or "303.4833" used to uniquely identify a concept within the scope of a given concept scheme.</skos:definition>
    <skos:scopeNote xml:lang="en">By convention, skos:notation is used with a typed literal in the object position of the triple.</skos:scopeNote>
    <!-- S15 -->
    <rdf:type rdf:resource="&owl;DatatypeProperty"/>
    <!-- For non-OWL aware applications -->
    <rdf:type rdf:resource="http://www.w3.org/1999/02/22-rdf-syntax-ns#Property"/>
  </rdf:Description>

  <rdf:Description rdf:about="&skos;note">
    <rdfs:label xml:lang="en">note</rdfs:label>
    <skos:definition xml:lang="en">A general note, for any purpose.</skos:definition>
    <skos:scopeNote xml:lang="en">This property may be used directly, or as a super-property for more specific note types.</skos:scopeNote>
    <!-- S16 -->
    <rdf:type rdf:resource="&owl;AnnotationProperty"/>
    <!-- For non-OWL aware applications -->
    <rdf:type rdf:resource="http://www.w3.org/1999/02/22-rdf-syntax-ns#Property"/>
  </rdf:Description>

  <rdf:Description rdf:about="&skos;changeNote">
    <rdfs:label xml:lang="en">change note</rdfs:label>
    <skos:definition xml:lang="en">A note about a modification to a concept.</skos:definition>
    <!-- S16 -->
    <rdf:type rdf:resource="&owl;AnnotationProperty"/>
    <!-- S17 -->
    <rdfs:subPropertyOf rdf:resource="&skos;note"/>
    <!-- For non-OWL aware applications -->
    <rdf:type rdf:resource="http://www.w3.org/1999/02/22-rdf-syntax-ns#Property"/>
  </rdf:Description>

  <rdf:Description rdf:about="&skos;definition">
    <rdfs:label xml:lang="en">definition</rdfs:label>
    <skos:definition xml:lang="en">A statement or formal explanation of the meaning of a concept.</skos:definition>
    <!-- S16 -->
    <rdf:type rdf:resource="&owl;AnnotationProperty"/>
    <!-- S17 -->
    <rdfs:subPropertyOf rdf:resource="&skos;note"/>
    <!-- For non-OWL aware applications -->
    <rdf:type rdf:resource="http://www.w3.org/1999/02/22-rdf-syntax-ns#Property"/>
  </rdf:Description>

  <rdf:Description rdf:about="&skos;editorialNote">
    <rdfs:label xml:lang="en">editorial note</rdfs:label>
    <skos:definition xml:lang="en">A note for an editor, translator or maintainer of the vocabulary.</skos:definition>
    <!-- S16 -->
    <rdf:type rdf:resource="&owl;AnnotationProperty"/>
    <!-- S17 -->
    <rdfs:subPropertyOf rdf:resource="&skos;note"/>
    <!-- For non-OWL aware applications -->
    <rdf:type rdf:resource="http://www.w3.org/1999/02/22-rdf-syntax-ns#Property"/>
  </rdf:Description>

  <rdf:Description rdf:about="&skos;example">
    <rdfs:label xml:lang="en">example</rdfs:label>
    <skos:definition xml:lang="en">An example of the use of a concept.</skos:definition>
    <!-- S16 -->
    <rdf:type rdf:resource="&owl;AnnotationProperty"/>
    <!-- S17 -->
    <rdfs:subPropertyOf rdf:resource="&skos;note"/>
    <!-- For non-OWL aware applications -->
    <rdf:type rdf:resource="http://www.w3.org/1999/02/22-rdf-syntax-ns#Property"/>
  </rdf:Description>

  <rdf:Description rdf:about="&skos;historyNote">
    <rdfs:label xml:lang="en">history note</rdfs:label>
    <skos:definition xml:lang="en">A note about the past state/use/meaning of a concept.</skos:definition>
    <!-- S16 -->
    <rdf:type rdf:resource="&owl;AnnotationProperty"/>
    <!-- S17 -->
    <rdfs:subPropertyOf rdf:resource="&skos;note"/>
    <!-- For non-OWL aware applications -->
    <rdf:type rdf:resource="http://www.w3.org/1999/02/22-rdf-syntax-ns#Property"/>
  </rdf:Description>

  <rdf:Description rdf:about="&skos;scopeNote">
    <rdfs:label xml:lang="en">scope note</rdfs:label>
    <skos:definition xml:lang="en">A note that helps to clarify the meaning and/or the use of a concept.</skos:definition>
    <!-- S16 -->
    <rdf:type rdf:resource="&owl;AnnotationProperty"/>
    <!-- S17 -->
    <rdfs:subPropertyOf rdf:resource="&skos;note"/>
    <!-- For non-OWL aware applications -->
    <rdf:type rdf:resource="http://www.w3.org/1999/02/22-rdf-syntax-ns#Property"/>
  </rdf:Description>

  <rdf:Description rdf:about="&skos;semanticRelation">
    <rdfs:label xml:lang="en">is in semantic relation with</rdfs:label>

    <skos:definition xml:lang="en">Links a concept to a concept related by meaning.</skos:definition>
    <skos:scopeNote xml:lang="en">This property should not be used directly, but as a super-property for all properties denoting a relationship of meaning between concepts.</skos:scopeNote>
    <!-- S18 -->
    <rdf:type rdf:resource="&owl;ObjectProperty"/>
    <!-- S19 -->
    <rdfs:domain rdf:resource="&skos;Concept"/>
    <!-- S20 -->
    <rdfs:range rdf:resource="&skos;Concept"/>
    <!-- For non-OWL aware applications -->
    <rdf:type rdf:resource="http://www.w3.org/1999/02/22-rdf-syntax-ns#Property"/>
  </rdf:Description>

  <rdf:Description rdf:about="&skos;broader">
    <rdfs:label xml:lang="en">has broader concept</rdfs:label>
    <skos:definition xml:lang="en">Relates a concept to a concept that is more general in meaning.</skos:definition>
    <rdfs:comment xml:lang="en">Broader concepts are typically rendered as parents in a concept hierarchy (tree).</rdfs:comment>
    <skos:scopeNote xml:lang="en">By convention, skos:broader is only used to assert an immediate (i.e. direct) hierarchical link between two conceptual resources.</skos:scopeNote>
    <!-- S18 -->
    <rdf:type rdf:resource="&owl;ObjectProperty"/>
    <!-- S22 -->
    <rdfs:subPropertyOf rdf:resource="&skos;broaderTransitive"/>
    <!-- S25 -->
    <owl:inverseOf rdf:resource="&skos;narrower"/>
    <!-- For non-OWL aware applications -->
    <rdf:type rdf:resource="http://www.w3.org/1999/02/22-rdf-syntax-ns#Property"/>
  </rdf:Description>

  <rdf:Description rdf:about="&skos;narrower">
    <rdfs:label xml:lang="en">has narrower concept</rdfs:label>
    <skos:definition xml:lang="en">Relates a concept to a concept that is more specific in meaning.</skos:definition>
    <skos:scopeNote xml:lang="en">By convention, skos:broader is only used to assert an immediate (i.e. direct) hierarchical link between two conceptual resources.</skos:scopeNote>
    <rdfs:comment xml:lang="en">Narrower concepts are typically rendered as children in a concept hierarchy (tree).</rdfs:comment>
    <!-- S18 -->
    <rdf:type rdf:resource="&owl;ObjectProperty"/>
    <!-- S22 -->
    <rdfs:subPropertyOf rdf:resource="&skos;narrowerTransitive"/>
    <!-- S25 -->
    <owl:inverseOf rdf:resource="&skos;broader"/>
    <!-- For non-OWL aware applications -->

    <rdf:type rdf:resource="http://www.w3.org/1999/02/22-rdf-syntax-ns#Property"/>
  </rdf:Description>

  <rdf:Description rdf:about="&skos;related">
    <rdfs:label xml:lang="en">has related concept</rdfs:label>
    <skos:definition xml:lang="en">Relates a concept to a concept with which there is an associative semantic relationship.</skos:definition>
    <!-- S18 -->
    <rdf:type rdf:resource="&owl;ObjectProperty"/>
    <!-- S21 -->
    <rdfs:subPropertyOf rdf:resource="&skos;semanticRelation"/>
    <!-- S23 -->
    <rdf:type rdf:resource="&owl;SymmetricProperty"/>
    <!-- S27 (not formally stated) -->
    <rdfs:comment xml:lang="en">skos:related is disjoint with skos:broaderTransitive</rdfs:comment>
    <!-- For non-OWL aware applications -->
    <rdf:type rdf:resource="http://www.w3.org/1999/02/22-rdf-syntax-ns#Property"/>

  </rdf:Description>

  <rdf:Description rdf:about="&skos;broaderTransitive">
    <rdfs:label xml:lang="en">has broader transitive</rdfs:label>
    <skos:definition>skos:broaderTransitive is a transitive superproperty of skos:broader.</skos:definition>
    <skos:scopeNote xml:lang="en">By convention, skos:broaderTransitive is not used to make assertions. Rather, the properties can be used to draw inferences about the transitive closure of the hierarchical relation, which is useful e.g. when implementing a simple query expansion algorithm in a search application.</skos:scopeNote>
    <!-- S18 -->
    <rdf:type rdf:resource="&owl;ObjectProperty"/>
    <!-- S21 -->
    <rdfs:subPropertyOf rdf:resource="&skos;semanticRelation"/>
    <!-- S24 -->
    <rdf:type rdf:resource="&owl;TransitiveProperty"/>
    <!-- S26 -->
    <owl:inverseOf rdf:resource="&skos;narrowerTransitive"/>
    <!-- For non-OWL aware applications -->
    <rdf:type rdf:resource="http://www.w3.org/1999/02/22-rdf-syntax-ns#Property"/>
  </rdf:Description>

  <rdf:Description rdf:about="&skos;narrowerTransitive">
    <rdfs:label xml:lang="en">has narrower transitive</rdfs:label>
    <skos:definition>skos:narrowerTransitive is a transitive superproperty of skos:narrower.</skos:definition>
    <skos:scopeNote xml:lang="en">By convention, skos:narrowerTransitive is not used to make assertions. Rather, the properties can be used to draw inferences about the transitive closure of the hierarchical relation, which is useful e.g. when implementing a simple query expansion algorithm in a search application.</skos:scopeNote>
    <!-- S18 -->
    <rdf:type rdf:resource="&owl;ObjectProperty"/>
    <!-- S21 -->
    <rdfs:subPropertyOf rdf:resource="&skos;semanticRelation"/>
    <!-- S24 -->
    <rdf:type rdf:resource="&owl;TransitiveProperty"/>
    <!-- S26 -->
    <owl:inverseOf rdf:resource="&skos;broaderTransitive"/>
    <!-- For non-OWL aware applications -->
    <rdf:type rdf:resource="http://www.w3.org/1999/02/22-rdf-syntax-ns#Property"/>

  </rdf:Description>

  <rdf:Description rdf:about="&skos;member">
    <rdfs:label xml:lang="en">has member</rdfs:label>
    <skos:definition xml:lang="en">Relates a collection to one of its members.</skos:definition>
    <!-- S30 -->
    <rdf:type rdf:resource="&owl;ObjectProperty"/>
    <!-- S31 -->
    <rdfs:domain rdf:resource="&skos;Collection"/>
    <!-- S32 -->
    <rdfs:range>
      <rdf:Description>
	<owl:unionOf rdf:parseType="Collection">
	  <rdf:Description rdf:about="&skos;Concept"/>
	  <rdf:Description rdf:about="&skos;Collection"/>
	</owl:unionOf>
      </rdf:Description>
    </rdfs:range>
    <!-- For non-OWL aware applications -->
    <rdf:type rdf:resource="http://www.w3.org/1999/02/22-rdf-syntax-ns#Property"/>
  </rdf:Description>

  <rdf:Description rdf:about="&skos;memberList">
    <rdfs:label xml:lang="en">has member list</rdfs:label>
    <skos:definition xml:lang="en">Relates an ordered collection to the RDF list containing its members.</skos:definition>
    <!-- S30 -->
    <rdf:type rdf:resource="&owl;ObjectProperty"/>
    <!-- S33 -->
    <rdfs:domain rdf:resource="&skos;OrderedCollection"/>
    <!-- S35 -->
    <rdf:type rdf:resource="&owl;FunctionalProperty"/>
    <!-- S34 -->
    <rdfs:range rdf:resource="http://www.w3.org/1999/02/22-rdf-syntax-ns#List"/>
    <!-- S36 (not formally stated) -->
    <rdfs:comment xml:lang="en">For any resource, every item in the list given as the value of the
      skos:memberList property is also a value of the skos:member property.</rdfs:comment>
    <!-- For non-OWL aware applications -->
    <rdf:type rdf:resource="http://www.w3.org/1999/02/22-rdf-syntax-ns#Property"/>
  </rdf:Description>

  <rdf:Description rdf:about="&skos;mappingRelation">
    <rdfs:label xml:lang="en">is in mapping relation with</rdfs:label>
    <skos:definition xml:lang="en">Relates two concepts coming, by convention, from different schemes, and that have comparable meanings</skos:definition>
    <rdfs:comment xml:lang="en">These concept mapping relations mirror semantic relations, and the data model defined below is similar (with the exception of skos:exactMatch) to the data model defined for semantic relations. A distinct vocabulary is provided for concept mapping relations, to provide a convenient way to differentiate links within a concept scheme from links between concept schemes. However, this pattern of usage is not a formal requirement of the SKOS data model, and relies on informal definitions of best practice.</rdfs:comment>
    <!-- S38 -->
    <rdf:type rdf:resource="&owl;ObjectProperty"/>
    <!-- S39 -->
    <rdfs:subPropertyOf rdf:resource="&skos;semanticRelation"/>
    <!-- For non-OWL aware applications -->
    <rdf:type rdf:resource="http://www.w3.org/1999/02/22-rdf-syntax-ns#Property"/>
  </rdf:Description>

  <rdf:Description rdf:about="&skos;broadMatch">
    <rdfs:label xml:lang="en">has broader match</rdfs:label>
    <skos:definition xml:lang="en">skos:broadMatch is used to state a hierarchical mapping link between two conceptual resources in different concept schemes.</skos:definition>
    <!-- S38 -->
    <rdf:type rdf:resource="&owl;ObjectProperty"/>
    <!-- S40 -->
    <rdfs:subPropertyOf rdf:resource="&skos;mappingRelation"/>
    <!-- S41 -->
    <rdfs:subPropertyOf rdf:resource="&skos;broader"/>
    <!-- S43 -->
    <owl:inverseOf rdf:resource="&skos;narrowMatch"/>
    <!-- For non-OWL aware applications -->
    <rdf:type rdf:resource="http://www.w3.org/1999/02/22-rdf-syntax-ns#Property"/>
  </rdf:Description>

  <rdf:Description rdf:about="&skos;narrowMatch">
    <rdfs:label xml:lang="en">has narrower match</rdfs:label>

    <skos:definition xml:lang="en">skos:narrowMatch is used to state a hierarchical mapping link between two conceptual resources in different concept schemes.</skos:definition>
    <!-- S38 -->
    <rdf:type rdf:resource="&owl;ObjectProperty"/>
    <!-- S40 -->
    <rdfs:subPropertyOf rdf:resource="&skos;mappingRelation"/>
    <!-- S41 -->
    <rdfs:subPropertyOf rdf:resource="&skos;narrower"/>
    <!-- S43 -->
    <owl:inverseOf rdf:resource="&skos;broadMatch"/>
    <!-- For non-OWL aware applications -->
    <rdf:type rdf:resource="http://www.w3.org/1999/02/22-rdf-syntax-ns#Property"/>
  </rdf:Description>

  <rdf:Description rdf:about="&skos;relatedMatch">
    <rdfs:label xml:lang="en">has related match</rdfs:label>
    <skos:definition xml:lang="en">skos:relatedMatch is used to state an associative mapping link between two conceptual resources in different concept schemes.</skos:definition>
    <!-- S38 -->
    <rdf:type rdf:resource="&owl;ObjectProperty"/>
    <!-- S40 -->
    <rdfs:subPropertyOf rdf:resource="&skos;mappingRelation"/>
    <!-- S41 -->
    <rdfs:subPropertyOf rdf:resource="&skos;related"/>
    <!-- S44 -->
    <rdf:type rdf:resource="&owl;SymmetricProperty"/>
    <!-- For non-OWL aware applications -->
    <rdf:type rdf:resource="http://www.w3.org/1999/02/22-rdf-syntax-ns#Property"/>
  </rdf:Description>

  <rdf:Description rdf:about="&skos;exactMatch">
    <rdfs:label xml:lang="en">has exact match</rdfs:label>
    <skos:definition xml:lang="en">skos:exactMatch is used to link two concepts, indicating a high degree of confidence that the concepts can be used interchangeably across a wide range of information retrieval applications. skos:exactMatch is a transitive property, and is a sub-property of skos:closeMatch.</skos:definition>
    <!-- S38 -->
    <rdf:type rdf:resource="&owl;ObjectProperty"/>
    <!-- S42 -->
    <rdfs:subPropertyOf rdf:resource="&skos;closeMatch"/>
    <!-- S44 -->
    <rdf:type rdf:resource="&owl;SymmetricProperty"/>
    <!-- S45 -->
    <rdf:type rdf:resource="&owl;TransitiveProperty"/>
    <!-- S46 (not formally stated) -->
    <rdfs:comment xml:lang="en">skos:exactMatch is disjoint with each of the properties skos:broadMatch and skos:relatedMatch.</rdfs:comment>
    <!-- For non-OWL aware applications -->
    <rdf:type rdf:resource="http://www.w3.org/1999/02/22-rdf-syntax-ns#Property"/>
  </rdf:Description>

  <rdf:Description rdf:about="&skos;closeMatch">
    <rdfs:label xml:lang="en">has close match</rdfs:label>
    <skos:definition xml:lang="en">skos:closeMatch is used to link two concepts that are sufficiently similar that they can be used interchangeably in some information retrieval applications. In order to avoid the possibility of "compound errors" when combining mappings across more than two concept schemes, skos:closeMatch is not declared to be a transitive property.</skos:definition>
    <!-- S38 -->
    <rdf:type rdf:resource="&owl;ObjectProperty"/>
    <!-- S40 -->
    <rdfs:subPropertyOf rdf:resource="&skos;mappingRelation"/>
    <!-- S44 -->
    <rdf:type rdf:resource="&owl;SymmetricProperty"/>
    <!-- For non-OWL aware applications -->
    <rdf:type rdf:resource="http://www.w3.org/1999/02/22-rdf-syntax-ns#Property"/>
  </rdf:Description>


<!-- FOAF -->

  <owl:AnnotationProperty rdf:about="http://xmlns.com/wot/0.1/assurance"/>
  <owl:AnnotationProperty rdf:about="http://xmlns.com/wot/0.1/src_assurance"/>
  <owl:AnnotationProperty rdf:about="http://www.w3.org/2003/06/sw-vocab-status/ns#term_status"/>
  <!--  DC terms are NOT annotation properties in general, so we consider the following 
	claims scoped to this document. They may be removed in future revisions if
	OWL tools become more flexible. -->
  <owl:AnnotationProperty rdf:about="http://purl.org/dc/elements/1.1/description"/>
  <owl:AnnotationProperty rdf:about="http://purl.org/dc/elements/1.1/title"/>
  <owl:AnnotationProperty rdf:about="http://purl.org/dc/elements/1.1/date"/>
  <rdf:Description rdf:about="http://www.w3.org/2000/01/rdf-schema#Class"/>

<!--  <rdf:Description rdf:about="http://www.w3.org/2000/01/rdf-schema#Resource"/>
  <rdf:Description rdf:about="http://www.w3.org/2000/01/rdf-schema#Literal"/> -->
  <!-- end of OWL/RDF interop voodoo. mostly. -->

  
<!-- FOAF classes (types) are listed first. -->

  <rdf:Description rdf:about="&foaf;Person" rdfs:label="Person" rdfs:comment="A person." vs:term_status="stable">
    
    <!-- aside: 
	are spatial things always spatially located? 
	Person includes imaginary people... discuss... -->
    <owl:disjointWith rdf:resource="&foaf;Document"/>
    <owl:disjointWith rdf:resource="&foaf;Organization"/>
    <owl:disjointWith rdf:resource="&foaf;Project"/>
  </rdf:Description>
  <rdf:Description rdf:about="&foaf;Document" rdfs:label="Document" rdfs:comment="A document." vs:term_status="testing">
    
    <owl:disjointWith rdf:resource="&foaf;Organization"/>
    <owl:disjointWith rdf:resource="&foaf;Person"/>
    <owl:disjointWith rdf:resource="&foaf;Project"/>
  </rdf:Description>
  <rdf:Description rdf:about="&foaf;Organization" rdfs:label="Organization" rdfs:comment="An organization." vs:term_status="stable">
    
    <owl:disjointWith rdf:resource="&foaf;Person"/>
    <owl:disjointWith rdf:resource="&foaf;Document"/>
  </rdf:Description>
  <rdf:Description rdf:about="&foaf;Group" vs:term_status="stable" rdfs:label="Group" rdfs:comment="A class of Agents.">
    
  </rdf:Description>
  <rdf:Description rdf:about="&foaf;Agent" vs:term_status="stable" rdfs:label="Agent" rdfs:comment="An agent (eg. person, group, software or physical artifact).">
    
    <owl:disjointWith rdf:resource="&foaf;Document"/>
  </rdf:Description>
  <rdf:Description rdf:about="&foaf;Project" vs:term_status="unstable" rdfs:label="Project" rdfs:comment="A project (a collective endeavour of some kind).">
    
    <owl:disjointWith rdf:resource="&foaf;Person"/>
    <owl:disjointWith rdf:resource="&foaf;Document"/>
  </rdf:Description>
  <rdf:Description rdf:about="&foaf;Image" vs:term_status="testing" rdfs:label="Image" rdfs:comment="An image.">
    
  </rdf:Description>

  <rdf:Description rdf:about="&foaf;PersonalProfileDocument" rdfs:label="PersonalProfileDocument" rdfs:comment="A personal profile RDF document." vs:term_status="testing">
    
  </rdf:Description>
	
  <rdf:Description rdf:about="&foaf;OnlineAccount" vs:term_status="unstable" rdfs:label="Online Account" rdfs:comment="An online account.">
    
  </rdf:Description>
  <rdf:Description rdf:about="&foaf;OnlineGamingAccount" vs:term_status="unstable" rdfs:label="Online Gaming Account" rdfs:comment="An online gaming account.">
    
  </rdf:Description>
  <rdf:Description rdf:about="&foaf;OnlineEcommerceAccount" vs:term_status="unstable" rdfs:label="Online E-commerce Account" rdfs:comment="An online e-commerce account.">
    
  </rdf:Description>
  <rdf:Description rdf:about="&foaf;OnlineChatAccount" vs:term_status="unstable" rdfs:label="Online Chat Account" rdfs:comment="An online chat account.">
    
  </rdf:Description>
<!-- FOAF properties (ie. relationships). -->
  <rdf:Property rdf:about="&foaf;mbox" vs:term_status="stable" rdfs:label="personal mailbox" rdfs:comment="A 
personal mailbox, ie. an Internet mailbox associated with exactly one owner, the first owner of this mailbox. This is a 'static inverse functional property', in that  there is (across time and change) at most one individual that ever has any particular value for foaf:mbox.">
    <rdf:type rdf:resource="&owl;InverseFunctionalProperty"/>
    <rdf:type rdf:resource="&owl;ObjectProperty"/>
    <rdfs:domain rdf:resource="&foaf;Agent"/>
    <rdfs:range rdf:resource="&owl;Thing"/>
  </rdf:Property>
  <rdf:Property rdf:about="&foaf;mbox_sha1sum" vs:term_status="testing" rdfs:label="sha1sum of a personal mailbox URI name" rdfs:comment="The sha1sum of the URI of an Internet mailbox associated with exactly one owner, the  first owner of the mailbox.">
    <rdf:type rdf:resource="&owl;InverseFunctionalProperty"/>

<!--
put it back in again 2006-01-29 - see 
http://chatlogs.planetrdf.com/swig/2006-01-29.html#T21-12-35
I have mailed rdfweb-dev@vapours.rdfweb.org for discussion.
Libby

Commenting out as a kindness to OWL DL users. The semantics didn't quite cover
our usage anyway, since (a) we want static-across-time, which is so beyond OWL as 
to be from another planet (b) we want identity reasoning invariant across xml:lang 
tagging. FOAF code will know what to do. OWL folks note, this assertion might return. 

danbri
-->
    <rdf:type rdf:resource="&owl;DatatypeProperty"/>
    <rdfs:domain rdf:resource="&foaf;Agent"/>
    <rdfs:range rdf:resource="http://www.w3.org/2000/01/rdf-schema#Literal"/>
  </rdf:Property>

  <rdf:Property rdf:about="&foaf;gender" vs:term_status="testing" 
rdfs:label="gender" 
rdfs:comment="The gender of this Agent (typically but not necessarily 'male' or 'female').">
    <rdf:type rdf:resource="&owl;FunctionalProperty"/>
    <rdf:type rdf:resource="&owl;DatatypeProperty"/>
    <rdfs:domain rdf:resource="&foaf;Agent"/>
    <rdfs:range rdf:resource="http://www.w3.org/2000/01/rdf-schema#Literal"/>
    <!-- whatever one's gender is, and we are liberal in leaving room for more options 
    than 'male' and 'female', we model this so that an agent has only one gender. -->
  </rdf:Property>



  <rdf:Property rdf:about="&foaf;geekcode" vs:term_status="testing" rdfs:label="geekcode" rdfs:comment="A textual geekcode for this person, see http://www.geekcode.com/geek.html">
    <rdf:type rdf:resource="&owl;DatatypeProperty"/>
    <rdfs:domain rdf:resource="&foaf;Person"/>
    <rdfs:range rdf:resource="http://www.w3.org/2000/01/rdf-schema#Literal"/>
  </rdf:Property>
  <rdf:Property rdf:about="&foaf;dnaChecksum" vs:term_status="unstable" rdfs:label="DNA checksum" rdfs:comment="A checksum for the DNA of some thing. Joke.">
    <rdf:type rdf:resource="&owl;DatatypeProperty"/>
    <rdfs:range rdf:resource="http://www.w3.org/2000/01/rdf-schema#Literal"/>
  </rdf:Property>
  <rdf:Property rdf:about="&foaf;sha1" vs:term_status="unstable" rdfs:label="sha1sum (hex)" rdfs:comment="A sha1sum hash, in hex.">
    <rdf:type rdf:resource="&owl;DatatypeProperty"/>
    <rdfs:domain rdf:resource="&foaf;Document"/>
<!-- rdf:type rdf:resource="&owl;InverseFunctionalProperty" -->
<!-- IFP under discussion -->
  </rdf:Property>
  <rdf:Property rdf:about="&foaf;based_near" vs:term_status="unstable" rdfs:label="based near" rdfs:comment="A location that something is based near, for some broadly human notion of near.">
<!-- see http://esw.w3.org/topic/GeoOnion for extension  ideas -->
<!-- this was ranged as Agent... hmm -->
    <rdf:type rdf:resource="&owl;ObjectProperty"/>
    <rdfs:domain rdf:resource="http://www.w3.org/2003/01/geo/wgs84_pos#SpatialThing"/>
    <rdfs:range rdf:resource="http://www.w3.org/2003/01/geo/wgs84_pos#SpatialThing"/>
  </rdf:Property>
<!-- FOAF naming properties -->
  <rdf:Property rdf:about="&foaf;title" vs:term_status="testing" rdfs:label="title" rdfs:comment="Title (Mr, Mrs, Ms, Dr. etc)">
    <rdf:type rdf:resource="&owl;DatatypeProperty"/>
  </rdf:Property>
  <rdf:Property rdf:about="&foaf;nick" vs:term_status="testing" rdfs:label="nickname" rdfs:comment="A short informal nickname characterising an agent (includes login identifiers, IRC and other chat nicknames).">
    <rdf:type rdf:resource="&owl;DatatypeProperty"/>
  </rdf:Property>
<!-- ......................... chat IDs ........................... -->
  <rdf:Property rdf:about="&foaf;jabberID" vs:term_status="testing" rdfs:label="jabber ID" rdfs:comment="A jabber ID for something.">
<!--
    <rdfs:subPropertyOf rdf:resource="&foaf;nick"/>
...different to the other IM IDs, as Jabber has wider usage, so 
we don't want the implied rdfs:domain here.

-->
    <rdfs:domain rdf:resource="&foaf;Agent"/>
    <rdfs:range rdf:resource="http://www.w3.org/2000/01/rdf-schema#Literal"/>
    <!-- there is a case for using resources/URIs here, ... -->
    <rdf:type rdf:resource="&owl;DatatypeProperty"/>
    <rdf:type rdf:resource="&owl;InverseFunctionalProperty"/>
  </rdf:Property>
  <rdf:Property rdf:about="&foaf;aimChatID" vs:term_status="testing" rdfs:label="AIM chat ID" rdfs:comment="An AIM chat ID">
    <rdf:type rdf:resource="&owl;DatatypeProperty"/>
    <rdfs:subPropertyOf rdf:resource="&foaf;nick"/>
    <rdfs:domain rdf:resource="&foaf;Agent"/>
    <rdfs:range rdf:resource="http://www.w3.org/2000/01/rdf-schema#Literal"/>
    <rdf:type rdf:resource="&owl;InverseFunctionalProperty"/>
  </rdf:Property>
<!-- http://www.stud.uni-karlsruhe.de/~uck4/ICQ/Packet-112.html -->
  <rdf:Property rdf:about="&foaf;icqChatID" vs:term_status="testing" rdfs:label="ICQ chat ID" rdfs:comment="An ICQ chat ID">
    <rdf:type rdf:resource="&owl;DatatypeProperty"/>
    <rdfs:subPropertyOf rdf:resource="&foaf;nick"/>
    <rdfs:domain rdf:resource="&foaf;Agent"/>
    <rdfs:range rdf:resource="http://www.w3.org/2000/01/rdf-schema#Literal"/>
    <rdf:type rdf:resource="&owl;InverseFunctionalProperty"/>
  </rdf:Property>
  <rdf:Property rdf:about="&foaf;yahooChatID" vs:term_status="testing" rdfs:label="Yahoo chat ID" rdfs:comment="A Yahoo chat ID">
    <rdf:type rdf:resource="&owl;DatatypeProperty"/>
    <rdfs:subPropertyOf rdf:resource="&foaf;nick"/>
    <rdfs:domain rdf:resource="&foaf;Agent"/>
    <rdfs:range rdf:resource="http://www.w3.org/2000/01/rdf-schema#Literal"/>
    <rdf:type rdf:resource="&owl;InverseFunctionalProperty"/>
  </rdf:Property>
  <rdf:Property rdf:about="&foaf;msnChatID" vs:term_status="testing" rdfs:label="MSN chat ID" rdfs:comment="An MSN chat ID">
    <rdf:type rdf:resource="&owl;DatatypeProperty"/>
    <rdfs:subPropertyOf rdf:resource="&foaf;nick"/>
    <rdfs:domain rdf:resource="&foaf;Agent"/>
    <rdfs:range rdf:resource="http://www.w3.org/2000/01/rdf-schema#Literal"/>
    <rdf:type rdf:resource="&owl;InverseFunctionalProperty"/>
  </rdf:Property>
<!-- ....................................................... -->
  <rdf:Property rdf:about="&foaf;name" vs:term_status="testing" rdfs:label="name" rdfs:comment="A name for some thing.">
    <rdf:type rdf:resource="&owl;DatatypeProperty"/>
    <rdfs:domain rdf:resource="&owl;Thing"/>
    <rdfs:range rdf:resource="http://www.w3.org/2000/01/rdf-schema#Literal"/>
    <rdfs:subPropertyOf rdf:resource="http://www.w3.org/2000/01/rdf-schema#label"/>
  </rdf:Property>
  <rdf:Property rdf:about="&foaf;firstName" vs:term_status="testing" rdfs:label="firstName" rdfs:comment="The first name of a person.">
    <rdf:type rdf:resource="&owl;DatatypeProperty"/>
    <rdfs:domain rdf:resource="&foaf;Person"/>
    <rdfs:range rdf:resource="http://www.w3.org/2000/01/rdf-schema#Literal"/>
  </rdf:Property>
  <rdf:Property rdf:about="&foaf;givenname" vs:term_status="testing" rdfs:label="Given name" rdfs:comment="The given name of some person.">
    <rdf:type rdf:resource="&owl;DatatypeProperty"/>
  </rdf:Property>
  <rdf:Property rdf:about="&foaf;surname" vs:term_status="testing" rdfs:label="Surname" rdfs:comment="The surname of some person.">
    <rdf:type rdf:resource="&owl;DatatypeProperty"/>
    <rdfs:domain rdf:resource="&foaf;Person"/>
    <rdfs:range rdf:resource="http://www.w3.org/2000/01/rdf-schema#Literal"/>
  </rdf:Property>
  <rdf:Property rdf:about="&foaf;family_name" vs:term_status="testing" rdfs:label="family_name" rdfs:comment="The family_name of some person.">
    <rdf:type rdf:resource="&owl;DatatypeProperty"/>
    <rdfs:domain rdf:resource="&foaf;Person"/>
    <rdfs:domain rdf:resource="&foaf;Person"/>
    <rdfs:range rdf:resource="http://www.w3.org/2000/01/rdf-schema#Literal"/>
  </rdf:Property>
<!-- end of naming properties. See http://rdfweb.org/issues/show_bug.cgi?id=7
	   for open issue / re-design discussions.
	-->
  <rdf:Property rdf:about="&foaf;phone" vs:term_status="testing" rdfs:label="phone" rdfs:comment="A phone,  specified using fully qualified tel: URI scheme (refs: http://www.w3.org/Addressing/schemes.html#tel).">
    <rdf:type rdf:resource="&owl;ObjectProperty"/>
  </rdf:Property>
  <rdf:Property rdf:about="&foaf;homepage" vs:term_status="stable" rdfs:label="homepage" rdfs:comment="A homepage for some thing.">
    <rdf:type rdf:resource="&owl;ObjectProperty"/>
    <rdfs:subPropertyOf rdf:resource="&foaf;page"/>
    <rdfs:subPropertyOf rdf:resource="&foaf;isPrimaryTopicOf"/>
    <rdf:type rdf:resource="&owl;InverseFunctionalProperty"/>
    <!--  previously: rdfs:domain rdf:resource="&foaf;Agent" -->
    <rdfs:domain rdf:resource="&owl;Thing"/>
    <rdfs:range rdf:resource="&foaf;Document"/>
  </rdf:Property>
  <rdf:Property rdf:about="&foaf;weblog" vs:term_status="testing" rdfs:label="weblog" rdfs:comment="A weblog of some thing (whether person, group, company etc.).">
    <rdf:type rdf:resource="&owl;ObjectProperty"/>
    <rdfs:subPropertyOf rdf:resource="&foaf;page"/>
    <rdf:type rdf:resource="&owl;InverseFunctionalProperty"/>
    <rdfs:domain rdf:resource="&foaf;Agent"/>
    <rdfs:range rdf:resource="&foaf;Document"/>
  </rdf:Property>
  <rdf:Property rdf:about="&foaf;tipjar" vs:term_status="testing" rdfs:label="tipjar" rdfs:comment="A tipjar document for this agent, describing means for payment and reward.">
    <rdf:type rdf:resource="&owl;ObjectProperty"/>
    <rdfs:subPropertyOf rdf:resource="&foaf;page"/>
    <rdfs:domain rdf:resource="&foaf;Agent"/>
    <rdfs:range rdf:resource="&foaf;Document"/>
  </rdf:Property>
  <rdf:Property rdf:about="&foaf;plan" vs:term_status="testing" rdfs:label="plan" rdfs:comment="A .plan comment, in the tradition of finger and '.plan' files.">
    <rdf:type rdf:resource="&owl;DatatypeProperty"/>
    <rdfs:domain rdf:resource="&foaf;Person"/>
    <rdfs:range rdf:resource="http://www.w3.org/2000/01/rdf-schema#Literal"/>
  </rdf:Property>
  <rdf:Property rdf:about="&foaf;made" vs:term_status="stable" rdfs:label="made" rdfs:comment="Something that was made by this agent.">
    <rdf:type rdf:resource="&owl;ObjectProperty"/>
    <rdfs:domain rdf:resource="&foaf;Agent"/>
    <rdfs:range rdf:resource="&owl;Thing"/>
    <owl:inverseOf rdf:resource="&foaf;maker"/>
  </rdf:Property>
  <rdf:Property rdf:about="&foaf;maker"  vs:term_status="stable" rdfs:label="maker" rdfs:comment="An agent that 
made this thing.">
    <rdf:type rdf:resource="&owl;ObjectProperty"/>
    <rdfs:domain rdf:resource="&owl;Thing"/>
    <rdfs:range rdf:resource="&foaf;Agent"/>
    <owl:inverseOf rdf:resource="&foaf;made"/>
  </rdf:Property>
  <rdf:Property rdf:about="&foaf;img" vs:term_status="testing" rdfs:label="image" rdfs:comment="An image that can be used to represent some thing (ie. those depictions which are particularly representative of something, eg. one's photo on a homepage).">
    <rdf:type rdf:resource="&owl;ObjectProperty"/>
    <rdfs:domain rdf:resource="&foaf;Person"/>
    <rdfs:range rdf:resource="&foaf;Image"/>
    <rdfs:subPropertyOf rdf:resource="&foaf;depiction"/>
  </rdf:Property>
  <rdf:Property rdf:about="&foaf;depiction" vs:term_status="testing" rdfs:label="depiction" rdfs:comment="A depiction of some thing.">
    <rdf:type rdf:resource="&owl;ObjectProperty"/>
    <rdfs:domain rdf:resource="&owl;Thing"/>
    <rdfs:range rdf:resource="&foaf;Image"/>
    <owl:inverseOf rdf:resource="&foaf;depicts"/>
  </rdf:Property>
  <rdf:Property rdf:about="&foaf;depicts" vs:term_status="testing" rdfs:label="depicts" rdfs:comment="A thing depicted in this representation.">
    <rdf:type rdf:resource="&owl;ObjectProperty"/>
    <rdfs:range rdf:resource="&owl;Thing"/>
    <rdfs:domain rdf:resource="&foaf;Image"/>
    <owl:inverseOf rdf:resource="&foaf;depiction"/>
  </rdf:Property>
  <rdf:Property rdf:about="&foaf;thumbnail" vs:term_status="testing" rdfs:label="thumbnail" rdfs:comment="A derived thumbnail image.">
    <rdf:type rdf:resource="&owl;ObjectProperty"/>
    <rdfs:domain rdf:resource="&foaf;Image"/>
    <rdfs:range rdf:resource="&foaf;Image"/>
  </rdf:Property>
  <rdf:Property rdf:about="&foaf;myersBriggs" vs:term_status="testing" rdfs:label="myersBriggs" rdfs:comment="A Myers Briggs (MBTI) personality classification.">
    <rdf:type rdf:resource="&owl;ObjectProperty"/>
    <rdfs:domain rdf:resource="&foaf;Person"/>
    <rdfs:range rdf:resource="http://www.w3.org/2000/01/rdf-schema#Literal"/>
  </rdf:Property>
  <rdf:Property rdf:about="&foaf;workplaceHomepage" vs:term_status="testing" rdfs:label="workplace homepage" rdfs:comment="A workplace homepage of some person; the homepage of an organization they work for.">
    <rdf:type rdf:resource="&owl;ObjectProperty"/>
    <rdfs:domain rdf:resource="&foaf;Person"/>
    <rdfs:range rdf:resource="&foaf;Document"/>
  </rdf:Property>
  <rdf:Property rdf:about="&foaf;workInfoHomepage" vs:term_status="testing" rdfs:label="work info homepage" rdfs:comment="A work info homepage of some person; a page about their work for some organization.">
    <rdf:type rdf:resource="&owl;ObjectProperty"/>
    <rdfs:domain rdf:resource="&foaf;Person"/>
    <rdfs:range rdf:resource="&foaf;Document"/>
  </rdf:Property>
  <rdf:Property rdf:about="&foaf;schoolHomepage" vs:term_status="testing" rdfs:label="schoolHomepage" rdfs:comment="A homepage of a school attended by the person.">
    <rdf:type rdf:resource="&owl;ObjectProperty"/>
    <rdfs:domain rdf:resource="&foaf;Person"/>
    <rdfs:range rdf:resource="&foaf;Document"/>
  </rdf:Property>
  <rdf:Property rdf:about="&foaf;knows" vs:term_status="testing" rdfs:label="knows" rdfs:comment="A person known by this person (indicating some level of reciprocated interaction between the parties).">
    <rdf:type rdf:resource="&owl;ObjectProperty"/>
    <rdfs:domain rdf:resource="&foaf;Person"/>
    <rdfs:range rdf:resource="&foaf;Person"/>
  </rdf:Property>
  <rdf:Property rdf:about="&foaf;interest" vs:term_status="testing" rdfs:label="interest" rdfs:comment="A page about a topic of interest to this person.">
<!-- we should distinguish the page from the topic more carefully. danbri 2002-07-08 -->
    <rdf:type rdf:resource="&owl;ObjectProperty"/>
    <rdfs:domain rdf:resource="&foaf;Person"/>
    <rdfs:range rdf:resource="&foaf;Document"/>
  </rdf:Property>
  <rdf:Property rdf:about="&foaf;topic_interest" vs:term_status="testing" rdfs:label="interest_topic" rdfs:comment="A thing of interest to this person.">
<!-- we should distinguish the page from the topic more carefully. danbri 2002-07-08 -->
<!--    foaf:interest_topic(P,R) 
		always true whenever
		foaf:interest(P,D), foaf:topic(D,R) 
		ie. a person has a foaf:topic_interest in all things 
		that are the foaf:topic of pages they have a foaf:interest in. 
		hmm, does this mean i'm forced to be interested in all the things that are the 
		topic of a page i'm interested in. thats a strong restriction on foaf:topic's utility.	-->
    <rdf:type rdf:resource="&owl;ObjectProperty"/>
    <rdfs:domain rdf:resource="&foaf;Person"/>
    <rdfs:range rdf:resource="&owl;Thing"/>
  </rdf:Property>
  <rdf:Property rdf:about="&foaf;publications" vs:term_status="unstable" rdfs:label="publications" rdfs:comment="A link to the publications of this person.">
    <rdf:type rdf:resource="&owl;ObjectProperty"/>
    <rdfs:domain rdf:resource="&foaf;Person"/>
    <rdfs:range rdf:resource="&foaf;Document"/>
  </rdf:Property>
<!-- by libby for ILRT mappings 2001-10-31 -->
  <rdf:Property rdf:about="&foaf;currentProject" vs:term_status="testing" rdfs:label="current project" rdfs:comment="A current project this person works on.">
    <rdf:type rdf:resource="&owl;ObjectProperty"/>
    <rdfs:domain rdf:resource="&foaf;Person"/>
    <rdfs:range rdf:resource="&owl;Thing"/>
  </rdf:Property>
  <rdf:Property rdf:about="&foaf;pastProject" vs:term_status="testing" rdfs:label="past project" rdfs:comment="A project this person has previously worked on.">
    <rdf:type rdf:resource="&owl;ObjectProperty"/>
    <rdfs:domain rdf:resource="&foaf;Person"/>
    <rdfs:range rdf:resource="&owl;Thing"/>
  </rdf:Property>
  <rdf:Property rdf:about="&foaf;fundedBy" vs:term_status="unstable" rdfs:label="funded by" rdfs:comment="An organization funding a project or person.">
    <rdf:type rdf:resource="&owl;ObjectProperty"/>
    <rdfs:domain rdf:resource="&owl;Thing"/>
    <rdfs:range rdf:resource="&owl;Thing"/>
  </rdf:Property>
  <rdf:Property rdf:about="&foaf;logo" vs:term_status="testing" rdfs:label="logo" rdfs:comment="A logo representing some thing.">
    <rdf:type rdf:resource="&owl;ObjectProperty"/>
    <rdfs:domain rdf:resource="&owl;Thing"/>
    <rdfs:range rdf:resource="&owl;Thing"/>
  </rdf:Property>
  <rdf:Property rdf:about="&foaf;topic" vs:term_status="testing" rdfs:label="topic" rdfs:comment="A topic of some page or document.">
    <rdf:type rdf:resource="&owl;ObjectProperty"/>
    <rdfs:domain rdf:resource="&foaf;Document"/>
    <rdfs:range rdf:resource="&owl;Thing"/>
    <owl:inverseOf rdf:resource="&foaf;page"/>
  </rdf:Property>
  <rdf:Property rdf:about="&foaf;primaryTopic"
 vs:term_status="testing" rdfs:label="primary topic" rdfs:comment="The primary topic of some page or document.">
    <rdf:type rdf:resource="&owl;FunctionalProperty"/>
    <rdf:type rdf:resource="&owl;ObjectProperty"/>
    <rdfs:domain rdf:resource="&foaf;Document"/>
    <rdfs:range rdf:resource="&owl;Thing"/>
    <owl:inverseOf rdf:resource="&foaf;isPrimaryTopicOf"/>
  </rdf:Property>

  <rdf:Property rdf:about="&foaf;isPrimaryTopicOf"
 vs:term_status="testing" rdfs:label="is primary topic of" rdfs:comment="A document that this thing is the primary topic of.">
    <rdf:type rdf:resource="&owl;InverseFunctionalProperty"/>
    <rdfs:subPropertyOf rdf:resource="&foaf;page"/>
    <owl:inverseOf rdf:resource="&foaf;primaryTopic"/>
    <rdfs:domain rdf:resource="&owl;Thing"/>
    <rdfs:range rdf:resource="&foaf;Document"/>
  </rdf:Property>

  <rdf:Property rdf:about="&foaf;page" vs:term_status="testing" rdfs:label="page" rdfs:comment="A page or document about this thing.">
    <rdf:type rdf:resource="&owl;ObjectProperty"/>
    <rdfs:domain rdf:resource="&owl;Thing"/>
    <rdfs:range rdf:resource="&foaf;Document"/>
    <owl:inverseOf rdf:resource="&foaf;topic"/>
  </rdf:Property>
  <rdf:Property rdf:about="&foaf;theme" vs:term_status="unstable" rdfs:label="theme" rdfs:comment="A theme.">
    <rdf:type rdf:resource="&owl;ObjectProperty"/>
    <rdfs:domain rdf:resource="&owl;Thing"/>
    <rdfs:range rdf:resource="&owl;Thing"/>
  </rdf:Property>
  <rdf:Property rdf:about="&foaf;holdsAccount" vs:term_status="unstable" rdfs:label="holds account" rdfs:comment="Indicates an account held by this agent.">
    <rdf:type rdf:resource="&owl;ObjectProperty"/>
    <rdfs:domain rdf:resource="&foaf;Agent"/>
    <rdfs:range rdf:resource="&foaf;OnlineAccount"/>
  </rdf:Property>
  <rdf:Property rdf:about="&foaf;accountServiceHomepage" vs:term_status="unstable" rdfs:label="account service homepage" rdfs:comment="Indicates a homepage of the service provide for this online account.">
    <rdf:type rdf:resource="&owl;ObjectProperty"/>
    <rdfs:domain rdf:resource="&foaf;OnlineAccount"/>
    <rdfs:range rdf:resource="&foaf;Document"/>
  </rdf:Property>
  <rdf:Property rdf:about="&foaf;accountName" vs:term_status="unstable" rdfs:label="account name" rdfs:comment="Indicates the name (identifier) associated with this online account.">
    <rdf:type rdf:resource="&owl;DatatypeProperty"/>
    <rdfs:domain rdf:resource="&foaf;OnlineAccount"/>
    <rdfs:range rdf:resource="http://www.w3.org/2000/01/rdf-schema#Literal"/>
  </rdf:Property>
  <rdf:Property rdf:about="&foaf;member" vs:term_status="stable" rdfs:label="member" rdfs:comment="Indicates a member of a Group">
    <rdf:type rdf:resource="&owl;ObjectProperty"/>
    <rdfs:domain rdf:resource="&foaf;Group"/>
    <rdfs:range rdf:resource="&foaf;Agent"/>
  </rdf:Property>

  <rdf:Property rdf:about="&foaf;membershipClass" vs:term_status="unstable" rdfs:label="membershipClass" rdfs:comment="Indicates the class of individuals that are a member of a Group">
    <rdf:type rdf:resource="&owl;AnnotationProperty"/>
  </rdf:Property>


  <rdf:Property rdf:about="&foaf;birthday" vs:term_status="unstable" rdfs:label="birthday" rdfs:comment="The birthday of this Agent, represented in mm-dd string form, eg. '12-31'.">
    <rdf:type rdf:resource="&owl;FunctionalProperty"/>
    <rdf:type rdf:resource="&owl;DatatypeProperty"/>
    <rdfs:domain rdf:resource="&foaf;Agent"/>
    <rdfs:range rdf:resource="&rdfs;Literal"/>
  </rdf:Property>


<!-- SIOC -->



<!-- Classes -->
<rdf:Description rdf:about="&sioc;Community">
  <rdfs:label xml:lang="en">Community</rdfs:label>
  <rdfs:comment xml:lang="en">Community is a high-level concept that defines an online community and what it consists of.</rdfs:comment>
  <owl:disjointWith rdf:resource="&sioc;Item"/>
  <owl:disjointWith rdf:resource="&sioc;Role"/>
  <owl:disjointWith rdf:resource="&sioc;User"/>
</rdf:Description>

<rdf:Description rdf:about="&sioc;Container">
  <rdfs:label xml:lang="en">Container</rdfs:label>
  <rdfs:comment xml:lang="en">An area in which content Items are contained.</rdfs:comment>
  <owl:disjointWith rdf:resource="&sioc;Item"/>
  <owl:disjointWith rdf:resource="&sioc;Role"/>
  <owl:disjointWith rdf:resource="&sioc;User"/>
  <owl:disjointWith rdf:resource="&sioc;Usergroup"/>
</rdf:Description>

<rdf:Description rdf:about="&sioc;Forum">
  <rdfs:label xml:lang="en">Forum</rdfs:label>
  <rdfs:comment xml:lang="en">A discussion area on which Posts or entries are made.</rdfs:comment>
</rdf:Description>

<rdf:Description rdf:about="&sioc;Item">
  <rdfs:label xml:lang="en">Item</rdfs:label>
  <rdfs:comment xml:lang="en">An Item is something which can be in a Container.</rdfs:comment>
  <owl:disjointWith rdf:resource="&sioc;Container"/>
  <owl:disjointWith rdf:resource="&sioc;Role"/>
  <owl:disjointWith rdf:resource="&sioc;Space"/>
  <owl:disjointWith rdf:resource="&sioc;User"/>
  <owl:disjointWith rdf:resource="&sioc;Usergroup"/>
</rdf:Description>

<rdf:Description rdf:about="&sioc;Post">
  <rdfs:label xml:lang="en">Post</rdfs:label>
  <rdfs:comment xml:lang="en">An article or message that can be posted to a Forum.</rdfs:comment>
</rdf:Description>

<rdf:Description rdf:about="&sioc;Role">
  <rdfs:label xml:lang="en">Role</rdfs:label>
  <rdfs:comment xml:lang="en">A Role is a function of a User within a scope of a particular Forum, Site, etc.</rdfs:comment>
  <owl:disjointWith rdf:resource="&sioc;Container"/>
  <owl:disjointWith rdf:resource="&sioc;Item"/>
  <owl:disjointWith rdf:resource="&sioc;Space"/>
  <owl:disjointWith rdf:resource="&sioc;User"/>
  <owl:disjointWith rdf:resource="&sioc;Usergroup"/>
</rdf:Description>

<rdf:Description rdf:about="&sioc;Space">
  <rdfs:label xml:lang="en">Space</rdfs:label>
  <rdfs:comment xml:lang="en">A Space is a place where data resides, e.g. on a website, desktop, fileshare, etc.</rdfs:comment>
  <owl:disjointWith rdf:resource="&sioc;Item"/>
  <owl:disjointWith rdf:resource="&sioc;Role"/>
  <owl:disjointWith rdf:resource="&sioc;User"/>
  <owl:disjointWith rdf:resource="&sioc;Usergroup"/>
</rdf:Description>

<rdf:Description rdf:about="&sioc;Site">
  <rdfs:label xml:lang="en">Site</rdfs:label>
  <rdfs:comment xml:lang="en">A Site can be the location of an online community or set of communities, with Users and Usergroups creating Items in a set of Containers. It can be thought of as a web-accessible data Space.</rdfs:comment>
</rdf:Description>

<rdf:Description rdf:about="&sioc;Thread">
  <rdfs:label xml:lang="en">Thread</rdfs:label>
  <rdfs:comment xml:lang="en">A container for a series of threaded discussion Posts or Items.</rdfs:comment>
</rdf:Description>

<rdf:Description rdf:about="&sioc;User">
  <rdfs:label xml:lang="en">User</rdfs:label>
  <rdfs:comment xml:lang="en">A User account in an online community site.</rdfs:comment>

  <owl:disjointWith rdf:resource="&sioc;Container"/>
  <owl:disjointWith rdf:resource="&sioc;Item"/>
  <owl:disjointWith rdf:resource="&sioc;Role"/>
  <owl:disjointWith rdf:resource="&sioc;Space"/>
  <owl:disjointWith rdf:resource="&sioc;Usergroup"/>
</rdf:Description>

<rdf:Description rdf:about="&sioc;Usergroup">
  <rdfs:label xml:lang="en">Usergroup</rdfs:label>
  <rdfs:comment xml:lang="en">A set of User accounts whose owners have a common purpose or interest. Can be used for access control purposes.</rdfs:comment>
  <owl:disjointWith rdf:resource="&sioc;Container"/>
  <owl:disjointWith rdf:resource="&sioc;Item"/>
  <owl:disjointWith rdf:resource="&sioc;Role"/>
  <owl:disjointWith rdf:resource="&sioc;Space"/>
  <owl:disjointWith rdf:resource="&sioc;User"/>
</rdf:Description>

<!-- Properties -->

<owl:ObjectProperty rdf:about="&sioc;about">
  <rdfs:label xml:lang="en">about</rdfs:label>
  <rdfs:comment xml:lang="en">Specifies that this Item is about a particular resource, e.g. a Post describing a book, hotel, etc.</rdfs:comment>
  <rdfs:domain rdf:resource="&sioc;Item"/>
</owl:ObjectProperty>

<owl:ObjectProperty rdf:about="&sioc;account_of">
  <rdfs:label xml:lang="en">account_of</rdfs:label>
  <rdfs:comment xml:lang="en">Refers to the foaf:Agent or foaf:Person who owns this sioc:User online account.</rdfs:comment>
  <rdfs:domain rdf:resource="&sioc;User"/>
  <rdfs:range rdf:resource="http://xmlns.com/foaf/0.1/Agent"/>
  <owl:inverseOf rdf:resource="http://xmlns.com/foaf/0.1/holdsAccount"/>
</owl:ObjectProperty>

<!-- @@todo: moving this property to the access module ? -->
<owl:ObjectProperty rdf:about="&sioc;administrator_of">
  <rdfs:label xml:lang="en">administrator_of</rdfs:label>
  <owl:inverseOf rdf:resource="&sioc;has_administrator"/>
  <rdfs:comment xml:lang="en">A Site that the User is an administrator of.</rdfs:comment>
  <rdfs:domain rdf:resource="&sioc;User"/>
  <rdfs:range rdf:resource="&sioc;Site"/>
</owl:ObjectProperty>

<owl:ObjectProperty rdf:about="&sioc;attachment">
  <rdfs:label xml:lang="en">attachment</rdfs:label>
  <rdfs:comment xml:lang="en">The URI of a file attached to an Item.</rdfs:comment>
  <rdfs:domain rdf:resource="&sioc;Item"/>
</owl:ObjectProperty>

<owl:ObjectProperty rdf:about="&sioc;avatar">
  <rdfs:label xml:lang="en">avatar</rdfs:label>
  <rdfs:comment xml:lang="en">An image or depiction used to represent this User.</rdfs:comment>
  <rdfs:domain rdf:resource="&sioc;User"/>
  <rdfs:subPropertyOf rdf:resource="http://xmlns.com/foaf/0.1/depiction"/>
</owl:ObjectProperty>

<owl:ObjectProperty rdf:about="&sioc;container_of">
  <rdfs:label xml:lang="en">container_of</rdfs:label>
  <owl:inverseOf rdf:resource="&sioc;has_container"/>
  <rdfs:comment xml:lang="en">An Item that this Container contains.</rdfs:comment>
  <rdfs:domain rdf:resource="&sioc;Container"/>
  <rdfs:range rdf:resource="&sioc;Item"/>
</owl:ObjectProperty>

<owl:DatatypeProperty rdf:about="&sioc;content">
  <rdfs:label xml:lang="en">content</rdfs:label>
  <rdfs:comment xml:lang="en">The content of the Item in plain text format.</rdfs:comment>
  <rdfs:domain rdf:resource="&sioc;Item"/>
  <rdfs:range rdf:resource="http://www.w3.org/2000/01/rdf-schema#Literal"/>
</owl:DatatypeProperty>

<owl:ObjectProperty rdf:about="&sioc;creator_of">
  <rdfs:label xml:lang="en">creator_of</rdfs:label>
  <owl:inverseOf rdf:resource="&sioc;has_creator"/>
  <rdfs:comment xml:lang="en">A resource that the User is a creator of.</rdfs:comment>
  <rdfs:domain rdf:resource="&sioc;User"/>
</owl:ObjectProperty>

<owl:TransitiveProperty rdf:about="&sioc;earlier_version">
  <rdfs:comment xml:lang="en">Links to a previous (older) revision of this Item or Post.</rdfs:comment>
  <rdfs:domain rdf:resource="&sioc;Item"/>
  <rdfs:label xml:lang="en">earlier_version</rdfs:label>
  <rdfs:range rdf:resource="&sioc;Item"/>
  <owl:inverseOf rdf:resource="&sioc;later_version"/>
</owl:TransitiveProperty>

<owl:ObjectProperty rdf:about="&sioc;email">
  <rdfs:label xml:lang="en">email</rdfs:label>
  <rdfs:comment xml:lang="en">An electronic mail address of the User.</rdfs:comment>
  <rdfs:domain rdf:resource="&sioc;User"/>
</owl:ObjectProperty>

<owl:DatatypeProperty rdf:about="&sioc;email_sha1">
  <rdfs:label xml:lang="en">email_sha1</rdfs:label>
  <rdfs:comment xml:lang="en">An electronic mail address of the User, encoded using SHA1.</rdfs:comment>
  <rdfs:domain rdf:resource="&sioc;User"/>
  <rdfs:range rdf:resource="http://www.w3.org/2000/01/rdf-schema#Literal"/>
</owl:DatatypeProperty>

<owl:ObjectProperty rdf:about="&sioc;feed">
  <rdfs:label xml:lang="en">feed</rdfs:label>
  <rdfs:comment xml:lang="en">A feed (e.g. RSS, Atom, etc.) pertaining to this resource (e.g. for a Forum, Site, User, etc.).</rdfs:comment>
</owl:ObjectProperty>

<owl:DatatypeProperty rdf:about="&sioc;follows">
  <rdfs:label xml:lang="en">follows</rdfs:label>
  <rdfs:comment xml:lang="en">Indicates that one User follows another User (e.g. for microblog posts or other content item updates).</rdfs:comment>
  <rdfs:domain rdf:resource="&sioc;User"/>
  <rdfs:range rdf:resource="&sioc;User"/>
</owl:DatatypeProperty>

<!-- @@todo: moving this property to the access module ? -->
<owl:ObjectProperty rdf:about="&sioc;function_of">
  <rdfs:label xml:lang="en">function_of</rdfs:label>
  <owl:inverseOf rdf:resource="&sioc;has_function"/>
  <rdfs:comment xml:lang="en">A User who has this Role.</rdfs:comment>
  <rdfs:domain rdf:resource="&sioc;Role"/>
</owl:ObjectProperty>

<owl:ObjectProperty rdf:about="&sioc;has_administrator">
  <rdfs:label xml:lang="en">has_administrator</rdfs:label>
  <owl:inverseOf rdf:resource="&sioc;administrator_of"/>
  <rdfs:comment xml:lang="en">A User who is an administrator of this Site.</rdfs:comment>
  <rdfs:domain rdf:resource="&sioc;Site"/>
  <rdfs:range rdf:resource="&sioc;User"/>
</owl:ObjectProperty>

<owl:ObjectProperty rdf:about="&sioc;has_container">
  <rdfs:label xml:lang="en">has_container</rdfs:label>
  <owl:inverseOf rdf:resource="&sioc;container_of"/>
  <rdfs:comment xml:lang="en">The Container to which this Item belongs.</rdfs:comment>
  <rdfs:domain rdf:resource="&sioc;Item"/>
  <rdfs:range rdf:resource="&sioc;Container"/>
</owl:ObjectProperty>

<owl:ObjectProperty rdf:about="&sioc;has_creator">
  <rdfs:label xml:lang="en">has_creator</rdfs:label>
  <owl:inverseOf rdf:resource="&sioc;creator_of"/>
  <rdfs:comment xml:lang="en">This is the User who made this resource.</rdfs:comment>
  <rdfs:range rdf:resource="&sioc;User"/>
</owl:ObjectProperty>

<!-- @@todo: moving this property to the access module ? -->
<owl:ObjectProperty rdf:about="&sioc;has_function">
  <rdfs:label xml:lang="en">has_function</rdfs:label>
  <owl:inverseOf rdf:resource="&sioc;function_of"/>
  <rdfs:comment xml:lang="en">A Role that this User has.</rdfs:comment>
  <rdfs:range rdf:resource="&sioc;Role"/>
</owl:ObjectProperty>

<owl:ObjectProperty rdf:about="&sioc;has_host">
  <rdfs:label xml:lang="en">has_host</rdfs:label>
  <owl:inverseOf rdf:resource="&sioc;host_of"/>
  <rdfs:comment xml:lang="en">The Site that hosts this Forum.</rdfs:comment>
  <rdfs:domain rdf:resource="&sioc;Forum"/>
  <rdfs:range rdf:resource="&sioc;Site"/>
</owl:ObjectProperty>

<owl:ObjectProperty rdf:about="&sioc;has_member">
  <rdfs:label xml:lang="en">has_member</rdfs:label>
  <owl:inverseOf rdf:resource="&sioc;member_of"/>
  <rdfs:comment xml:lang="en">A User who is a member of this Usergroup.</rdfs:comment>
  <rdfs:domain rdf:resource="&sioc;Usergroup"/>
  <rdfs:range rdf:resource="&sioc;User"/>
</owl:ObjectProperty>

<!-- @@todo: moving this property to the access module ? -->
<owl:ObjectProperty rdf:about="&sioc;has_moderator">
  <rdfs:label xml:lang="en">has_moderator</rdfs:label>
  <rdf:type rdf:resource="http://www.w3.org/2002/07/owl#ObjectProperty"/>
  <rdfs:comment xml:lang="en">A User who is a moderator of this Forum.</rdfs:comment>
  <rdfs:domain rdf:resource="&sioc;Forum"/>
  <rdfs:range rdf:resource="&sioc;User"/>
</owl:ObjectProperty>

<owl:ObjectProperty rdf:about="&sioc;has_modifier">
  <rdfs:label xml:lang="en">has_modifier</rdfs:label>
  <owl:inverseOf rdf:resource="&sioc;modifier_of"/>
  <rdfs:comment xml:lang="en">A User who modified this Item.</rdfs:comment>
  <rdfs:domain rdf:resource="&sioc;Item"/>
  <rdfs:range rdf:resource="&sioc;User"/>
</owl:ObjectProperty>

<owl:ObjectProperty rdf:about="&sioc;has_owner">
  <rdfs:label xml:lang="en">has_owner</rdfs:label>
  <owl:inverseOf rdf:resource="&sioc;owner_of"/>
  <rdfs:comment xml:lang="en">A User that this resource is owned by.</rdfs:comment>
  <rdfs:range rdf:resource="&sioc;User"/>
</owl:ObjectProperty>

<owl:ObjectProperty rdf:about="&sioc;has_parent">
  <rdfs:label xml:lang="en">has_parent</rdfs:label>
  <owl:inverseOf rdf:resource="&sioc;parent_of"/>
  <rdfs:comment xml:lang="en">A Container or Forum that this Container or Forum is a child of.</rdfs:comment>
  <rdfs:domain rdf:resource="&sioc;Container"/>
  <rdfs:range rdf:resource="&sioc;Container"/>
</owl:ObjectProperty>

<owl:ObjectProperty rdf:about="&sioc;has_reply">
  <rdfs:label xml:lang="en">has_reply</rdfs:label>
  <owl:inverseOf rdf:resource="&sioc;reply_of"/>
  <rdfs:comment xml:lang="en">Points to an Item or Post that is a reply or response to this Item or Post.</rdfs:comment>
  <rdfs:domain rdf:resource="&sioc;Item"/>
  <rdfs:range rdf:resource="&sioc;Item"/>
</owl:ObjectProperty>

<!-- @@todo: moving this property to the access module ? -->
<owl:ObjectProperty rdf:about="&sioc;has_scope">
  <rdfs:label xml:lang="en">has_scope</rdfs:label>
  <owl:inverseOf rdf:resource="&sioc;scope_of"/>
  <rdfs:comment xml:lang="en">A resource that this Role applies to.</rdfs:comment>
  <rdfs:domain rdf:resource="&sioc;Role"/>
</owl:ObjectProperty>

<owl:ObjectProperty rdf:about="&sioc;has_space">
  <rdfs:label xml:lang="en">has_space</rdfs:label>
  <owl:inverseOf rdf:resource="&sioc;space_of"/>
  <rdfs:comment xml:lang="en">A data Space which this resource is a part of.</rdfs:comment>
  <rdfs:range rdf:resource="&sioc;Space"/>
</owl:ObjectProperty>

<owl:ObjectProperty rdf:about="&sioc;has_subscriber">
  <rdfs:label xml:lang="en">has_subscriber</rdfs:label>
  <owl:inverseOf rdf:resource="&sioc;subscriber_of"/>
  <rdfs:comment xml:lang="en">A User who is subscribed to this Container.</rdfs:comment>
  <rdfs:domain rdf:resource="&sioc;Container"/>
  <rdfs:range rdf:resource="&sioc;User"/>
  <rdfs:seeAlso rdf:resource="&sioc;feed"/>
</owl:ObjectProperty>

<owl:ObjectProperty rdf:about="&sioc;has_usergroup">
  <rdfs:label xml:lang="en">has_usergroup</rdfs:label>
  <owl:inverseOf rdf:resource="&sioc;usergroup_of"/>
  <rdfs:comment xml:lang="en">Points to a Usergroup that has certain access to this Space.</rdfs:comment>
  <rdfs:domain rdf:resource="&sioc;Space"/>
  <rdfs:range rdf:resource="&sioc;Usergroup"/>
</owl:ObjectProperty>

<owl:ObjectProperty rdf:about="&sioc;host_of">
  <rdfs:label xml:lang="en">host_of</rdfs:label>
  <owl:inverseOf rdf:resource="&sioc;has_host"/>
  <rdfs:comment xml:lang="en">A Forum that is hosted on this Site.</rdfs:comment>
  <rdfs:domain rdf:resource="&sioc;Site"/>
  <rdfs:range rdf:resource="&sioc;Forum"/>
</owl:ObjectProperty>

<owl:DatatypeProperty rdf:about="&sioc;id">
  <rdfs:label xml:lang="en">id</rdfs:label>
  <rdfs:comment xml:lang="en">An identifier of a SIOC concept instance. For example, a user ID. Must be unique for instances of each type of SIOC concept within the same site.</rdfs:comment>
  <rdfs:range rdf:resource="http://www.w3.org/2000/01/rdf-schema#Literal"/>
</owl:DatatypeProperty>

<owl:DatatypeProperty rdf:about="&sioc;ip_address">
  <rdfs:label xml:lang="en">ip_address</rdfs:label>
  <rdfs:comment xml:lang="en">The IP address used when creating this Item. This can be associated with a creator. Some wiki articles list the IP addresses for the creator or modifiers when the usernames are absent.</rdfs:comment>
  <rdfs:domain rdf:resource="&sioc;Item"/>
  <rdfs:range rdf:resource="http://www.w3.org/2000/01/rdf-schema#Literal"/>
</owl:DatatypeProperty>

<owl:TransitiveProperty rdf:about="&sioc;later_version">
  <rdfs:comment xml:lang="en">Links to a later (newer) revision of this Item or Post.</rdfs:comment>
  <rdfs:domain rdf:resource="&sioc;Item"/>
  <rdfs:label xml:lang="en">later_version</rdfs:label>
  <rdfs:range rdf:resource="&sioc;Item"/>
  <owl:inverseOf rdf:resource="&sioc;earlier_version"/>
</owl:TransitiveProperty>

<owl:ObjectProperty rdf:about="&sioc;latest_version">
  <rdfs:comment xml:lang="en">Links to the latest revision of this Item or Post.</rdfs:comment>
  <rdfs:domain rdf:resource="&sioc;Item"/>
  <rdfs:label xml:lang="en">latest_version</rdfs:label>
  <rdfs:range rdf:resource="&sioc;Item"/>
</owl:ObjectProperty>

<owl:ObjectProperty rdf:about="&sioc;link">
  <rdfs:label xml:lang="en">link</rdfs:label>
  <rdfs:comment xml:lang="en">A URI of a document which contains this SIOC object.</rdfs:comment>
</owl:ObjectProperty>

<owl:ObjectProperty rdf:about="&sioc;links_to">
  <rdfs:label xml:lang="en">links_to</rdfs:label>
  <rdfs:comment xml:lang="en">Links extracted from hyperlinks within a SIOC concept, e.g. Post or Site.</rdfs:comment>
  <rdfs:subPropertyOf rdf:resource="http://purl.org/dc/terms/references"/>
</owl:ObjectProperty>

<owl:ObjectProperty rdf:about="&sioc;member_of">
  <rdfs:label xml:lang="en">member_of</rdfs:label>
  <owl:inverseOf rdf:resource="&sioc;has_member"/>
  <rdfs:comment xml:lang="en">A Usergroup that this User is a member of.</rdfs:comment>
  <rdfs:domain rdf:resource="&sioc;User"/>
  <rdfs:range rdf:resource="&sioc;Usergroup"/>
</owl:ObjectProperty>

<owl:ObjectProperty rdf:about="&sioc;moderator_of">
  <rdfs:label xml:lang="en">moderator_of</rdfs:label>
  <owl:inverseOf rdf:resource="&sioc;has_moderator"/>
  <rdfs:comment xml:lang="en">A Forum that User is a moderator of.</rdfs:comment>
  <rdfs:domain rdf:resource="&sioc;User"/>
  <rdfs:range rdf:resource="&sioc;Forum"/>
</owl:ObjectProperty>

<owl:ObjectProperty rdf:about="&sioc;modifier_of">
  <rdfs:label xml:lang="en">modifier_of</rdfs:label>
  <owl:inverseOf rdf:resource="&sioc;has_modifier"/>
  <rdfs:comment xml:lang="en">An Item that this User has modified.</rdfs:comment>
  <rdfs:domain rdf:resource="&sioc;User"/>
  <rdfs:range rdf:resource="&sioc;Item"/>
</owl:ObjectProperty>

<owl:DatatypeProperty rdf:about="&sioc;name">
  <rdfs:label xml:lang="en">name</rdfs:label>
  <rdfs:comment xml:lang="en">The name of a SIOC instance, e.g. a username for a User, group name for a Usergroup, etc.</rdfs:comment>
  <rdfs:range rdf:resource="http://www.w3.org/2000/01/rdf-schema#Literal"/>
</owl:DatatypeProperty>

<owl:ObjectProperty rdf:about="&sioc;next_by_date">
  <rdfs:label xml:lang="en">next_by_date</rdfs:label>
  <owl:inverseOf rdf:resource="&sioc;previous_by_date"/>
  <rdfs:comment xml:lang="en">Next Item or Post in a given Container sorted by date.</rdfs:comment>
  <rdfs:domain rdf:resource="&sioc;Item"/>
  <rdfs:range rdf:resource="&sioc;Item"/>
</owl:ObjectProperty>

<owl:ObjectProperty rdf:about="&sioc;next_version">
  <rdfs:label xml:lang="en">next_version</rdfs:label>
  <owl:inverseOf rdf:resource="&sioc;previous_version"/>
  <rdfs:comment xml:lang="en">Links to the next revision of this Item or Post.</rdfs:comment>
  <rdfs:domain rdf:resource="&sioc;Item"/>
  <rdfs:range rdf:resource="&sioc;Item"/>
  <rdfs:subPropertyOf rdf:resource="&sioc;later_version"/>
</owl:ObjectProperty>

<owl:DatatypeProperty rdf:about="&sioc;note">
  <rdfs:label xml:lang="en">note</rdfs:label>
  <rdfs:comment xml:lang="en">A note associated with this resource, for example, if it has been edited by a User.</rdfs:comment>
  <rdfs:range rdf:resource="http://www.w3.org/2000/01/rdf-schema#Literal"/>
</owl:DatatypeProperty>

<owl:DatatypeProperty rdf:about="&sioc;num_replies">
  <rdfs:label xml:lang="en">num_replies</rdfs:label>
  <rdfs:comment xml:lang="en">The number of replies that this Item, Thread, Post, etc. has. Useful for when the reply structure is absent.</rdfs:comment>
  <rdfs:range rdf:resource="http://www.w3.org/2001/XMLSchema#integer"/>
</owl:DatatypeProperty>

<owl:DatatypeProperty rdf:about="&sioc;num_views">
  <rdfs:label xml:lang="en">num_views</rdfs:label>
  <rdfs:comment xml:lang="en">The number of times this Item, Thread, User profile, etc. has been viewed.</rdfs:comment>
  <rdfs:range rdf:resource="http://www.w3.org/2001/XMLSchema#integer"/>
</owl:DatatypeProperty>

<owl:ObjectProperty rdf:about="&sioc;owner_of">
  <rdfs:label xml:lang="en">owner_of</rdfs:label>
  <owl:inverseOf rdf:resource="&sioc;has_owner"/>
  <rdfs:comment xml:lang="en">A resource owned by a particular User, for example, a weblog or image gallery.</rdfs:comment>
  <rdfs:domain rdf:resource="&sioc;User"/>
</owl:ObjectProperty>

<owl:ObjectProperty rdf:about="&sioc;parent_of">
  <rdfs:label xml:lang="en">parent_of</rdfs:label>
  <owl:inverseOf rdf:resource="&sioc;has_parent"/>
  <rdfs:comment xml:lang="en">A child Container or Forum that this Container or Forum is a parent of.</rdfs:comment>
  <rdfs:domain rdf:resource="&sioc;Container"/>
  <rdfs:range rdf:resource="&sioc;Container"/>
</owl:ObjectProperty>

<owl:ObjectProperty rdf:about="&sioc;previous_by_date">
  <rdfs:label xml:lang="en">previous_by_date</rdfs:label>
  <owl:inverseOf rdf:resource="&sioc;next_by_date"/>
  <rdfs:comment xml:lang="en">Previous Item or Post in a given Container sorted by date.</rdfs:comment>
  <rdfs:domain rdf:resource="&sioc;Item"/>
  <rdfs:range rdf:resource="&sioc;Item"/>
</owl:ObjectProperty>

<owl:ObjectProperty rdf:about="&sioc;previous_version">
  <rdfs:label xml:lang="en">previous_version</rdfs:label>
  <owl:inverseOf rdf:resource="&sioc;next_version"/>
  <rdfs:comment xml:lang="en">Links to the previous revision of this Item or Post.</rdfs:comment>
  <rdfs:domain rdf:resource="&sioc;Item"/>
  <rdfs:range rdf:resource="&sioc;Item"/>
  <rdfs:subPropertyOf rdf:resource="&sioc;earlier_version"/>
</owl:ObjectProperty>

<owl:ObjectProperty rdf:about="&sioc;related_to">
  <rdfs:label xml:lang="en">related_to</rdfs:label>
  <rdf:type rdf:resource="http://www.w3.org/2002/07/owl#ObjectProperty"/>
  <rdfs:comment xml:lang="en">Related Posts for this Post, perhaps determined implicitly from topics or references.</rdfs:comment>
</owl:ObjectProperty>

<owl:ObjectProperty rdf:about="&sioc;reply_of">
  <rdfs:label xml:lang="en">reply_of</rdfs:label>
  <owl:inverseOf rdf:resource="&sioc;has_reply"/>
  <rdfs:comment xml:lang="en">Links to an Item or Post which this Item or Post is a reply to.</rdfs:comment>
  <rdfs:domain rdf:resource="&sioc;Item"/>
  <rdfs:range rdf:resource="&sioc;Item"/>
</owl:ObjectProperty>

<!-- @@todo: moving this property to the access module ? -->
<owl:ObjectProperty rdf:about="&sioc;scope_of">
  <rdfs:label xml:lang="en">scope_of</rdfs:label>
  <owl:inverseOf rdf:resource="&sioc;has_scope"/>
  <rdfs:comment xml:lang="en">A Role that has a scope of this resource.</rdfs:comment>
  <rdfs:range rdf:resource="&sioc;Role"/>
</owl:ObjectProperty>

<owl:SymmetricProperty rdf:about="&sioc;sibling">
  <rdfs:label xml:lang="en">sibling</rdfs:label>
  <rdfs:comment xml:lang="en">An Item may have a sibling or a twin that exists in a different Container, but the siblings may differ in some small way (for example, language, category, etc.). The sibling of this Item should be self-describing (that is, it should contain all available information).</rdfs:comment>
  <rdfs:domain rdf:resource="&sioc;Item"/>
  <rdfs:range rdf:resource="&sioc;Item"/>
</owl:SymmetricProperty>

<owl:ObjectProperty rdf:about="&sioc;space_of">
  <rdfs:label xml:lang="en">space_of</rdfs:label>
  <owl:inverseOf rdf:resource="&sioc;has_space"/>
  <rdfs:comment xml:lang="en">A resource which belongs to this data Space.</rdfs:comment>
  <rdfs:domain rdf:resource="&sioc;Space"/>
</owl:ObjectProperty>

<owl:ObjectProperty rdf:about="&sioc;subscriber_of">
  <rdfs:label xml:lang="en">subscriber_of</rdfs:label>
  <owl:inverseOf rdf:resource="&sioc;has_subscriber"/>
  <rdfs:comment xml:lang="en">A Container that a User is subscribed to.</rdfs:comment>
  <rdfs:domain rdf:resource="&sioc;User"/>
  <rdfs:range rdf:resource="&sioc;Container"/>
  <rdfs:seeAlso rdf:resource="&sioc;feed"/>
</owl:ObjectProperty>

<owl:ObjectProperty rdf:about="&sioc;topic">
  <rdfs:label xml:lang="en">topic</rdfs:label>
  <rdfs:comment xml:lang="en">A topic of interest, linking to the appropriate URI, e.g. in the Open Directory Project or of a SKOS category.</rdfs:comment>
  <rdfs:subPropertyOf rdf:resource="http://purl.org/dc/terms/subject"/>
</owl:ObjectProperty>

<owl:ObjectProperty rdf:about="&sioc;usergroup_of">
  <rdfs:label xml:lang="en">usergroup_of</rdfs:label>
  <owl:inverseOf rdf:resource="&sioc;has_usergroup"/>
  <rdfs:comment xml:lang="en">A Space that the Usergroup has access to.</rdfs:comment>
  <rdfs:domain rdf:resource="&sioc;Usergroup"/>
  <rdfs:range rdf:resource="&sioc;Space"/>
</owl:ObjectProperty>

<!-- SIOC TYPES -->


<!-- Classes -->

<!-- Subtypes of sioc:Container -->

<rdf:Description rdf:about="http://rdfs.org/sioc/types#AddressBook">
  <rdfs:label xml:lang="en">Address Book</rdfs:label>
  <rdfs:comment xml:lang="en">Describes a collection of personal or organisational addresses.</rdfs:comment>
  <rdfs:isDefinedBy rdf:resource="http://rdfs.org/sioc/types#"/>
  <rdfs:seeAlso rdf:resource="http://xmlns.com/foaf/0.1/Agent"/>
</rdf:Description>

<rdf:Description rdf:about="http://rdfs.org/sioc/types#AnnotationSet">
  <rdfs:label xml:lang="en">Annotation Set</rdfs:label>
  <rdfs:comment xml:lang="en">Describes a set of annotations, for example, those created by a particular user or related to a particular topic.</rdfs:comment>

  <rdfs:isDefinedBy rdf:resource="http://rdfs.org/sioc/types#"/>
  <rdfs:seeAlso rdf:resource="http://www.w3.org/2000/10/annotation-ns#Annotation"/>
</rdf:Description>

<rdf:Description rdf:about="http://rdfs.org/sioc/types#AudioChannel">
  <rdfs:label xml:lang="en">Audio Channel</rdfs:label>
  <rdfs:comment xml:lang="en">Describes a channel for distributing audio or sound files, for example, a podcast.</rdfs:comment>

  <rdfs:isDefinedBy rdf:resource="http://rdfs.org/sioc/types#"/>
  <rdfs:seeAlso rdf:resource="http://purl.org/dc/dcmitype/Sound"/>
</rdf:Description>

<rdf:Description rdf:about="http://rdfs.org/sioc/types#BookmarkFolder">
  <rdfs:label xml:lang="en">Bookmark Folder</rdfs:label>
  <rdfs:comment xml:lang="en">Describes a shared collection of bookmarks.</rdfs:comment>

  <rdfs:isDefinedBy rdf:resource="http://rdfs.org/sioc/types#"/>
  <rdfs:seeAlso rdf:resource="http://www.w3.org/2002/01/bookmark#Bookmark"/>
</rdf:Description>

<rdf:Description rdf:about="http://rdfs.org/sioc/types#Briefcase">
  <rdfs:label xml:lang="en">Briefcase</rdfs:label>
  <rdfs:comment xml:lang="en">Describes a briefcase or file service.</rdfs:comment>

  <rdfs:isDefinedBy rdf:resource="http://rdfs.org/sioc/types#"/>
  <rdfs:seeAlso rdf:resource="http://xmlns.com/foaf/0.1/Document"/>
</rdf:Description>

<rdf:Description rdf:about="http://rdfs.org/sioc/types#EventCalendar">
  <rdfs:label xml:lang="en">Event Calendar</rdfs:label>
  <rdfs:comment xml:lang="en">Describes a calendar of events.</rdfs:comment>

  <rdfs:isDefinedBy rdf:resource="http://rdfs.org/sioc/types#"/>
  <rdfs:seeAlso rdf:resource="http://www.w3.org/2002/12/cal/icaltzd#VEVENT"/>
</rdf:Description>

<rdf:Description rdf:about="http://rdfs.org/sioc/types#ImageGallery">
  <rdfs:label xml:lang="en">Image Gallery</rdfs:label>
  <rdfs:comment xml:lang="en">Describes an image gallery, for example, a photo album.</rdfs:comment>

  <rdfs:isDefinedBy rdf:resource="http://rdfs.org/sioc/types#"/>
  <rdfs:seeAlso rdf:resource="http://www.w3.org/2003/12/exif/ns/IFD"/>
</rdf:Description>

<rdf:Description rdf:about="http://rdfs.org/sioc/types#ProjectDirectory">
  <rdfs:label xml:lang="en">Project Directory</rdfs:label>
  <rdfs:comment xml:lang="en">Describes a project directory.</rdfs:comment>

  <rdfs:isDefinedBy rdf:resource="http://rdfs.org/sioc/types#"/>
  <rdfs:seeAlso rdf:resource="http://usefulinc.com/ns/doap#Project"/>
</rdf:Description>

<rdf:Description rdf:about="http://rdfs.org/sioc/types#ResumeBank">
  <rdfs:label xml:lang="en">Resume Bank</rdfs:label>
  <rdfs:comment xml:lang="en">Describes a collection of resumes.</rdfs:comment>

  <rdfs:isDefinedBy rdf:resource="http://rdfs.org/sioc/types#"/>
  <rdfs:seeAlso rdf:resource="http://captsolo.net/semweb/resume/cv.rdfs#Resume"/>
</rdf:Description>

<rdf:Description rdf:about="http://rdfs.org/sioc/types#ReviewArea">
  <rdfs:label xml:lang="en">Review Area</rdfs:label>
  <rdfs:comment xml:lang="en">Describes an area where reviews are posted.</rdfs:comment>

  <rdfs:isDefinedBy rdf:resource="http://rdfs.org/sioc/types#"/>
  <rdfs:seeAlso rdf:resource="http://www.isi.edu/webscripter/communityreview/abstract-review-o#Review"/>
  <rdfs:seeAlso rdf:resource="http://dannyayers.com/xmlns/rev/#Review"/>
</rdf:Description>

<rdf:Description rdf:about="http://rdfs.org/sioc/types#SubscriptionList">
  <rdfs:label xml:lang="en">Subscription List</rdfs:label>
  <rdfs:comment xml:lang="en">Describes a shared set of feed subscriptions.</rdfs:comment>

  <rdfs:isDefinedBy rdf:resource="http://rdfs.org/sioc/types#"/>
  <rdfs:seeAlso rdf:resource="http://atomowl.org/ontologies/atomrdf#Feed"/>
</rdf:Description>

<rdf:Description rdf:about="http://rdfs.org/sioc/types#SurveyCollection">
  <rdfs:label xml:lang="en">Survey Collection</rdfs:label>
  <rdfs:comment xml:lang="en">Describes an area where survey data can be collected, e.g. from polls.</rdfs:comment>

  <rdfs:isDefinedBy rdf:resource="http://rdfs.org/sioc/types#"/>
  <rdfs:seeAlso rdf:resource="http://rdfs.org/sioc/types#Poll"/>  
</rdf:Description>

<rdf:Description rdf:about="http://rdfs.org/sioc/types#VideoChannel">
  <rdfs:label xml:lang="en">Video Channel</rdfs:label>
  <rdfs:comment xml:lang="en">Describes a channel for distributing videos (moving image) files, for example, a video podcast.</rdfs:comment>

  <rdfs:isDefinedBy rdf:resource="http://rdfs.org/sioc/types#"/>
  <rdfs:seeAlso rdf:resource="http://purl.org/dc/dcmitype/MovingImage"/>
</rdf:Description>

<rdf:Description rdf:about="http://rdfs.org/sioc/types#Wiki">
  <rdfs:label xml:lang="en">Wiki</rdfs:label>
  <rdfs:comment xml:lang="en">Describes a wiki space.</rdfs:comment>

  <rdfs:isDefinedBy rdf:resource="http://rdfs.org/sioc/types#"/>
  <rdfs:seeAlso rdf:resource="http://rdfs.org/sioc/types#WikiArticle"/>  
</rdf:Description>

<!-- Types of sioc:Container for creating lists -->

<rdf:Description rdf:about="http://rdfs.org/sioc/types#FavouriteThings">
  <rdfs:label xml:lang="en">Favourite Things</rdfs:label>
  <rdfs:comment xml:lang="en">Describes a list or a collection of one's favourite things.</rdfs:comment>

  <rdfs:isDefinedBy rdf:resource="http://rdfs.org/sioc/types#"/>
</rdf:Description>

<rdf:Description rdf:about="http://rdfs.org/sioc/types#OfferList">
  <rdfs:label xml:lang="en">Offer List</rdfs:label>
  <rdfs:comment xml:lang="en">Describes a list of the items someone has available to offer.</rdfs:comment>

  <rdfs:isDefinedBy rdf:resource="http://rdfs.org/sioc/types#"/>
</rdf:Description>

<rdf:Description rdf:about="http://rdfs.org/sioc/types#Playlist">
  <rdfs:label xml:lang="en">Playlist</rdfs:label>
  <rdfs:comment xml:lang="en">Describes a list of media items that have been played or can be played.</rdfs:comment>

  <rdfs:isDefinedBy rdf:resource="http://rdfs.org/sioc/types#"/>
</rdf:Description>

<rdf:Description rdf:about="http://rdfs.org/sioc/types#ReadingList">
  <rdfs:label xml:lang="en">Reading List</rdfs:label>
  <rdfs:comment xml:lang="en">Describes a list of books or other materials that have been read or are suggested for reading.</rdfs:comment>

  <rdfs:isDefinedBy rdf:resource="http://rdfs.org/sioc/types#"/>
</rdf:Description>

<rdf:Description rdf:about="http://rdfs.org/sioc/types#WishList">
  <rdfs:label xml:lang="en">Wish List</rdfs:label>
  <rdfs:comment xml:lang="en">Describes a list of the items someone wishes to get.</rdfs:comment>

  <rdfs:isDefinedBy rdf:resource="http://rdfs.org/sioc/types#"/>
</rdf:Description>

<!-- Subtypes of sioc:Forum -->

<rdf:Description rdf:about="http://rdfs.org/sioc/types#ArgumentativeDiscussion">
  <rdfs:label xml:lang="en">Argumentative Discussion</rdfs:label>
  <rdfs:comment xml:lang="en">Describes a discussion area where logical arguments can take place.</rdfs:comment>

  <rdfs:isDefinedBy rdf:resource="http://rdfs.org/sioc/types#"/>
  <rdfs:seeAlso rdf:resource="http://purl.org/ibis#Idea"/>
</rdf:Description>

<rdf:Description rdf:about="http://rdfs.org/sioc/types#ChatChannel">
  <rdfs:label xml:lang="en">Chat Channel</rdfs:label>
  <rdfs:comment xml:lang="en">Describes a channel for chat or instant messages, for example, via IRC or IM.</rdfs:comment>

  <rdfs:isDefinedBy rdf:resource="http://rdfs.org/sioc/types#"/>
  <rdfs:seeAlso rdf:resource="http://rdfs.org/sioc/types#InstantMessage"/>
</rdf:Description>

<rdf:Description rdf:about="http://rdfs.org/sioc/types#MailingList">
  <rdfs:label xml:lang="en">Mailing List</rdfs:label>
  <rdfs:comment xml:lang="en">Describes an electronic mailing list.</rdfs:comment>

  <rdfs:isDefinedBy rdf:resource="http://rdfs.org/sioc/types#"/>
  <rdfs:seeAlso rdf:resource="http://rdfs.org/sioc/types#MailMessage"/>
</rdf:Description>

<rdf:Description rdf:about="http://rdfs.org/sioc/types#MessageBoard">
  <rdfs:label xml:lang="en">Message Board</rdfs:label>
  <rdfs:comment xml:lang="en">Describes a message board, also known as an online bulletin board or discussion forum.</rdfs:comment>

  <rdfs:isDefinedBy rdf:resource="http://rdfs.org/sioc/types#"/>
  <rdfs:seeAlso rdf:resource="http://rdfs.org/sioc/types#BoardPost"/>
</rdf:Description>

<rdf:Description rdf:about="http://rdfs.org/sioc/types#Microblog">
  <rdfs:label xml:lang="en">Microblog</rdfs:label>
  <rdfs:comment xml:lang="en">Describes a microblog, i.e. a blog consisting of short text messages.</rdfs:comment>

  <rdfs:isDefinedBy rdf:resource="http://rdfs.org/sioc/types#"/>
  <rdfs:seeAlso rdf:resource="http://rdfs.org/sioc/types#MicroblogPost"/>
</rdf:Description>

<rdf:Description rdf:about="http://rdfs.org/sioc/types#Weblog">
  <rdfs:label xml:lang="en">Weblog</rdfs:label>
  <rdfs:comment xml:lang="en">Describes a weblog (blog), i.e. an online journal.</rdfs:comment>

  <rdfs:isDefinedBy rdf:resource="http://rdfs.org/sioc/types#"/>
  <rdfs:seeAlso rdf:resource="http://rdfs.org/sioc/types#BlogPost"/>
</rdf:Description>

<!-- Subtypes of sioc:Item -->

<rdf:Description rdf:about="http://rdfs.org/sioc/types#Poll">
  <rdfs:label xml:lang="en">Poll</rdfs:label>
  <rdfs:comment xml:lang="en">Describes a posted item that contains a poll or survey content.</rdfs:comment>

  <rdfs:isDefinedBy rdf:resource="http://rdfs.org/sioc/types#"/>
  <rdfs:seeAlso rdf:resource="http://rdfs.org/sioc/types#SurveyCollection"/>
</rdf:Description>

<!-- Subtypes of sioc:Post -->

<rdf:Description rdf:about="http://rdfs.org/sioc/types#BlogPost">
  <rdfs:label xml:lang="en">Blog Post</rdfs:label>
  <rdfs:comment xml:lang="en">Describes a post that is specifically made on a weblog.</rdfs:comment>

  <rdfs:isDefinedBy rdf:resource="http://rdfs.org/sioc/types#"/>
  <rdfs:seeAlso rdf:resource="http://rdfs.org/sioc/types#Weblog"/>
</rdf:Description>

<rdf:Description rdf:about="http://rdfs.org/sioc/types#BoardPost">
  <rdfs:label xml:lang="en">Board Post</rdfs:label>
  <rdfs:comment xml:lang="en">Describes a post that is specifically made on a message board.</rdfs:comment>

  <rdfs:isDefinedBy rdf:resource="http://rdfs.org/sioc/types#"/>
  <rdfs:seeAlso rdf:resource="http://rdfs.org/sioc/types#MessageBoard"/>
</rdf:Description>

<rdf:Description rdf:about="http://rdfs.org/sioc/types#Comment">
  <rdfs:label xml:lang="en">Comment</rdfs:label>
  <rdfs:comment xml:lang="en">Comment is a subtype of sioc:Post and allows one to explicitly indicate that this SIOC post is a comment.  Note that comments have a narrower scope than sioc:Post and may not apply to all types of community site.</rdfs:comment>

  <rdfs:isDefinedBy rdf:resource="http://rdfs.org/sioc/types#"/>
  <rdfs:seeAlso rdf:resource="http://rdfs.org/sioc/types#Forum"/>
</rdf:Description>

<rdf:Description rdf:about="http://rdfs.org/sioc/types#InstantMessage">
  <rdfs:label xml:lang="en">Instant Message</rdfs:label>
  <rdfs:comment xml:lang="en">Describes an instant message, e.g. sent via Jabber.</rdfs:comment>

  <rdfs:isDefinedBy rdf:resource="http://rdfs.org/sioc/types#"/>
  <rdfs:seeAlso rdf:resource="http://rdfs.org/sioc/types#ChatChannel"/>
</rdf:Description>

<rdf:Description rdf:about="http://rdfs.org/sioc/types#MailMessage">
  <rdfs:label xml:lang="en">Mail Message</rdfs:label>
  <rdfs:comment xml:lang="en">Describes an electronic mail message, e.g. a post sent to a mailing list.</rdfs:comment>

  <rdfs:isDefinedBy rdf:resource="http://rdfs.org/sioc/types#"/>
  <rdfs:seeAlso rdf:resource="http://rdfs.org/sioc/types#MailingList"/>
</rdf:Description>

<rdf:Description rdf:about="http://rdfs.org/sioc/types#MicroblogPost">
  <rdfs:label xml:lang="en">Microblog Post</rdfs:label>
  <rdfs:comment xml:lang="en">Describes a post that is specifically made on a microblog.</rdfs:comment>

  <rdfs:isDefinedBy rdf:resource="http://rdfs.org/sioc/types#"/>
  <rdfs:seeAlso rdf:resource="http://rdfs.org/sioc/types#Microblog"/>
</rdf:Description>

<rdf:Description rdf:about="http://rdfs.org/sioc/types#WikiArticle">
  <rdfs:label xml:lang="en">Wiki Article</rdfs:label>
  <rdfs:comment xml:lang="en">Describes a wiki article.</rdfs:comment>

  <rdfs:isDefinedBy rdf:resource="http://rdfs.org/sioc/types#"/>
  <rdfs:seeAlso rdf:resource="http://rdfs.org/sioc/types#Wiki"/>
</rdf:Description>

<!-- Subtypes of sioc:Post for question and answer sites -->

<rdf:Description rdf:about="http://rdfs.org/sioc/types#Answer">
  <rdfs:label xml:lang="en">Answer</rdfs:label>
  <rdfs:comment xml:lang="en">A Post that provides an answer in reply to a Question.</rdfs:comment>

  <rdfs:isDefinedBy rdf:resource="http://rdfs.org/sioc/types#"/>
</rdf:Description>

<rdf:Description rdf:about="http://rdfs.org/sioc/types#BestAnswer">
  <rdfs:label xml:lang="en">Best Answer</rdfs:label>
  <rdfs:comment xml:lang="en">A Post that is the best answer to a Question, as chosen by the User who asked the Question or as voted by a Community of Users.</rdfs:comment>

  <rdfs:isDefinedBy rdf:resource="http://rdfs.org/sioc/types#"/>
</rdf:Description>

<rdf:Description rdf:about="http://rdfs.org/sioc/types#Question">
  <rdfs:label xml:lang="en">Question</rdfs:label>
  <rdfs:comment xml:lang="en">A Post that asks a Question.</rdfs:comment>

  <rdfs:isDefinedBy rdf:resource="http://rdfs.org/sioc/types#"/>
</rdf:Description>

<!-- Types of sioc:topic for defining some different ways used to classify things in online communities -->

<rdf:Description rdf:about="http://rdfs.org/sioc/types#Category">
  <rdfs:label xml:lang="en">Category</rdfs:label>
  <rdfs:comment xml:lang="en">Category is used on the object of sioc:topic to indicate that this resource is a category on a site.</rdfs:comment>
  <rdfs:isDefinedBy rdf:resource="http://rdfs.org/sioc/types#"/>

</rdf:Description>
  
<rdf:Description rdf:about="http://rdfs.org/sioc/types#Tag">
  <rdfs:label xml:lang="en">Tag</rdfs:label>
  <rdfs:comment xml:lang="en">Tag is used on the object of sioc:topic to indicate that this resource is a tag on a site.</rdfs:comment>
  <rdfs:isDefinedBy rdf:resource="http://rdfs.org/sioc/types#"/>
</rdf:Description>



<!-- GEO -->

<rdf:Description rdf:about="http://www.w3.org/2003/01/geo/wgs84_pos#SpatialThing">
 <rdfs:label>SpatialThing</rdfs:label>
 <rdfs:comment>Anything with spatial extent, i.e. size, shape, or position. e.g. people, places, bowling balls, as well as abstract areas like cubes.
</rdfs:comment>
</rdf:Description>


<rdf:Description rdf:about="http://www.w3.org/2003/01/geo/wgs84_pos#Point">

 <rdfs:label>Point</rdfs:label>
 <rdfs:comment>A point, typically described using a coordinate system relative to Earth, such as WGS84.
</rdfs:comment>

<rdfs:comment>
Uniquely identified by lat/long/alt. i.e.

spaciallyIntersects(P1, P2) :- lat(P1, LAT), long(P1, LONG), alt(P1, ALT),
  lat(P2, LAT), long(P2, LONG), alt(P2, ALT).

sameThing(P1, P2) :- type(P1, Point), type(P2, Point), spaciallyIntersects(P1, P2).
</rdfs:comment>
</rdf:Description>


<rdf:Property rdf:about="http://www.w3.org/2003/01/geo/wgs84_pos#lat">
 <rdfs:domain rdf:resource="http://www.w3.org/2003/01/geo/wgs84_pos#SpatialThing" />
 <rdfs:label>latitude</rdfs:label>
 <rdfs:comment>The WGS84 latitude of a SpatialThing (decimal degrees).</rdfs:comment>
</rdf:Property>

<rdf:Property rdf:about="http://www.w3.org/2003/01/geo/wgs84_pos#long">
 <rdfs:domain rdf:resource="http://www.w3.org/2003/01/geo/wgs84_pos#SpatialThing" />
 <rdfs:label>longitude</rdfs:label>
 <rdfs:comment>The WGS84 longitude of a SpatialThing (decimal degrees).</rdfs:comment>
</rdf:Property>

<rdf:Property rdf:about="http://www.w3.org/2003/01/geo/wgs84_pos#alt">
 <rdfs:domain rdf:resource="http://www.w3.org/2003/01/geo/wgs84_pos#SpatialThing" />
 <rdfs:label>altitude</rdfs:label>
 <rdfs:comment>The WGS84 altitude of a SpatialThing (decimal meters 
above the local reference ellipsoid).</rdfs:comment>
</rdf:Property>

<!-- not sure we really need this -->
<rdf:Property rdf:about="http://www.w3.org/2003/01/geo/wgs84_pos#lat_long">
 <rdfs:label>lat/long</rdfs:label>
 <rdfs:comment>A comma-separated representation of a latitude, longitude coordinate.</rdfs:comment>
</rdf:Property>


<!-- RELATIONSHIP -->


  <rdf:Description rdf:about="http://purl.org/vocab/relationship/friendOf">
    <rdf:type rdf:resource="http://www.w3.org/2002/07/owl#SymmetricProperty"/>
    <owl:equivalentClass rdf:resource="http://www.perceive.net/schemas/relationship/friendOf"/>
    <rdfs:subPropertyOf rdf:resource="http://xmlns.com/foaf/0.1/knows"/>
    <rdfs:label xml:lang="en">friend of</rdfs:label>
    <skos:definition xml:lang="en">A person who shares mutual friendship with this person.</skos:definition>
    <rdfs:domain rdf:resource="http://xmlns.com/foaf/0.1/Person"/>
    <rdfs:range rdf:resource="http://xmlns.com/foaf/0.1/Person"/>
    <rdfs:isDefinedBy rdf:resource="http://purl.org/vocab/relationship/"/>
  </rdf:Description>

  <rdf:Description rdf:about="http://purl.org/vocab/relationship/acquaintanceOf">
    <rdf:type rdf:resource="http://www.w3.org/2002/07/owl#SymmetricProperty"/>
    <owl:equivalentClass rdf:resource="http://www.perceive.net/schemas/relationship/acquaintanceOf"/>
    <rdfs:subPropertyOf rdf:resource="http://xmlns.com/foaf/0.1/knows"/>
    <rdfs:label xml:lang="en">acquaintance of</rdfs:label>
    <skos:definition xml:lang="en">A person having more than slight or superficial knowledge of this person but short of friendship.</skos:definition>
    <rdfs:domain rdf:resource="http://xmlns.com/foaf/0.1/Person"/>
    <rdfs:range rdf:resource="http://xmlns.com/foaf/0.1/Person"/>
    <rdfs:isDefinedBy rdf:resource="http://purl.org/vocab/relationship/"/>
  </rdf:Description>

  <rdf:Description rdf:about="http://purl.org/vocab/relationship/parentOf">
    <rdf:type rdf:resource="http://www.w3.org/1999/02/22-rdf-syntax-ns#Property"/>
    <owl:equivalentClass rdf:resource="http://www.perceive.net/schemas/relationship/parentOf"/>
    <owl:inverseOf rdf:resource="http://purl.org/vocab/relationship/childOf"/>
    <rdfs:subPropertyOf rdf:resource="http://xmlns.com/foaf/0.1/knows"/>
    <rdfs:label xml:lang="en">parent of</rdfs:label>
    <skos:definition xml:lang="en">A person who has given birth to or nurtured and raised this person.</skos:definition>
    <rdfs:domain rdf:resource="http://xmlns.com/foaf/0.1/Person"/>
    <rdfs:range rdf:resource="http://xmlns.com/foaf/0.1/Person"/>
    <rdfs:isDefinedBy rdf:resource="http://purl.org/vocab/relationship/"/>
  </rdf:Description>

  <rdf:Description rdf:about="http://purl.org/vocab/relationship/siblingOf">
    <rdf:type rdf:resource="http://www.w3.org/2002/07/owl#SymmetricProperty"/>
    <owl:equivalentClass rdf:resource="http://www.perceive.net/schemas/relationship/siblingOf"/>
    <rdfs:subPropertyOf rdf:resource="http://xmlns.com/foaf/0.1/knows"/>
    <rdfs:label xml:lang="en">sibling of</rdfs:label>
    <skos:definition xml:lang="en">A person having one or both parents in common with this person.</skos:definition>
    <rdfs:domain rdf:resource="http://xmlns.com/foaf/0.1/Person"/>
    <rdfs:range rdf:resource="http://xmlns.com/foaf/0.1/Person"/>
    <rdfs:isDefinedBy rdf:resource="http://purl.org/vocab/relationship/"/>
  </rdf:Description>

  <rdf:Description rdf:about="http://purl.org/vocab/relationship/childOf">
    <rdf:type rdf:resource="http://www.w3.org/1999/02/22-rdf-syntax-ns#Property"/>
    <owl:equivalentClass rdf:resource="http://www.perceive.net/schemas/relationship/childOf"/>
    <owl:inverseOf rdf:resource="http://purl.org/vocab/relationship/parentOf"/>
    <rdfs:subPropertyOf rdf:resource="http://xmlns.com/foaf/0.1/knows"/>
    <rdfs:label xml:lang="en">child of</rdfs:label>
    <skos:definition xml:lang="en">A person who was given birth to or nurtured and raised by this person.</skos:definition>
    <rdfs:domain rdf:resource="http://xmlns.com/foaf/0.1/Person"/>
    <rdfs:range rdf:resource="http://xmlns.com/foaf/0.1/Person"/>
    <rdfs:isDefinedBy rdf:resource="http://purl.org/vocab/relationship/"/>
  </rdf:Description>

  <rdf:Description rdf:about="http://purl.org/vocab/relationship/grandchildOf">
    <rdf:type rdf:resource="http://www.w3.org/1999/02/22-rdf-syntax-ns#Property"/>
    <owl:equivalentClass rdf:resource="http://www.perceive.net/schemas/relationship/grandchildOf"/>
    <owl:inverseOf rdf:resource="http://purl.org/vocab/relationship/grandparentOf"/>
    <rdfs:subPropertyOf rdf:resource="http://xmlns.com/foaf/0.1/knows"/>
    <rdfs:label xml:lang="en">grandchild of</rdfs:label>
    <rdfs:label>Grandchild Of</rdfs:label>
    <skos:definition xml:lang="en">A person who is a child of any of this person's children.</skos:definition>
    <rdfs:domain rdf:resource="http://xmlns.com/foaf/0.1/Person"/>
    <rdfs:range rdf:resource="http://xmlns.com/foaf/0.1/Person"/>
    <rdfs:isDefinedBy rdf:resource="http://purl.org/vocab/relationship/"/>
  </rdf:Description>

  <rdf:Description rdf:about="http://purl.org/vocab/relationship/spouseOf">
    <rdf:type rdf:resource="http://www.w3.org/2002/07/owl#SymmetricProperty"/>
    <owl:equivalentClass rdf:resource="http://www.perceive.net/schemas/relationship/spouseOf"/>
    <rdfs:subPropertyOf rdf:resource="http://xmlns.com/foaf/0.1/knows"/>
    <rdfs:label xml:lang="en">spouse of</rdfs:label>
    <skos:definition xml:lang="en">A person who is married to this person</skos:definition>
    <rdfs:range rdf:resource="http://xmlns.com/foaf/0.1/Person"/>
    <rdfs:isDefinedBy rdf:resource="http://purl.org/vocab/relationship/"/>
  </rdf:Description>

  <rdf:Description rdf:about="http://purl.org/vocab/relationship/enemyOf">
    <rdf:type rdf:resource="http://www.w3.org/1999/02/22-rdf-syntax-ns#Property"/>
    <owl:equivalentClass rdf:resource="http://www.perceive.net/schemas/relationship/enemyOf"/>
    <rdfs:subPropertyOf rdf:resource="http://xmlns.com/foaf/0.1/knows"/>
    <rdfs:label xml:lang="en">enemy of</rdfs:label>
    <skos:definition xml:lang="en">A person towards whom this person feels hatred, intends injury to, or opposes the interests of.</skos:definition>
    <rdfs:domain rdf:resource="http://xmlns.com/foaf/0.1/Person"/>
    <rdfs:range rdf:resource="http://xmlns.com/foaf/0.1/Person"/>
    <rdfs:isDefinedBy rdf:resource="http://purl.org/vocab/relationship/"/>
  </rdf:Description>

  <rdf:Description rdf:about="http://purl.org/vocab/relationship/antagonistOf">
    <rdf:type rdf:resource="http://www.w3.org/1999/02/22-rdf-syntax-ns#Property"/>
    <owl:equivalentClass rdf:resource="http://www.perceive.net/schemas/relationship/antagonistOf"/>
    <rdfs:subPropertyOf rdf:resource="http://xmlns.com/foaf/0.1/knows"/>
    <rdfs:label xml:lang="en">antagonist of</rdfs:label>
    <skos:definition xml:lang="en">A person who opposes and contends against this person.</skos:definition>
    <rdfs:domain rdf:resource="http://xmlns.com/foaf/0.1/Person"/>
    <rdfs:range rdf:resource="http://xmlns.com/foaf/0.1/Person"/>
    <rdfs:isDefinedBy rdf:resource="http://purl.org/vocab/relationship/"/>
  </rdf:Description>

  <rdf:Description rdf:about="http://purl.org/vocab/relationship/ambivalentOf">
    <rdf:type rdf:resource="http://www.w3.org/1999/02/22-rdf-syntax-ns#Property"/>
    <owl:equivalentClass rdf:resource="http://www.perceive.net/schemas/relationship/ambivalentOf"/>
    <rdfs:subPropertyOf rdf:resource="http://xmlns.com/foaf/0.1/knows"/>
    <rdfs:label xml:lang="en">ambivalent of</rdfs:label>
    <skos:definition xml:lang="en">A person towards whom this person has mixed feelings or emotions.</skos:definition>
    <rdfs:domain rdf:resource="http://xmlns.com/foaf/0.1/Person"/>
    <rdfs:range rdf:resource="http://xmlns.com/foaf/0.1/Person"/>
    <rdfs:isDefinedBy rdf:resource="http://purl.org/vocab/relationship/"/>
  </rdf:Description>

  <rdf:Description rdf:about="http://purl.org/vocab/relationship/lostContactWith">
    <rdf:type rdf:resource="http://www.w3.org/2002/07/owl#SymmetricProperty"/>
    <rdfs:subPropertyOf rdf:resource="http://xmlns.com/foaf/0.1/knows"/>
    <rdfs:label xml:lang="en">lost contact with</rdfs:label>
    <skos:definition xml:lang="en">A person who was once known by this person but has subsequently become uncontactable.</skos:definition>
    <rdfs:domain rdf:resource="http://xmlns.com/foaf/0.1/Person"/>
    <rdfs:range rdf:resource="http://xmlns.com/foaf/0.1/Person"/>
    <rdfs:isDefinedBy rdf:resource="http://purl.org/vocab/relationship/"/>
  </rdf:Description>

  <rdf:Description rdf:about="http://purl.org/vocab/relationship/knowsOf">
    <rdf:type rdf:resource="http://www.w3.org/1999/02/22-rdf-syntax-ns#Property"/>
    <rdfs:subPropertyOf rdf:resource="http://xmlns.com/foaf/0.1/knows"/>
    <rdfs:label xml:lang="en">knows of</rdfs:label>
    <skos:definition xml:lang="en">A person who has come to be known to this person through their actions or position.</skos:definition>
    <rdfs:domain rdf:resource="http://xmlns.com/foaf/0.1/Person"/>
    <rdfs:range rdf:resource="http://xmlns.com/foaf/0.1/Person"/>
    <rdfs:isDefinedBy rdf:resource="http://purl.org/vocab/relationship/"/>
  </rdf:Description>

  <rdf:Description rdf:about="http://purl.org/vocab/relationship/wouldLikeToKnow">
    <rdf:type rdf:resource="http://www.w3.org/1999/02/22-rdf-syntax-ns#Property"/>
    <rdfs:subPropertyOf rdf:resource="http://xmlns.com/foaf/0.1/knows"/>
    <rdfs:label xml:lang="en">would like to now</rdfs:label>
    <skos:definition xml:lang="en">A person whom this person would desire to know more closely.</skos:definition>
    <rdfs:domain rdf:resource="http://xmlns.com/foaf/0.1/Person"/>
    <rdfs:range rdf:resource="http://xmlns.com/foaf/0.1/Person"/>
    <rdfs:isDefinedBy rdf:resource="http://purl.org/vocab/relationship/"/>
  </rdf:Description>

  <rdf:Description rdf:about="http://purl.org/vocab/relationship/knowsInPassing">
    <rdf:type rdf:resource="http://www.w3.org/1999/02/22-rdf-syntax-ns#Property"/>
    <rdfs:subPropertyOf rdf:resource="http://xmlns.com/foaf/0.1/knows"/>
    <rdfs:label xml:lang="en">knows in passing</rdfs:label>
    <skos:definition xml:lang="en">A person whom this person has slight or superficial knowledge of.</skos:definition>
    <rdfs:domain rdf:resource="http://xmlns.com/foaf/0.1/Person"/>
    <rdfs:range rdf:resource="http://xmlns.com/foaf/0.1/Person"/>
    <rdfs:isDefinedBy rdf:resource="http://purl.org/vocab/relationship/"/>
  </rdf:Description>

  <rdf:Description rdf:about="http://purl.org/vocab/relationship/knowsByReputation">
    <rdf:type rdf:resource="http://www.w3.org/1999/02/22-rdf-syntax-ns#Property"/>
    <rdfs:subPropertyOf rdf:resource="http://xmlns.com/foaf/0.1/knows"/>
    <rdfs:label xml:lang="en">knows by reputation</rdfs:label>
    <skos:definition xml:lang="en">A person known by this person primarily for a particular action, position or field of endeavour.</skos:definition>
    <rdfs:domain rdf:resource="http://xmlns.com/foaf/0.1/Person"/>
    <rdfs:range rdf:resource="http://xmlns.com/foaf/0.1/Person"/>
    <rdfs:isDefinedBy rdf:resource="http://purl.org/vocab/relationship/"/>
  </rdf:Description>

  <rdf:Description rdf:about="http://purl.org/vocab/relationship/closeFriendOf">
    <rdf:type rdf:resource="http://www.w3.org/2002/07/owl#SymmetricProperty"/>
    <rdfs:subPropertyOf rdf:resource="http://xmlns.com/foaf/0.1/knows"/>
    <rdfs:label xml:lang="en">close friend of</rdfs:label>
    <skos:definition xml:lang="en">A person who shares a close mutual friendship with this person.</skos:definition>
    <rdfs:domain rdf:resource="http://xmlns.com/foaf/0.1/Person"/>
    <rdfs:range rdf:resource="http://xmlns.com/foaf/0.1/Person"/>
    <rdfs:isDefinedBy rdf:resource="http://purl.org/vocab/relationship/"/>
  </rdf:Description>

  <rdf:Description rdf:about="http://purl.org/vocab/relationship/hasMet">
    <rdf:type rdf:resource="http://www.w3.org/2002/07/owl#SymmetricProperty"/>
    <rdfs:subPropertyOf rdf:resource="http://xmlns.com/foaf/0.1/knows"/>
    <rdfs:label xml:lang="en">has met</rdfs:label>
    <skos:definition xml:lang="en">A person who has met this person whether in passing or longer.</skos:definition>
    <rdfs:domain rdf:resource="http://xmlns.com/foaf/0.1/Person"/>
    <rdfs:range rdf:resource="http://xmlns.com/foaf/0.1/Person"/>
    <rdfs:isDefinedBy rdf:resource="http://purl.org/vocab/relationship/"/>
  </rdf:Description>

  <rdf:Description rdf:about="http://purl.org/vocab/relationship/worksWith">
    <rdf:type rdf:resource="http://www.w3.org/2002/07/owl#SymmetricProperty"/>
    <rdf:type rdf:resource="http://www.w3.org/2002/07/owl#TransitiveProperty"/>
    <rdfs:subPropertyOf rdf:resource="http://xmlns.com/foaf/0.1/knows"/>
    <rdfs:label xml:lang="en">works with</rdfs:label>
    <skos:definition xml:lang="en">A person who works for the same employer as this person.</skos:definition>
    <rdfs:domain rdf:resource="http://xmlns.com/foaf/0.1/Person"/>
    <rdfs:range rdf:resource="http://xmlns.com/foaf/0.1/Person"/>
    <rdfs:isDefinedBy rdf:resource="http://purl.org/vocab/relationship/"/>
  </rdf:Description>

  <rdf:Description rdf:about="http://purl.org/vocab/relationship/colleagueOf">
    <rdf:type rdf:resource="http://www.w3.org/2002/07/owl#SymmetricProperty"/>
    <rdfs:subPropertyOf rdf:resource="http://xmlns.com/foaf/0.1/knows"/>
    <rdfs:label xml:lang="en">colleague of</rdfs:label>
    <skos:definition xml:lang="en">A person who is a member of the same profession as this person.</skos:definition>
    <rdfs:domain rdf:resource="http://xmlns.com/foaf/0.1/Person"/>
    <rdfs:range rdf:resource="http://xmlns.com/foaf/0.1/Person"/>
    <rdfs:isDefinedBy rdf:resource="http://purl.org/vocab/relationship/"/>
  </rdf:Description>

  <rdf:Description rdf:about="http://purl.org/vocab/relationship/collaboratesWith">
    <rdf:type rdf:resource="http://www.w3.org/2002/07/owl#SymmetricProperty"/>
    <rdfs:subPropertyOf rdf:resource="http://xmlns.com/foaf/0.1/knows"/>
    <rdfs:label xml:lang="en">collaborates with</rdfs:label>
    <skos:definition xml:lang="en">A person who works towards a common goal with this person.</skos:definition>
    <rdfs:domain rdf:resource="http://xmlns.com/foaf/0.1/Person"/>
    <rdfs:range rdf:resource="http://xmlns.com/foaf/0.1/Person"/>
    <rdfs:isDefinedBy rdf:resource="http://purl.org/vocab/relationship/"/>
  </rdf:Description>

  <rdf:Description rdf:about="http://purl.org/vocab/relationship/employerOf">
    <rdf:type rdf:resource="http://www.w3.org/1999/02/22-rdf-syntax-ns#Property"/>
    <owl:inverseOf rdf:resource="http://purl.org/vocab/relationship/employedBy"/>
    <rdfs:subPropertyOf rdf:resource="http://xmlns.com/foaf/0.1/knows"/>
    <rdfs:label xml:lang="en">employer of</rdfs:label>
    <skos:definition xml:lang="en">A person who engages the services of this person.</skos:definition>
    <rdfs:domain rdf:resource="http://xmlns.com/foaf/0.1/Person"/>
    <rdfs:range rdf:resource="http://xmlns.com/foaf/0.1/Person"/>
    <rdfs:isDefinedBy rdf:resource="http://purl.org/vocab/relationship/"/>
  </rdf:Description>

  <rdf:Description rdf:about="http://purl.org/vocab/relationship/employedBy">
    <rdf:type rdf:resource="http://www.w3.org/1999/02/22-rdf-syntax-ns#Property"/>
    <owl:inverseOf rdf:resource="http://purl.org/vocab/relationship/employerOf"/>
    <rdfs:subPropertyOf rdf:resource="http://xmlns.com/foaf/0.1/knows"/>
    <rdfs:label xml:lang="en">employed by</rdfs:label>
    <skos:definition xml:lang="en">A person for whom this person's services have been engaged.</skos:definition>
    <rdfs:domain rdf:resource="http://xmlns.com/foaf/0.1/Person"/>
    <rdfs:range rdf:resource="http://xmlns.com/foaf/0.1/Person"/>
    <rdfs:isDefinedBy rdf:resource="http://purl.org/vocab/relationship/"/>
  </rdf:Description>

  <rdf:Description rdf:about="http://purl.org/vocab/relationship/mentorOf">
    <rdf:type rdf:resource="http://www.w3.org/1999/02/22-rdf-syntax-ns#Property"/>
    <owl:inverseOf rdf:resource="http://purl.org/vocab/relationship/apprenticeTo"/>
    <rdfs:subPropertyOf rdf:resource="http://xmlns.com/foaf/0.1/knows"/>
    <rdfs:label xml:lang="en">mentor of</rdfs:label>
    <skos:definition xml:lang="en">A person who serves as a trusted counselor or teacher to this person.</skos:definition>
    <rdfs:domain rdf:resource="http://xmlns.com/foaf/0.1/Person"/>
    <rdfs:range rdf:resource="http://xmlns.com/foaf/0.1/Person"/>
    <rdfs:isDefinedBy rdf:resource="http://purl.org/vocab/relationship/"/>
  </rdf:Description>

  <rdf:Description rdf:about="http://purl.org/vocab/relationship/apprenticeTo">
    <rdf:type rdf:resource="http://www.w3.org/1999/02/22-rdf-syntax-ns#Property"/>
    <owl:inverseOf rdf:resource="http://purl.org/vocab/relationship/mentorOf"/>
    <rdfs:subPropertyOf rdf:resource="http://xmlns.com/foaf/0.1/knows"/>
    <rdfs:label xml:lang="en">apprentice to</rdfs:label>
    <skos:definition xml:lang="en">A person to whom this person serves as a trusted counselor or teacher.</skos:definition>
    <rdfs:domain rdf:resource="http://xmlns.com/foaf/0.1/Person"/>
    <rdfs:range rdf:resource="http://xmlns.com/foaf/0.1/Person"/>
    <rdfs:isDefinedBy rdf:resource="http://purl.org/vocab/relationship/"/>
  </rdf:Description>

  <rdf:Description rdf:about="http://purl.org/vocab/relationship/livesWith">
    <rdf:type rdf:resource="http://www.w3.org/2002/07/owl#SymmetricProperty"/>
    <rdf:type rdf:resource="http://www.w3.org/2002/07/owl#TransitiveProperty"/>
    <rdfs:isDefinedBy rdf:resource="http://purl.org/vocab/relationship/"/>
    <rdfs:subPropertyOf rdf:resource="http://xmlns.com/foaf/0.1/knows"/>
    <rdfs:label xml:lang="en">lives with</rdfs:label>
    <skos:definition xml:lang="en">A person who shares a residence with this person.</skos:definition>
    <rdfs:domain rdf:resource="http://xmlns.com/foaf/0.1/Person"/>
    <rdfs:range rdf:resource="http://xmlns.com/foaf/0.1/Person"/>
  </rdf:Description>

  <rdf:Description rdf:about="http://purl.org/vocab/relationship/neighborOf">
    <rdf:type rdf:resource="http://www.w3.org/2002/07/owl#SymmetricProperty"/>
    <rdf:type rdf:resource="http://www.w3.org/2002/07/owl#TransitiveProperty"/>
    <rdfs:subPropertyOf rdf:resource="http://xmlns.com/foaf/0.1/knows"/>
    <rdfs:label xml:lang="en">neighbor of</rdfs:label>
    <skos:definition xml:lang="en">A person who lives in the same locality as this person.</skos:definition>
    <rdfs:domain rdf:resource="http://xmlns.com/foaf/0.1/Person"/>
    <rdfs:range rdf:resource="http://xmlns.com/foaf/0.1/Person"/>
    <rdfs:isDefinedBy rdf:resource="http://purl.org/vocab/relationship/"/>
  </rdf:Description>

  <rdf:Description rdf:about="http://purl.org/vocab/relationship/grandparentOf">
    <rdf:type rdf:resource="http://www.w3.org/1999/02/22-rdf-syntax-ns#Property"/>
    <owl:inverseOf rdf:resource="http://purl.org/vocab/relationship/grandchildOf"/>
    <rdfs:subPropertyOf rdf:resource="http://xmlns.com/foaf/0.1/knows"/>
    <rdfs:label xml:lang="en">grandparent of</rdfs:label>
    <skos:definition xml:lang="en">A person who is the parent of any of this person's parents.</skos:definition>
    <rdfs:domain rdf:resource="http://xmlns.com/foaf/0.1/Person"/>
    <rdfs:range rdf:resource="http://xmlns.com/foaf/0.1/Person"/>
    <rdfs:isDefinedBy rdf:resource="http://purl.org/vocab/relationship/"/>
  </rdf:Description>

  <rdf:Description rdf:about="http://purl.org/vocab/relationship/lifePartnerOf">
    <rdf:type rdf:resource="http://www.w3.org/2002/07/owl#SymmetricProperty"/>
    <rdfs:subPropertyOf rdf:resource="http://xmlns.com/foaf/0.1/knows"/>
    <rdfs:label xml:lang="en">life partner of</rdfs:label>
    <skos:definition xml:lang="en">A person who has made a long-term commitment to this person's.</skos:definition>
    <rdfs:domain rdf:resource="http://xmlns.com/foaf/0.1/Person"/>
    <rdfs:range rdf:resource="http://xmlns.com/foaf/0.1/Person"/>
    <rdfs:isDefinedBy rdf:resource="http://purl.org/vocab/relationship/"/>
  </rdf:Description>

  <rdf:Description rdf:about="http://purl.org/vocab/relationship/engagedTo">
    <rdf:type rdf:resource="http://www.w3.org/2002/07/owl#SymmetricProperty"/>
    <rdfs:subPropertyOf rdf:resource="http://xmlns.com/foaf/0.1/knows"/>
    <rdfs:label xml:lang="en">engaged to</rdfs:label>
    <skos:definition xml:lang="en">A person to whom this person is betrothed.</skos:definition>
    <rdfs:domain rdf:resource="http://xmlns.com/foaf/0.1/Person"/>
    <rdfs:range rdf:resource="http://xmlns.com/foaf/0.1/Person"/>
    <rdfs:isDefinedBy rdf:resource="http://purl.org/vocab/relationship/"/>
  </rdf:Description>

  <rdf:Description rdf:about="http://purl.org/vocab/relationship/ancestorOf">
    <rdf:type rdf:resource="http://www.w3.org/2002/07/owl#TransitiveProperty"/>
    <owl:inverseOf rdf:resource="http://purl.org/vocab/relationship/descendantOf"/>
    <rdfs:subPropertyOf rdf:resource="http://xmlns.com/foaf/0.1/knows"/>
    <rdfs:label xml:lang="en">ancestor of</rdfs:label>
    <skos:definition xml:lang="en">A person who is a descendant of this person.</skos:definition>
    <rdfs:domain rdf:resource="http://xmlns.com/foaf/0.1/Person"/>
    <rdfs:range rdf:resource="http://xmlns.com/foaf/0.1/Person"/>
    <rdfs:isDefinedBy rdf:resource="http://purl.org/vocab/relationship/"/>
  </rdf:Description>

  <rdf:Description rdf:about="http://purl.org/vocab/relationship/descendantOf">
    <rdfs:label>Descendant Of</rdfs:label>
    <rdfs:label xml:lang="en">descendant of</rdfs:label>
    <rdf:type rdf:resource="http://www.w3.org/2002/07/owl#TransitiveProperty"/>
    <owl:inverseOf rdf:resource="http://purl.org/vocab/relationship/ancestorOf"/>
    <rdfs:subPropertyOf rdf:resource="http://xmlns.com/foaf/0.1/knows"/>
    <skos:definition xml:lang="en">A person from whom this person is descended.</skos:definition>
    <rdfs:domain rdf:resource="http://xmlns.com/foaf/0.1/Person"/>
    <rdfs:range rdf:resource="http://xmlns.com/foaf/0.1/Person"/>
    <rdfs:isDefinedBy rdf:resource="http://purl.org/vocab/relationship/"/>
  </rdf:Description>

  <rdf:Description rdf:about="http://purl.org/vocab/relationship/participantIn">
    <rdf:type rdf:resource="http://www.w3.org/1999/02/22-rdf-syntax-ns#Property"/>
    <rdfs:subPropertyOf rdf:resource="http://xmlns.com/foaf/0.1/knows"/>
    <rdfs:label xml:lang="en">participant in</rdfs:label>
    <rdfs:domain rdf:resource="http://xmlns.com/foaf/0.1/Person"/>
    <rdfs:range rdf:resource="http://purl.org/vocab/relationship/Relationship"/>
    <rdfs:isDefinedBy rdf:resource="http://purl.org/vocab/relationship/"/>
  </rdf:Description>

  <rdf:Description rdf:about="http://purl.org/vocab/relationship/participant">
    <rdf:type rdf:resource="http://www.w3.org/1999/02/22-rdf-syntax-ns#Property"/>
    <rdfs:subPropertyOf rdf:resource="http://xmlns.com/foaf/0.1/knows"/>
    <rdfs:label xml:lang="en">participant</rdfs:label>
    <rdfs:domain rdf:resource="http://purl.org/vocab/relationship/Relationship"/>
    <rdfs:range rdf:resource="http://xmlns.com/foaf/0.1/Person"/>
    <rdfs:isDefinedBy rdf:resource="http://purl.org/vocab/relationship/"/>
  </rdf:Description>

  <rdf:Description rdf:about="http://purl.org/vocab/relationship/influencedBy">
    <rdf:type rdf:resource="http://www.w3.org/1999/02/22-rdf-syntax-ns#Property"/>
    <rdfs:subPropertyOf rdf:resource="http://xmlns.com/foaf/0.1/knows"/>
    <rdfs:label xml:lang="en">influenced by</rdfs:label>
    <skos:definition xml:lang="en">a person who has influenced this person.</skos:definition>
    <rdfs:domain rdf:resource="http://xmlns.com/foaf/0.1/Person"/>
    <rdfs:range rdf:resource="http://xmlns.com/foaf/0.1/Person"/>
    <rdfs:isDefinedBy rdf:resource="http://purl.org/vocab/relationship/"/>
  </rdf:Description>


<!-- TAGS -->

    <owl:ObjectProperty rdf:about="http://www.holygoat.co.uk/owl/redwood/0.1/tags/associatedTag">
        <rdfs:comment xml:lang="en">The object is a Tag which plays a role in the subject Tagging.</rdfs:comment>
        <rdfs:domain rdf:resource="http://www.holygoat.co.uk/owl/redwood/0.1/tags/Tagging"/>
        <rdfs:label>associated tag</rdfs:label>
        <rdfs:range rdf:resource="http://www.holygoat.co.uk/owl/redwood/0.1/tags/Tag"/>
        <vs:term_status>testing</vs:term_status>
    </owl:ObjectProperty>

    <owl:ObjectProperty rdf:about="http://www.holygoat.co.uk/owl/redwood/0.1/tags/equivalentTag">
        <rdfs:comment xml:lang="en">The two tags are asserted to be equivalent --- that is, that whenever one is associated with a resource, the other tag can be logically inferred to also be associated. Be very careful with this. I'm not sure if this should be a subproperty of owl:sameAs.</rdfs:comment>
        <rdfs:domain rdf:resource="http://www.holygoat.co.uk/owl/redwood/0.1/tags/Tag"/>
        <rdfs:label xml:lang="en">equivalent tag</rdfs:label>
        <rdfs:range rdf:resource="http://www.holygoat.co.uk/owl/redwood/0.1/tags/Tag"/>
        <rdfs:subPropertyOf rdf:resource="http://www.w3.org/2002/07/owl#sameAs"/>
        <vs:term_status>testing</vs:term_status>
    </owl:ObjectProperty>

    <owl:ObjectProperty rdf:about="http://www.holygoat.co.uk/owl/redwood/0.1/tags/isTagOf">
        <rdfs:comment xml:lang="en">Indicates that the subject tag applies to the object resource. This does not assert by who, when, or why the tagging occurred. For that information, use a reified Tagging resource.</rdfs:comment>
        <rdfs:domain rdf:resource="http://www.holygoat.co.uk/owl/redwood/0.1/tags/Tag"/>
        <rdfs:label xml:lang="en">is tag of</rdfs:label>
        <owl:inverseOf rdf:resource="http://www.holygoat.co.uk/owl/redwood/0.1/tags/taggedWithTag"/>
    </owl:ObjectProperty>

    <owl:DatatypeProperty rdf:about="http://www.holygoat.co.uk/owl/redwood/0.1/tags/name">
        <rdfs:comment xml:lang="en">The name of a tag. Note that we can't relate this to skos:prefLabel because we cannot guarantee that tags have unique labels in a given conceptual scheme. Or can we?</rdfs:comment>
        <rdfs:domain rdf:resource="http://www.holygoat.co.uk/owl/redwood/0.1/tags/Tag"/>
        <rdfs:label xml:lang="en">tag name</rdfs:label>
        <rdfs:subPropertyOf rdf:resource="http://purl.org/dc/elements/1.1/title"/>
        <rdfs:subPropertyOf rdf:resource="http://www.w3.org/2000/01/rdf-schema#label"/>
    </owl:DatatypeProperty>

    <owl:ObjectProperty rdf:about="http://www.holygoat.co.uk/owl/redwood/0.1/tags/relatedTag">
        <rdfs:comment xml:lang="en">The two tags are asserted as being related. This might be symmetric, but it certainly isn't transitive.</rdfs:comment>
        <rdfs:domain rdf:resource="http://www.holygoat.co.uk/owl/redwood/0.1/tags/Tag"/>
        <rdfs:label xml:lang="en">related tag</rdfs:label>
        <rdfs:range rdf:resource="http://www.holygoat.co.uk/owl/redwood/0.1/tags/Tag"/>
        <rdfs:subPropertyOf rdf:resource="http://www.w3.org/2004/02/skos/core#semanticRelation"/>
        <vs:term_status>testing</vs:term_status>
    </owl:ObjectProperty>

    <owl:ObjectProperty rdf:about="http://www.holygoat.co.uk/owl/redwood/0.1/tags/tag">
        <rdfs:comment xml:lang="en">The relationship between a resource and a Tagging. Note, of course, that this allows us to tag tags and taggings themselves...</rdfs:comment>
        <rdfs:label xml:lang="en">tag</rdfs:label>
        <rdfs:range rdf:resource="http://www.holygoat.co.uk/owl/redwood/0.1/tags/Tagging"/>
    </owl:ObjectProperty>

    <owl:DatatypeProperty rdf:about="http://www.holygoat.co.uk/owl/redwood/0.1/tags/tagName">
        <rdfs:comment xml:lang="en">The name of a tag. Note that we can't relate this to skos:prefLabel because we cannot guarantee that tags have unique labels in a given conceptual scheme. Or can we? DEPRECATED 2005-05-19: redundant 'tag'.</rdfs:comment>
        <rdfs:domain rdf:resource="http://www.holygoat.co.uk/owl/redwood/0.1/tags/Tag"/>
        <rdfs:label xml:lang="en">tag name</rdfs:label>
        <rdfs:subPropertyOf rdf:resource="http://purl.org/dc/elements/1.1/title"/>
        <rdfs:subPropertyOf rdf:resource="http://www.w3.org/2000/01/rdf-schema#label"/>
    </owl:DatatypeProperty>

    <owl:ObjectProperty rdf:about="http://www.holygoat.co.uk/owl/redwood/0.1/tags/taggedBy">
        <rdfs:comment xml:lang="en">The object plays the role of the tagger in the subject Tagging.</rdfs:comment>
        <rdfs:domain rdf:resource="http://www.holygoat.co.uk/owl/redwood/0.1/tags/Tagging"/>
        <rdfs:label xml:lang="en">tagged by</rdfs:label>
        <rdfs:range rdf:resource="http://xmlns.com/foaf/0.1/Agent"/>
        <vs:term_status>testing</vs:term_status>
    </owl:ObjectProperty>

    <owl:DatatypeProperty rdf:about="http://www.holygoat.co.uk/owl/redwood/0.1/tags/taggedOn">
        <rdfs:comment xml:lang="en">The subject Tagging occurred at the subject time and date.</rdfs:comment>
        <rdfs:domain rdf:resource="http://www.holygoat.co.uk/owl/redwood/0.1/tags/Tagging"/>
        <rdfs:label xml:lang="en">tagged on</rdfs:label>
        <rdfs:subPropertyOf rdf:resource="http://purl.org/dc/elements/1.1/date"/>
        <vs:term_status>testing</vs:term_status>
    </owl:DatatypeProperty>

    <owl:ObjectProperty rdf:about="http://www.holygoat.co.uk/owl/redwood/0.1/tags/taggedResource">
        <rdfs:comment xml:lang="en">The object is a resource which plays a role in the subject Tagging.</rdfs:comment>
        <rdfs:domain rdf:resource="http://www.holygoat.co.uk/owl/redwood/0.1/tags/Tagging"/>
        <rdfs:label xml:lang="en">tagged resource</rdfs:label>
        <vs:term_status>testing</vs:term_status>
    </owl:ObjectProperty>

    <owl:ObjectProperty rdf:about="http://www.holygoat.co.uk/owl/redwood/0.1/tags/taggedWithTag">
        <rdfs:comment xml:lang="en">Indicates that the subject has been tagged with the object tag. This does not assert by who, when, or why the tagging occurred. For that information, use a reified Tagging resource.</rdfs:comment>
        <rdfs:label xml:lang="en">tagged with tag</rdfs:label>
        <rdfs:range rdf:resource="http://www.holygoat.co.uk/owl/redwood/0.1/tags/Tag"/>
        <rdfs:subPropertyOf rdf:resource="http://www.w3.org/2004/02/skos/core#subject"/>
    </owl:ObjectProperty>




    <owl:DatatypeProperty rdf:about="http://ns.ontowiki.net/SysOnt/order" rdfs:label="order">
      <rdf:type rdf:resource="&owl;FunctionalProperty"/>
      <rdfs:domain rdf:resource="&owl;Thing"/>
      <rdfs:range rdf:resource="&xsd;nonNegativeInteger"/>
    </owl:DatatypeProperty>

</rdf:RDF>


